<?xml version="1.0"?>
<rdf:RDF xmlns="http://www.dronetology.net/dronetology#"
     xml:base="http://www.dronetology.net/dronetology"
     xmlns:qudt="http://qudt.org/schema/qudt/"
     xmlns:owl="http://www.w3.org/2002/07/owl#"
     xmlns:xsd="http://www.w3.org/2001/XMLSchema#"
     xmlns:rdfs="http://www.w3.org/2000/01/rdf-schema#"
     xmlns:ssn="http://www.w3.org/ns/ssn/"
     xmlns:geo1="http://www.w3.org/2003/01/geo/"
     xmlns:geo="http://www.opengis.net/ont/geosparql"
     xmlns:ont="http://www.opengis.net/ont/"
     xmlns:rdf="http://www.w3.org/1999/02/22-rdf-syntax-ns#"
     xmlns:pos="http://www.w3.org/2003/01/geo/pos#"
     xmlns:terms="http://purl.org/dc/terms/"
     xmlns:xml="http://www.w3.org/XML/1998/namespace"
     xmlns:DUL="http://www.ontologydesignpatterns.org/ont/dul/DUL.owl#"
     xmlns:time="http://www.w3.org/2006/time#"
     xmlns:dc="http://purl.org/dc/elements/1.1/"
     xmlns:sosa="http://www.w3.org/ns/sosa/">
    <owl:Ontology rdf:about="http://www.dronetology.net/dronetology#">
        <dc:contributor rdf:datatype="http://www.w3.org/2001/XMLSchema#string">Alberto Córdoba</dc:contributor>
        <terms:license rdf:resource="http://www.dronetology.net/dronetology#DronetologyLicenseTerms"/>
        <dc:contributor rdf:datatype="http://www.w3.org/2001/XMLSchema#string">José Javier Astrain</dc:contributor>
        <dc:abstract rdf:datatype="http://www.w3.org/2001/XMLSchema#string">Dronetology aims to define the knowledge necessary for a UAV to operate autonomously and infer new knowledge,
necessary for a UAV to operate autonomously and to infer new knowledge to improve the efficiency and safety of the mission.</dc:abstract>
        <dc:rights rdf:datatype="http://www.w3.org/2001/XMLSchema#string"></dc:rights>
        <dc:contributor rdf:datatype="http://www.w3.org/2001/XMLSchema#string">Jesús Villadangos</dc:contributor>
        <dc:creator rdf:datatype="http://www.w3.org/2001/XMLSchema#string">David Martín-Lammerding</dc:creator>
        <dc:title rdf:datatype="http://www.w3.org/2001/XMLSchema#string">Dronetology</dc:title>
    </owl:Ontology>
    


    <!-- 
    ///////////////////////////////////////////////////////////////////////////////////////
    //
    // Annotation properties
    //
    ///////////////////////////////////////////////////////////////////////////////////////
     -->

    


    <!-- http://purl.org/dc/elements/1.1/abstract -->

    <owl:AnnotationProperty rdf:about="http://purl.org/dc/elements/1.1/abstract"/>
    


    <!-- http://purl.org/dc/elements/1.1/contributor -->

    <owl:AnnotationProperty rdf:about="http://purl.org/dc/elements/1.1/contributor"/>
    


    <!-- http://purl.org/dc/elements/1.1/creator -->

    <owl:AnnotationProperty rdf:about="http://purl.org/dc/elements/1.1/creator"/>
    


    <!-- http://purl.org/dc/elements/1.1/description -->

    <owl:AnnotationProperty rdf:about="http://purl.org/dc/elements/1.1/description"/>
    


    <!-- http://purl.org/dc/elements/1.1/rights -->

    <owl:AnnotationProperty rdf:about="http://purl.org/dc/elements/1.1/rights"/>
    


    <!-- http://purl.org/dc/elements/1.1/subject -->

    <owl:AnnotationProperty rdf:about="http://purl.org/dc/elements/1.1/subject"/>
    


    <!-- http://purl.org/dc/elements/1.1/title -->

    <owl:AnnotationProperty rdf:about="http://purl.org/dc/elements/1.1/title"/>
    


    <!-- http://purl.org/dc/terms/license -->

    <owl:AnnotationProperty rdf:about="http://purl.org/dc/terms/license"/>
    


    <!-- http://www.dronetology.net/dronetology#hasInterval -->

    <owl:AnnotationProperty rdf:about="http://www.dronetology.net/dronetology#hasInterval"/>
    


    <!-- http://www.dronetology.net/dronetology#hasLatLon -->

    <owl:AnnotationProperty rdf:about="http://www.dronetology.net/dronetology#hasLatLon"/>
    


    <!-- http://www.dronetology.net/dronetology#hasMeasurementZValue -->

    <owl:AnnotationProperty rdf:about="http://www.dronetology.net/dronetology#hasMeasurementZValue">
        <rdfs:range rdf:resource="http://www.w3.org/2001/XMLSchema#float"/>
        <rdfs:domain rdf:resource="http://www.dronetology.net/dronetology#Parameter"/>
        <rdfs:domain rdf:resource="http://www.dronetology.net/dronetology#VectorParameter"/>
    </owl:AnnotationProperty>
    


    <!-- http://www.dronetology.net/dronetology#hasParameterName -->

    <owl:AnnotationProperty rdf:about="http://www.dronetology.net/dronetology#hasParameterName">
        <rdfs:range rdf:resource="http://www.w3.org/2001/XMLSchema#string"/>
        <rdfs:domain rdf:resource="http://www.dronetology.net/dronetology#Parameter"/>
    </owl:AnnotationProperty>
    


    <!-- http://www.dronetology.net/dronetology#hasParameterUnit -->

    <owl:AnnotationProperty rdf:about="http://www.dronetology.net/dronetology#hasParameterUnit"/>
    


    <!-- http://www.dronetology.net/dronetology#hasType -->

    <owl:AnnotationProperty rdf:about="http://www.dronetology.net/dronetology#hasType"/>
    


    <!-- http://www.dronetology.net/dronetology#hasTypeId -->

    <owl:AnnotationProperty rdf:about="http://www.dronetology.net/dronetology#hasTypeId"/>
    


    <!-- http://www.ontologydesignpatterns.org/ont/dul/DUL.owl#satisfies -->

    <owl:AnnotationProperty rdf:about="http://www.ontologydesignpatterns.org/ont/dul/DUL.owl#satisfies"/>
    


    <!-- http://www.opengis.net/ont/geosparqllat -->

    <owl:AnnotationProperty rdf:about="http://www.opengis.net/ont/geosparqllat"/>
    


    <!-- http://www.opengis.net/ont/geosparqllat_long -->

    <owl:AnnotationProperty rdf:about="http://www.opengis.net/ont/geosparqllat_long"/>
    


    <!-- http://www.opengis.net/ont/geosparqllong -->

    <owl:AnnotationProperty rdf:about="http://www.opengis.net/ont/geosparqllong"/>
    


    <!-- http://www.w3.org/2000/01/rdf-schema#subClassOf -->

    <owl:AnnotationProperty rdf:about="http://www.w3.org/2000/01/rdf-schema#subClassOf"/>
    


    <!-- http://www.w3.org/2002/07/owl#maxCardinality -->

    <owl:AnnotationProperty rdf:about="http://www.w3.org/2002/07/owl#maxCardinality"/>
    


    <!-- http://www.w3.org/2002/07/owl#minCardinality -->

    <owl:AnnotationProperty rdf:about="http://www.w3.org/2002/07/owl#minCardinality"/>
    


    <!-- http://www.w3.org/2002/07/owl#qualifiedCardinality -->

    <owl:AnnotationProperty rdf:about="http://www.w3.org/2002/07/owl#qualifiedCardinality"/>
    


    <!-- http://www.w3.org/2003/01/geo/lat -->

    <owl:AnnotationProperty rdf:about="http://www.w3.org/2003/01/geo/lat"/>
    


    <!-- http://www.w3.org/2003/01/geo/lat_long -->

    <owl:AnnotationProperty rdf:about="http://www.w3.org/2003/01/geo/lat_long"/>
    


    <!-- http://www.w3.org/2003/01/geo/long -->

    <owl:AnnotationProperty rdf:about="http://www.w3.org/2003/01/geo/long"/>
    


    <!-- 
    ///////////////////////////////////////////////////////////////////////////////////////
    //
    // Object Properties
    //
    ///////////////////////////////////////////////////////////////////////////////////////
     -->

    


    <!-- http://qudt.org/schema/qudt/hasUnit -->

    <owl:ObjectProperty rdf:about="http://qudt.org/schema/qudt/hasUnit">
        <owl:inverseOf rdf:resource="http://www.dronetology.net/dronetology#isUnitOf"/>
        <rdfs:domain rdf:resource="http://qudt.org/schema/qudt/Quantity"/>
        <rdfs:range rdf:resource="http://qudt.org/schema/qudt/Unit"/>
        <rdfs:comment xml:lang="en">hasUnit. Relates a quantity with a unit of measurement.</rdfs:comment>
        <rdfs:label xml:lang="en">hasUnit</rdfs:label>
    </owl:ObjectProperty>
    


    <!-- http://qudt.org/schema/qudt/value -->

    <owl:ObjectProperty rdf:about="http://qudt.org/schema/qudt/value"/>
    


    <!-- http://www.dronetology.net/dronetology#activates -->

    <owl:ObjectProperty rdf:about="http://www.dronetology.net/dronetology#activates">
        <owl:inverseOf rdf:resource="http://www.dronetology.net/dronetology#isActivatedBy"/>
        <rdfs:domain rdf:resource="http://www.dronetology.net/dronetology#CommunicationMessage"/>
        <rdfs:range rdf:resource="http://www.dronetology.net/dronetology#Alarm"/>
        <rdfs:comment xml:lang="en">activates. Relates a message with an alarm.</rdfs:comment>
        <rdfs:label xml:lang="en">activates</rdfs:label>
    </owl:ObjectProperty>
    


    <!-- http://www.dronetology.net/dronetology#collaboratedBy -->

    <owl:ObjectProperty rdf:about="http://www.dronetology.net/dronetology#collaboratedBy">
        <rdfs:subPropertyOf rdf:resource="http://www.dronetology.net/dronetology#hasARelationshipWith"/>
        <owl:inverseOf rdf:resource="http://www.dronetology.net/dronetology#collaborates"/>
        <rdfs:comment xml:lang="en">collaboratedBy. Relates two drones that collaborate.</rdfs:comment>
        <rdfs:label xml:lang="en">collaboratedBy</rdfs:label>
    </owl:ObjectProperty>
    


    <!-- http://www.dronetology.net/dronetology#collaborates -->

    <owl:ObjectProperty rdf:about="http://www.dronetology.net/dronetology#collaborates">
        <rdfs:subPropertyOf rdf:resource="http://www.dronetology.net/dronetology#hasARelationshipWith"/>
        <rdfs:comment xml:lang="en">collaborates. Relates two drones that collaborate.</rdfs:comment>
        <rdfs:label xml:lang="en">collaborates</rdfs:label>
    </owl:ObjectProperty>
    


    <!-- http://www.dronetology.net/dronetology#combinationOf -->

    <owl:ObjectProperty rdf:about="http://www.dronetology.net/dronetology#combinationOf">
        <owl:inverseOf rdf:resource="http://www.dronetology.net/dronetology#decompositionOf"/>
        <rdfs:domain rdf:resource="http://www.dronetology.net/dronetology#Requirement"/>
        <rdfs:range rdf:resource="http://www.dronetology.net/dronetology#Requirement"/>
        <rdfs:comment xml:lang="en">combinationOf. Relates a requirement with sub-requirements following a hierarchical structure.</rdfs:comment>
        <rdfs:label xml:lang="en">combinationOf</rdfs:label>
    </owl:ObjectProperty>
    


    <!-- http://www.dronetology.net/dronetology#combinesTo -->

    <owl:ObjectProperty rdf:about="http://www.dronetology.net/dronetology#combinesTo">
        <owl:inverseOf rdf:resource="http://www.dronetology.net/dronetology#decomposesTo"/>
        <rdfs:domain rdf:resource="http://www.dronetology.net/dronetology#Function"/>
        <rdfs:range rdf:resource="http://www.dronetology.net/dronetology#Function"/>
        <rdfs:comment xml:lang="en">combinesTo. Relates a sub-functions with a high level function.</rdfs:comment>
        <rdfs:label xml:lang="en">combinesTo</rdfs:label>
    </owl:ObjectProperty>
    


    <!-- http://www.dronetology.net/dronetology#complyWith -->

    <owl:ObjectProperty rdf:about="http://www.dronetology.net/dronetology#complyWith">
        <owl:inverseOf rdf:resource="http://www.dronetology.net/dronetology#isFulfilledBy"/>
        <rdfs:domain rdf:resource="http://www.dronetology.net/dronetology#Drone"/>
        <rdfs:range rdf:resource="http://www.dronetology.net/dronetology#Regulation"/>
        <rdfs:comment xml:lang="en">complyWith. Relates a Drone with a Regulation.</rdfs:comment>
        <rdfs:label xml:lang="en">complyWith</rdfs:label>
    </owl:ObjectProperty>
    


    <!-- http://www.dronetology.net/dronetology#constrainedBy -->

    <owl:ObjectProperty rdf:about="http://www.dronetology.net/dronetology#constrainedBy">
        <owl:inverseOf rdf:resource="http://www.dronetology.net/dronetology#constrains"/>
        <rdfs:domain rdf:resource="http://www.dronetology.net/dronetology#Parameter"/>
        <rdfs:range rdf:resource="http://www.dronetology.net/dronetology#Constraint"/>
        <rdfs:comment xml:lang="en">constrainedBy. Relates a parameter that constrain a specific product constrain.</rdfs:comment>
        <rdfs:label xml:lang="en">constrainedBy</rdfs:label>
    </owl:ObjectProperty>
    


    <!-- http://www.dronetology.net/dronetology#constrains -->

    <owl:ObjectProperty rdf:about="http://www.dronetology.net/dronetology#constrains">
        <rdfs:domain rdf:resource="http://www.dronetology.net/dronetology#Constraint"/>
        <rdfs:range rdf:resource="http://www.dronetology.net/dronetology#Parameter"/>
        <rdfs:comment xml:lang="en">constraint. Relates a producto constraint with a parameter</rdfs:comment>
        <rdfs:label xml:lang="en">constrains</rdfs:label>
    </owl:ObjectProperty>
    


    <!-- http://www.dronetology.net/dronetology#cooperatedBy -->

    <owl:ObjectProperty rdf:about="http://www.dronetology.net/dronetology#cooperatedBy">
        <rdfs:subPropertyOf rdf:resource="http://www.dronetology.net/dronetology#hasARelationshipWith"/>
        <owl:inverseOf rdf:resource="http://www.dronetology.net/dronetology#cooperates"/>
        <rdfs:domain rdf:resource="http://www.dronetology.net/dronetology#Drone"/>
        <rdfs:range rdf:resource="http://www.dronetology.net/dronetology#Drone"/>
        <rdfs:comment xml:lang="en">cooperatedBy. Relates two drones that cooperate.</rdfs:comment>
        <rdfs:label xml:lang="en">cooperatedBy</rdfs:label>
    </owl:ObjectProperty>
    


    <!-- http://www.dronetology.net/dronetology#cooperates -->

    <owl:ObjectProperty rdf:about="http://www.dronetology.net/dronetology#cooperates">
        <rdfs:subPropertyOf rdf:resource="http://www.dronetology.net/dronetology#hasARelationshipWith"/>
        <rdfs:domain rdf:resource="http://www.dronetology.net/dronetology#Drone"/>
        <rdfs:range rdf:resource="http://www.dronetology.net/dronetology#Drone"/>
        <rdfs:comment xml:lang="en">cooperates. Relates two drones that cooperate.</rdfs:comment>
        <rdfs:label xml:lang="en">cooperates</rdfs:label>
    </owl:ObjectProperty>
    


    <!-- http://www.dronetology.net/dronetology#coordinatedBy -->

    <owl:ObjectProperty rdf:about="http://www.dronetology.net/dronetology#coordinatedBy">
        <rdfs:subPropertyOf rdf:resource="http://www.dronetology.net/dronetology#hasARelationshipWith"/>
        <owl:inverseOf rdf:resource="http://www.dronetology.net/dronetology#coordinates"/>
        <rdfs:comment xml:lang="en">coordinatedBy.  Relates two drones that coordinate.</rdfs:comment>
        <rdfs:label xml:lang="en">coordinatesBy</rdfs:label>
    </owl:ObjectProperty>
    


    <!-- http://www.dronetology.net/dronetology#coordinates -->

    <owl:ObjectProperty rdf:about="http://www.dronetology.net/dronetology#coordinates">
        <rdfs:subPropertyOf rdf:resource="http://www.dronetology.net/dronetology#hasARelationshipWith"/>
        <rdfs:comment xml:lang="en">coordinates.  Relates two drones that coordinate.</rdfs:comment>
        <rdfs:label xml:lang="en">coordinates</rdfs:label>
    </owl:ObjectProperty>
    


    <!-- http://www.dronetology.net/dronetology#decomposesTo -->

    <owl:ObjectProperty rdf:about="http://www.dronetology.net/dronetology#decomposesTo">
        <rdfs:domain rdf:resource="http://www.dronetology.net/dronetology#Function"/>
        <rdfs:range rdf:resource="http://www.dronetology.net/dronetology#Function"/>
        <rdfs:comment xml:lang="en">decomposesTo. Relates a high level function with its sub-functions.</rdfs:comment>
        <rdfs:label xml:lang="en">decomposesTo</rdfs:label>
    </owl:ObjectProperty>
    


    <!-- http://www.dronetology.net/dronetology#decompositionOf -->

    <owl:ObjectProperty rdf:about="http://www.dronetology.net/dronetology#decompositionOf">
        <rdfs:domain rdf:resource="http://www.dronetology.net/dronetology#Requirement"/>
        <rdfs:range rdf:resource="http://www.dronetology.net/dronetology#Requirement"/>
        <rdfs:comment xml:lang="en">decompositionOf. Relates sub-requirements with their ancestor requirement.</rdfs:comment>
        <rdfs:label xml:lang="en">decompositionOf</rdfs:label>
    </owl:ObjectProperty>
    


    <!-- http://www.dronetology.net/dronetology#derivedFrom -->

    <owl:ObjectProperty rdf:about="http://www.dronetology.net/dronetology#derivedFrom">
        <owl:inverseOf rdf:resource="http://www.dronetology.net/dronetology#derives"/>
        <rdfs:domain rdf:resource="http://www.dronetology.net/dronetology#Component"/>
        <rdfs:range rdf:resource="http://www.dronetology.net/dronetology#Component"/>
        <rdfs:comment xml:lang="en">derivedFrom. Relates a component with the initial component.</rdfs:comment>
        <rdfs:label xml:lang="en">derivedFrom</rdfs:label>
    </owl:ObjectProperty>
    


    <!-- http://www.dronetology.net/dronetology#derives -->

    <owl:ObjectProperty rdf:about="http://www.dronetology.net/dronetology#derives">
        <rdfs:domain rdf:resource="http://www.dronetology.net/dronetology#Component"/>
        <rdfs:range rdf:resource="http://www.dronetology.net/dronetology#Component"/>
        <rdfs:comment xml:lang="en">derives. Relates a component with a newer version.</rdfs:comment>
        <rdfs:label xml:lang="en">derives</rdfs:label>
    </owl:ObjectProperty>
    


    <!-- http://www.dronetology.net/dronetology#hasAPrioriRelationshipWith -->

    <owl:ObjectProperty rdf:about="http://www.dronetology.net/dronetology#hasAPrioriRelationshipWith">
        <rdfs:subPropertyOf rdf:resource="http://www.dronetology.net/dronetology#hasARelationshipWith"/>
        <rdfs:comment xml:lang="en">hasAPrioriRelationshipWith. Relates two drones when the relation is established before the mission.</rdfs:comment>
        <rdfs:label xml:lang="en">hasAPrioriRelationshipWith</rdfs:label>
    </owl:ObjectProperty>
    


    <!-- http://www.dronetology.net/dronetology#hasARelationshipWith -->

    <owl:ObjectProperty rdf:about="http://www.dronetology.net/dronetology#hasARelationshipWith">
        <owl:inverseOf rdf:resource="http://www.dronetology.net/dronetology#isRelationshipOf"/>
        <rdfs:domain rdf:resource="http://www.dronetology.net/dronetology#Drone"/>
        <rdfs:range rdf:resource="http://www.dronetology.net/dronetology#Drone"/>
        <rdfs:comment xml:lang="en">hasARelationShip</rdfs:comment>
        <rdfs:comment xml:lang="en">hasARelationShip. Relates drones with any kind or relationship between them.</rdfs:comment>
    </owl:ObjectProperty>
    


    <!-- http://www.dronetology.net/dronetology#hasComponent -->

    <owl:ObjectProperty rdf:about="http://www.dronetology.net/dronetology#hasComponent">
        <owl:inverseOf rdf:resource="http://www.dronetology.net/dronetology#isComponentOf"/>
        <rdfs:domain rdf:resource="http://www.dronetology.net/dronetology#Drone"/>
        <rdfs:range rdf:resource="http://www.dronetology.net/dronetology#Component"/>
        <rdfs:comment xml:lang="en">hasComponent. Relates components with the drone.</rdfs:comment>
        <rdfs:label xml:lang="en">hasComponent</rdfs:label>
    </owl:ObjectProperty>
    


    <!-- http://www.dronetology.net/dronetology#hasComprehension -->

    <owl:ObjectProperty rdf:about="http://www.dronetology.net/dronetology#hasComprehension">
        <owl:inverseOf rdf:resource="http://www.dronetology.net/dronetology#usedInComprehension"/>
        <rdfs:domain rdf:resource="http://www.dronetology.net/dronetology#SituationalAwareness"/>
        <rdfs:range rdf:resource="http://www.dronetology.net/dronetology#MissionElement"/>
        <rdfs:comment xml:lang="en">hasComprehension. Identifies any mission element that provides situational awareness at the level of comprehension.</rdfs:comment>
        <rdfs:label xml:lang="en">hasComprehension</rdfs:label>
    </owl:ObjectProperty>
    


    <!-- http://www.dronetology.net/dronetology#hasDirectPart -->

    <owl:ObjectProperty rdf:about="http://www.dronetology.net/dronetology#hasDirectPart">
        <rdfs:subPropertyOf rdf:resource="http://www.dronetology.net/dronetology#hasPart"/>
        <owl:inverseOf rdf:resource="http://www.dronetology.net/dronetology#isDirectPartOf"/>
        <rdfs:domain rdf:resource="http://www.dronetology.net/dronetology#Component"/>
        <rdfs:range rdf:resource="http://www.dronetology.net/dronetology#Component"/>
        <rdfs:comment xml:lang="en">hasDirectPart. Relates a part with its direct sub-part.</rdfs:comment>
        <rdfs:label xml:lang="en">hasDirectPart</rdfs:label>
    </owl:ObjectProperty>
    


    <!-- http://www.dronetology.net/dronetology#hasDrone -->

    <owl:ObjectProperty rdf:about="http://www.dronetology.net/dronetology#hasDrone">
        <owl:inverseOf rdf:resource="http://www.dronetology.net/dronetology#isDroneOf"/>
        <rdfs:domain rdf:resource="http://www.dronetology.net/dronetology#Swarm"/>
        <rdfs:range rdf:resource="http://www.dronetology.net/dronetology#Drone"/>
        <rdfs:comment xml:lang="en">hasDrone. Relates a swarm with a drone.</rdfs:comment>
        <rdfs:label xml:lang="en">hasDrone</rdfs:label>
    </owl:ObjectProperty>
    


    <!-- http://www.dronetology.net/dronetology#hasElement -->

    <owl:ObjectProperty rdf:about="http://www.dronetology.net/dronetology#hasElement">
        <owl:inverseOf rdf:resource="http://www.dronetology.net/dronetology#isElementOf"/>
        <rdfs:domain rdf:resource="http://www.dronetology.net/dronetology#Mission"/>
        <rdfs:range rdf:resource="http://www.dronetology.net/dronetology#MissionElement"/>
        <rdfs:comment xml:lang="en">hasElement. Relates a mission element with the mission</rdfs:comment>
        <rdfs:label xml:lang="en">hasElement</rdfs:label>
    </owl:ObjectProperty>
    


    <!-- http://www.dronetology.net/dronetology#hasExpression -->

    <owl:ObjectProperty rdf:about="http://www.dronetology.net/dronetology#hasExpression">
        <owl:inverseOf rdf:resource="http://www.dronetology.net/dronetology#isExpressionOf"/>
        <rdfs:domain rdf:resource="http://www.dronetology.net/dronetology#Requirement"/>
        <rdfs:range rdf:resource="http://www.dronetology.net/dronetology#Constraint"/>
        <rdfs:comment xml:lang="en">hasExpresion. Relates a requirement with a constraint.</rdfs:comment>
        <rdfs:label xml:lang="en">hasExpresion</rdfs:label>
    </owl:ObjectProperty>
    


    <!-- http://www.dronetology.net/dronetology#hasFeature -->

    <owl:ObjectProperty rdf:about="http://www.dronetology.net/dronetology#hasFeature">
        <owl:inverseOf rdf:resource="http://www.dronetology.net/dronetology#isFeatureOf"/>
        <rdfs:domain rdf:resource="http://www.dronetology.net/dronetology#Component"/>
        <rdfs:range rdf:resource="http://www.dronetology.net/dronetology#Feature"/>
        <rdfs:comment xml:lang="en">hasFeature. Relates a component with a feature.</rdfs:comment>
        <rdfs:label xml:lang="en">hasFeature</rdfs:label>
    </owl:ObjectProperty>
    


    <!-- http://www.dronetology.net/dronetology#hasFunction -->

    <owl:ObjectProperty rdf:about="http://www.dronetology.net/dronetology#hasFunction">
        <owl:inverseOf rdf:resource="http://www.dronetology.net/dronetology#isFunctionOf"/>
        <rdfs:domain rdf:resource="http://www.dronetology.net/dronetology#Component"/>
        <rdfs:range rdf:resource="http://www.dronetology.net/dronetology#Function"/>
        <rdfs:comment xml:lang="en">hasFunction. Relates a component with its function.</rdfs:comment>
        <rdfs:label xml:lang="en">hasFunction</rdfs:label>
    </owl:ObjectProperty>
    


    <!-- http://www.dronetology.net/dronetology#hasGeometry -->

    <owl:ObjectProperty rdf:about="http://www.dronetology.net/dronetology#hasGeometry">
        <rdfs:subPropertyOf rdf:resource="http://www.opengis.net/ont/geosparql#hasGeometry"/>
        <owl:inverseOf rdf:resource="http://www.dronetology.net/dronetology#isGeometryOf"/>
        <rdfs:domain>
            <owl:Class>
                <owl:unionOf rdf:parseType="Collection">
                    <rdf:Description rdf:about="http://www.dronetology.net/dronetology#MissionGeometryElement"/>
                    <rdf:Description rdf:about="http://www.dronetology.net/dronetology#MissionGeometryPointElement"/>
                </owl:unionOf>
            </owl:Class>
        </rdfs:domain>
        <rdfs:range rdf:resource="http://www.opengis.net/ont/geosparql#Geometry"/>
        <rdfs:comment xml:lang="en">hasGeometry. Relates a mission element with its geometry.</rdfs:comment>
        <rdfs:label xml:lang="en">hasGeometry</rdfs:label>
    </owl:ObjectProperty>
    


    <!-- http://www.dronetology.net/dronetology#hasHeight -->

    <owl:ObjectProperty rdf:about="http://www.dronetology.net/dronetology#hasHeight">
        <owl:inverseOf rdf:resource="http://www.dronetology.net/dronetology#isHeightOf"/>
        <rdfs:domain>
            <owl:Class>
                <owl:unionOf rdf:parseType="Collection">
                    <rdf:Description rdf:about="http://www.dronetology.net/dronetology#MissionGeometryElement"/>
                    <rdf:Description rdf:about="http://www.dronetology.net/dronetology#MissionGeometryPointElement"/>
                </owl:unionOf>
            </owl:Class>
        </rdfs:domain>
        <rdfs:range rdf:resource="http://www.dronetology.net/dronetology#Height"/>
        <rdfs:comment xml:lang="en">hasHeight. Relates mission elements with a height.</rdfs:comment>
        <rdfs:label xml:lang="en">hasHeight</rdfs:label>
    </owl:ObjectProperty>
    


    <!-- http://www.dronetology.net/dronetology#hasImpact -->

    <owl:ObjectProperty rdf:about="http://www.dronetology.net/dronetology#hasImpact">
        <owl:inverseOf rdf:resource="http://www.dronetology.net/dronetology#isImpactOf"/>
        <rdfs:domain rdf:resource="http://www.dronetology.net/dronetology#Risk"/>
        <rdfs:range rdf:resource="http://www.dronetology.net/dronetology#RiskImpact"/>
        <rdfs:comment xml:lang="en">hasImpact. Relates a risk with its impact.</rdfs:comment>
        <rdfs:label xml:lang="en">hasImpact</rdfs:label>
    </owl:ObjectProperty>
    


    <!-- http://www.dronetology.net/dronetology#hasLicence -->

    <owl:ObjectProperty rdf:about="http://www.dronetology.net/dronetology#hasLicence">
        <owl:inverseOf rdf:resource="http://www.dronetology.net/dronetology#isLicenceOf"/>
        <rdfs:domain rdf:resource="http://www.dronetology.net/dronetology#MissionPilot"/>
        <rdfs:range rdf:resource="http://www.dronetology.net/dronetology#PilotLicence"/>
        <rdfs:comment xml:lang="en">hasLicence. Relates a mission pilot with the legal licence to fly a drone.</rdfs:comment>
        <rdfs:label xml:lang="en">hasLicence</rdfs:label>
    </owl:ObjectProperty>
    


    <!-- http://www.dronetology.net/dronetology#hasLikelihood -->

    <owl:ObjectProperty rdf:about="http://www.dronetology.net/dronetology#hasLikelihood">
        <owl:inverseOf rdf:resource="http://www.dronetology.net/dronetology#isLikelihoodOf"/>
        <rdfs:domain rdf:resource="http://www.dronetology.net/dronetology#Risk"/>
        <rdfs:range rdf:resource="http://www.dronetology.net/dronetology#RiskLikelihood"/>
        <rdfs:comment xml:lang="en">hasLikelihood. Relates a risk wit its likelihood.</rdfs:comment>
        <rdfs:label xml:lang="en">hasLikelihood</rdfs:label>
    </owl:ObjectProperty>
    


    <!-- http://www.dronetology.net/dronetology#hasManufacturer -->

    <owl:ObjectProperty rdf:about="http://www.dronetology.net/dronetology#hasManufacturer">
        <rdfs:domain rdf:resource="http://www.dronetology.net/dronetology#Drone"/>
        <rdfs:range rdf:resource="http://www.dronetology.net/dronetology#Manufacturer"/>
        <rdfs:comment xml:lang="en">hasManufacturer. Relates a component with its manufacturer.</rdfs:comment>
        <rdfs:label xml:lang="en">hasManufacturer</rdfs:label>
    </owl:ObjectProperty>
    


    <!-- http://www.dronetology.net/dronetology#hasMass -->

    <owl:ObjectProperty rdf:about="http://www.dronetology.net/dronetology#hasMass">
        <owl:inverseOf rdf:resource="http://www.dronetology.net/dronetology#isMassOf"/>
        <rdfs:domain rdf:resource="http://www.dronetology.net/dronetology#Component"/>
        <rdfs:range rdf:resource="http://www.dronetology.net/dronetology#Mass"/>
        <rdfs:comment xml:lang="en">hasMass. Relates a component with its mass or weight.</rdfs:comment>
        <rdfs:label xml:lang="en">hasMass</rdfs:label>
    </owl:ObjectProperty>
    


    <!-- http://www.dronetology.net/dronetology#hasMission -->

    <owl:ObjectProperty rdf:about="http://www.dronetology.net/dronetology#hasMission">
        <owl:inverseOf rdf:resource="http://www.dronetology.net/dronetology#isMissionOf"/>
        <rdfs:domain rdf:resource="http://www.dronetology.net/dronetology#Drone"/>
        <rdfs:range rdf:resource="http://www.dronetology.net/dronetology#Mission"/>
        <rdfs:comment xml:lang="en">hasMission. Relates a drone with its missions</rdfs:comment>
        <rdfs:label xml:lang="en">hasMission</rdfs:label>
    </owl:ObjectProperty>
    


    <!-- http://www.dronetology.net/dronetology#hasMissionMode -->

    <owl:ObjectProperty rdf:about="http://www.dronetology.net/dronetology#hasMissionMode">
        <owl:inverseOf rdf:resource="http://www.dronetology.net/dronetology#isMissionModeOf"/>
        <rdfs:domain rdf:resource="http://www.dronetology.net/dronetology#Mission"/>
        <rdfs:range rdf:resource="http://www.dronetology.net/dronetology#MissionMode"/>
        <owl:propertyDisjointWith rdf:resource="http://www.dronetology.net/dronetology#isMissionModeOf"/>
        <rdfs:comment xml:lang="en">hasMissionMode. Relates a mission with the mission mode.</rdfs:comment>
        <rdfs:label xml:lang="en">hasMissionMode</rdfs:label>
    </owl:ObjectProperty>
    


    <!-- http://www.dronetology.net/dronetology#hasMissionPriority -->

    <owl:ObjectProperty rdf:about="http://www.dronetology.net/dronetology#hasMissionPriority">
        <owl:inverseOf rdf:resource="http://www.dronetology.net/dronetology#isMissionPriorityOf"/>
        <rdfs:domain rdf:resource="http://www.dronetology.net/dronetology#Mission"/>
        <rdfs:range rdf:resource="http://www.dronetology.net/dronetology#MissionPriority"/>
        <rdfs:comment xml:lang="en">hasMissionPriority. Relates a mission with its priority.</rdfs:comment>
        <rdfs:label xml:lang="en">hasMissionPriority</rdfs:label>
    </owl:ObjectProperty>
    


    <!-- http://www.dronetology.net/dronetology#hasMissionStatus -->

    <owl:ObjectProperty rdf:about="http://www.dronetology.net/dronetology#hasMissionStatus">
        <rdfs:domain rdf:resource="http://www.dronetology.net/dronetology#Mission"/>
        <rdfs:range rdf:resource="http://www.dronetology.net/dronetology#MissionStatus"/>
        <owl:propertyDisjointWith rdf:resource="http://www.dronetology.net/dronetology#isMissionStatusOf"/>
        <rdfs:comment xml:lang="en">hasMissionStatus. Relates a mission with its status</rdfs:comment>
        <rdfs:label xml:lang="en">hasMissionStatus</rdfs:label>
    </owl:ObjectProperty>
    


    <!-- http://www.dronetology.net/dronetology#hasNext -->

    <owl:ObjectProperty rdf:about="http://www.dronetology.net/dronetology#hasNext">
        <owl:inverseOf rdf:resource="http://www.dronetology.net/dronetology#hasPrevious"/>
        <rdfs:domain rdf:resource="http://www.dronetology.net/dronetology#Waypoint"/>
        <rdfs:range rdf:resource="http://www.dronetology.net/dronetology#Waypoint"/>
        <rdfs:comment xml:lang="en">hasNext. Relates a waypoint with the next one.</rdfs:comment>
        <rdfs:label xml:lang="en">hasNext</rdfs:label>
    </owl:ObjectProperty>
    


    <!-- http://www.dronetology.net/dronetology#hasObjective -->

    <owl:ObjectProperty rdf:about="http://www.dronetology.net/dronetology#hasObjective">
        <owl:inverseOf rdf:resource="http://www.dronetology.net/dronetology#isObjectiveOf"/>
        <rdfs:domain rdf:resource="http://www.dronetology.net/dronetology#Mission"/>
        <rdfs:range rdf:resource="http://www.dronetology.net/dronetology#MissionObjective"/>
        <rdfs:comment xml:lang="en">hasObjective. Relates a mission with its objective</rdfs:comment>
        <rdfs:label xml:lang="en">hasObjective</rdfs:label>
    </owl:ObjectProperty>
    


    <!-- http://www.dronetology.net/dronetology#hasParameter -->

    <owl:ObjectProperty rdf:about="http://www.dronetology.net/dronetology#hasParameter">
        <owl:inverseOf rdf:resource="http://www.dronetology.net/dronetology#isParameterOf"/>
        <rdfs:domain>
            <owl:Class>
                <owl:unionOf rdf:parseType="Collection">
                    <rdf:Description rdf:about="http://www.dronetology.net/dronetology#Component"/>
                    <rdf:Description rdf:about="http://www.dronetology.net/dronetology#Feature"/>
                </owl:unionOf>
            </owl:Class>
        </rdfs:domain>
        <rdfs:range rdf:resource="http://www.dronetology.net/dronetology#Parameter"/>
        <rdfs:comment xml:lang="en">hasParameter. Relates a component or a feature with a parameter.</rdfs:comment>
        <rdfs:label xml:lang="en">hasParameter</rdfs:label>
    </owl:ObjectProperty>
    


    <!-- http://www.dronetology.net/dronetology#hasParameterQuantity -->

    <owl:ObjectProperty rdf:about="http://www.dronetology.net/dronetology#hasParameterQuantity">
        <owl:inverseOf rdf:resource="http://www.dronetology.net/dronetology#isParameterQuantityOf"/>
        <rdfs:domain rdf:resource="http://www.dronetology.net/dronetology#Parameter"/>
        <rdfs:range rdf:resource="http://qudt.org/schema/qudt/Quantity"/>
        <rdfs:comment xml:lang="en">hasParameterQuantity. Relates a parameter with a quantity.</rdfs:comment>
        <rdfs:label xml:lang="en">hasParameterQuantity</rdfs:label>
    </owl:ObjectProperty>
    


    <!-- http://www.dronetology.net/dronetology#hasPart -->

    <owl:ObjectProperty rdf:about="http://www.dronetology.net/dronetology#hasPart">
        <owl:equivalentProperty rdf:resource="http://www.ontologydesignpatterns.org/ont/dul/DUL.owl#hasPart"/>
        <rdfs:subPropertyOf rdf:resource="http://www.ontologydesignpatterns.org/ont/dul/DUL.owl#hasPart"/>
        <owl:inverseOf rdf:resource="http://www.dronetology.net/dronetology#isPartOf"/>
        <rdf:type rdf:resource="http://www.w3.org/2002/07/owl#TransitiveProperty"/>
        <rdfs:domain rdf:resource="http://www.dronetology.net/dronetology#Component"/>
        <rdfs:range rdf:resource="http://www.dronetology.net/dronetology#Component"/>
        <rdfs:comment xml:lang="en">hasPart. Relates an element with its parts.</rdfs:comment>
        <rdfs:label xml:lang="en">hasPart</rdfs:label>
    </owl:ObjectProperty>
    


    <!-- http://www.dronetology.net/dronetology#hasPerception -->

    <owl:ObjectProperty rdf:about="http://www.dronetology.net/dronetology#hasPerception">
        <owl:inverseOf rdf:resource="http://www.dronetology.net/dronetology#usedInPerception"/>
        <rdfs:domain rdf:resource="http://www.dronetology.net/dronetology#SituationalAwareness"/>
        <rdfs:range rdf:resource="http://www.dronetology.net/dronetology#MissionElement"/>
        <rdfs:comment xml:lang="en">hasPerception. Relates a mission element with the perception layer of the situational awareness.</rdfs:comment>
        <rdfs:label xml:lang="en">hasPerception</rdfs:label>
    </owl:ObjectProperty>
    


    <!-- http://www.dronetology.net/dronetology#hasPilot -->

    <owl:ObjectProperty rdf:about="http://www.dronetology.net/dronetology#hasPilot">
        <rdfs:domain rdf:resource="http://www.dronetology.net/dronetology#Mission"/>
        <rdfs:range rdf:resource="http://www.dronetology.net/dronetology#Pilot"/>
        <rdfs:comment xml:lang="en">hasPilot. Relates a mission with a pilot.</rdfs:comment>
        <rdfs:label xml:lang="en">hasPilot</rdfs:label>
    </owl:ObjectProperty>
    


    <!-- http://www.dronetology.net/dronetology#hasPrevious -->

    <owl:ObjectProperty rdf:about="http://www.dronetology.net/dronetology#hasPrevious">
        <rdfs:domain rdf:resource="http://www.dronetology.net/dronetology#Waypoint"/>
        <rdfs:range rdf:resource="http://www.dronetology.net/dronetology#Waypoint"/>
        <rdfs:comment xml:lang="en">hasPrevious. Relates a waypoint with the previous one.</rdfs:comment>
        <rdfs:label xml:lang="en">hasPrevious</rdfs:label>
    </owl:ObjectProperty>
    


    <!-- http://www.dronetology.net/dronetology#hasProduct -->

    <owl:ObjectProperty rdf:about="http://www.dronetology.net/dronetology#hasProduct">
        <owl:inverseOf rdf:resource="http://www.dronetology.net/dronetology#isProductOf"/>
        <rdfs:domain rdf:resource="http://www.dronetology.net/dronetology#Drone"/>
        <rdfs:range rdf:resource="http://www.dronetology.net/dronetology#Product"/>
        <rdfs:comment xml:lang="en">hasProduct. Relates a drone with a product.</rdfs:comment>
        <rdfs:label xml:lang="en">hasProduct</rdfs:label>
    </owl:ObjectProperty>
    


    <!-- http://www.dronetology.net/dronetology#hasProjection -->

    <owl:ObjectProperty rdf:about="http://www.dronetology.net/dronetology#hasProjection">
        <owl:inverseOf rdf:resource="http://www.dronetology.net/dronetology#usedInProjection"/>
        <rdfs:domain rdf:resource="http://www.dronetology.net/dronetology#SituationalAwareness"/>
        <rdfs:range rdf:resource="http://www.dronetology.net/dronetology#MissionElement"/>
        <rdfs:comment xml:lang="en">hasProjection. Relates a mission element with the projection layer of the situational awareness.</rdfs:comment>
        <rdfs:label xml:lang="en">hasProjection</rdfs:label>
    </owl:ObjectProperty>
    


    <!-- http://www.dronetology.net/dronetology#hasQuantity -->

    <owl:ObjectProperty rdf:about="http://www.dronetology.net/dronetology#hasQuantity">
        <owl:inverseOf rdf:resource="http://www.dronetology.net/dronetology#isQuantityOf"/>
        <rdfs:domain rdf:resource="http://www.dronetology.net/dronetology#Regulation"/>
        <rdfs:range rdf:resource="http://qudt.org/schema/qudt/Quantity"/>
        <rdfs:comment xml:lang="en">hasQuantity. Relates a drone regulation with a quantity.</rdfs:comment>
        <rdfs:label xml:lang="en">hasQuantity</rdfs:label>
    </owl:ObjectProperty>
    


    <!-- http://www.dronetology.net/dronetology#hasSensedQuantity -->

    <owl:ObjectProperty rdf:about="http://www.dronetology.net/dronetology#hasSensedQuantity">
        <owl:inverseOf rdf:resource="http://www.dronetology.net/dronetology#isSensedQuantityOf"/>
        <rdfs:domain rdf:resource="http://www.dronetology.net/dronetology#MissionSensorData"/>
        <rdfs:range rdf:resource="http://qudt.org/schema/qudt/Quantity"/>
        <rdfs:comment xml:lang="en">hasSensedQuantity. Relates data obtained from a sensor during a mission with a quantity.</rdfs:comment>
        <rdfs:label xml:lang="en">hasSensedQuantity</rdfs:label>
    </owl:ObjectProperty>
    


    <!-- http://www.dronetology.net/dronetology#hasSensor -->

    <owl:ObjectProperty rdf:about="http://www.dronetology.net/dronetology#hasSensor">
        <owl:inverseOf rdf:resource="http://www.dronetology.net/dronetology#isSensorOf"/>
        <rdfs:domain rdf:resource="http://www.dronetology.net/dronetology#MissionSensorData"/>
        <rdfs:range rdf:resource="http://www.w3.org/ns/sosa#Sensor"/>
        <rdfs:comment xml:lang="en">hasSensor. Relates data obtained from a sensor and the sensor.</rdfs:comment>
        <rdfs:label xml:lang="en">hasSensor</rdfs:label>
    </owl:ObjectProperty>
    


    <!-- http://www.dronetology.net/dronetology#hasTelemetryQuantity -->

    <owl:ObjectProperty rdf:about="http://www.dronetology.net/dronetology#hasTelemetryQuantity">
        <owl:inverseOf rdf:resource="http://www.dronetology.net/dronetology#isTelemetryQuantityOf"/>
        <rdfs:domain rdf:resource="http://www.dronetology.net/dronetology#Telemetry"/>
        <rdfs:range rdf:resource="http://qudt.org/schema/qudt/Quantity"/>
        <rdfs:comment xml:lang="en">hasTelemetryQuantity. Relates the drone telemetry with a quantity.</rdfs:comment>
        <rdfs:label xml:lang="en">hasTelemetryQuantity</rdfs:label>
    </owl:ObjectProperty>
    


    <!-- http://www.dronetology.net/dronetology#hasTimeInterval -->

    <owl:ObjectProperty rdf:about="http://www.dronetology.net/dronetology#hasTimeInterval">
        <owl:inverseOf rdf:resource="http://www.dronetology.net/dronetology#isTimeIntervalOf"/>
        <rdfs:domain rdf:resource="http://www.dronetology.net/dronetology#MissionTemporalElement"/>
        <rdfs:range rdf:resource="http://www.w3.org/2006/time#TemporalEntity"/>
        <rdfs:comment xml:lang="en">hasTimeInterval. Relates mission elements that depends on time with a temporal entity.</rdfs:comment>
        <rdfs:label xml:lang="en">hasTimeInterval</rdfs:label>
    </owl:ObjectProperty>
    


    <!-- http://www.dronetology.net/dronetology#hasWaypoint -->

    <owl:ObjectProperty rdf:about="http://www.dronetology.net/dronetology#hasWaypoint">
        <owl:inverseOf rdf:resource="http://www.dronetology.net/dronetology#isWaypointOf"/>
        <rdfs:domain>
            <owl:Class>
                <owl:unionOf rdf:parseType="Collection">
                    <rdf:Description rdf:about="http://www.dronetology.net/dronetology#FlightPlan"/>
                    <rdf:Description rdf:about="http://www.dronetology.net/dronetology#FlightSegments"/>
                </owl:unionOf>
            </owl:Class>
        </rdfs:domain>
        <rdfs:range rdf:resource="http://www.dronetology.net/dronetology#Waypoint"/>
        <rdfs:comment xml:lang="en">hasWaypoint. Relates a fligh plan or a fligh segment with a waypoint.</rdfs:comment>
        <rdfs:label xml:lang="en">hasWaypoint</rdfs:label>
    </owl:ObjectProperty>
    


    <!-- http://www.dronetology.net/dronetology#hasWeatherParameter -->

    <owl:ObjectProperty rdf:about="http://www.dronetology.net/dronetology#hasWeatherParameter">
        <owl:inverseOf rdf:resource="http://www.dronetology.net/dronetology#isWeatherParameterOf"/>
        <rdfs:domain rdf:resource="http://www.dronetology.net/dronetology#MissionWeatherReport"/>
        <rdfs:range rdf:resource="http://qudt.org/schema/qudt/Quantity"/>
        <rdfs:comment xml:lang="en">hasWeatherParameter, Relates a weather report with a parameter.</rdfs:comment>
        <rdfs:label xml:lang="en">hasWeatherParameter</rdfs:label>
    </owl:ObjectProperty>
    


    <!-- http://www.dronetology.net/dronetology#installedAt -->

    <owl:ObjectProperty rdf:about="http://www.dronetology.net/dronetology#installedAt">
        <owl:inverseOf rdf:resource="http://www.dronetology.net/dronetology#instantOfInstallation"/>
        <rdfs:domain rdf:resource="http://www.dronetology.net/dronetology#Component"/>
        <rdfs:range rdf:resource="http://www.w3.org/2006/time#Instant"/>
        <rdfs:comment xml:lang="en">installedAt. Relates a time instant and a component, i.e. when the component was installed.</rdfs:comment>
        <rdfs:label xml:lang="en">installedAt</rdfs:label>
    </owl:ObjectProperty>
    


    <!-- http://www.dronetology.net/dronetology#instantOfInstallation -->

    <owl:ObjectProperty rdf:about="http://www.dronetology.net/dronetology#instantOfInstallation">
        <rdfs:domain rdf:resource="http://www.w3.org/2006/time#Instant"/>
        <rdfs:range rdf:resource="http://www.dronetology.net/dronetology#Component"/>
        <rdfs:comment xml:lang="en">instantOfInstallation. Relates the instant of the instalation with the component installed.</rdfs:comment>
        <rdfs:label xml:lang="en">instantOfInstallation</rdfs:label>
    </owl:ObjectProperty>
    


    <!-- http://www.dronetology.net/dronetology#isAMissionElementRelatedWith -->

    <owl:ObjectProperty rdf:about="http://www.dronetology.net/dronetology#isAMissionElementRelatedWith">
        <owl:inverseOf rdf:resource="http://www.dronetology.net/dronetology#relatedWithAMissionElement"/>
        <rdfs:domain rdf:resource="http://www.dronetology.net/dronetology#MissionElement"/>
        <rdfs:range rdf:resource="http://www.w3.org/2002/07/owl#Thing"/>
        <rdfs:comment xml:lang="en">isAMissionElementRelatedWith. Relates generically any instance of any type with a mission element.</rdfs:comment>
        <rdfs:label xml:lang="en">isAMissionElementRelatedWith</rdfs:label>
    </owl:ObjectProperty>
    


    <!-- http://www.dronetology.net/dronetology#isActivatedBy -->

    <owl:ObjectProperty rdf:about="http://www.dronetology.net/dronetology#isActivatedBy">
        <rdfs:domain rdf:resource="http://www.dronetology.net/dronetology#Alarm"/>
        <rdfs:range rdf:resource="http://www.dronetology.net/dronetology#CommunicationMessage"/>
        <rdfs:comment xml:lang="en">isActivatedBy. Relates an alarm with a communication message.</rdfs:comment>
        <rdfs:label xml:lang="en">isActivatedBy</rdfs:label>
    </owl:ObjectProperty>
    


    <!-- http://www.dronetology.net/dronetology#isComponentOf -->

    <owl:ObjectProperty rdf:about="http://www.dronetology.net/dronetology#isComponentOf">
        <rdfs:domain rdf:resource="http://www.dronetology.net/dronetology#Component"/>
        <rdfs:range rdf:resource="http://www.dronetology.net/dronetology#Drone"/>
        <rdfs:comment xml:lang="en">isComponentOf. Relates a component with the drone.</rdfs:comment>
        <rdfs:label xml:lang="en">isComponentOf</rdfs:label>
    </owl:ObjectProperty>
    


    <!-- http://www.dronetology.net/dronetology#isDirectPartOf -->

    <owl:ObjectProperty rdf:about="http://www.dronetology.net/dronetology#isDirectPartOf">
        <rdfs:subPropertyOf rdf:resource="http://www.dronetology.net/dronetology#isPartOf"/>
        <rdfs:domain rdf:resource="http://www.dronetology.net/dronetology#Component"/>
        <rdfs:range rdf:resource="http://www.dronetology.net/dronetology#Component"/>
        <rdfs:comment xml:lang="en">isDirectPart. Relates a part and its direct ancestor part.</rdfs:comment>
    </owl:ObjectProperty>
    


    <!-- http://www.dronetology.net/dronetology#isDroneOf -->

    <owl:ObjectProperty rdf:about="http://www.dronetology.net/dronetology#isDroneOf">
        <rdfs:domain rdf:resource="http://www.dronetology.net/dronetology#Drone"/>
        <rdfs:range rdf:resource="http://www.dronetology.net/dronetology#Swarm"/>
        <rdfs:comment xml:lang="en">isDroneOf. Relates a drone with a swarm.</rdfs:comment>
        <rdfs:label xml:lang="en">isDroneOf</rdfs:label>
    </owl:ObjectProperty>
    


    <!-- http://www.dronetology.net/dronetology#isElementOf -->

    <owl:ObjectProperty rdf:about="http://www.dronetology.net/dronetology#isElementOf">
        <rdfs:domain rdf:resource="http://www.dronetology.net/dronetology#MissionElement"/>
        <rdfs:range rdf:resource="http://www.dronetology.net/dronetology#Mission"/>
        <rdfs:comment xml:lang="en">isElementOf. Relates a mission element with a mission.</rdfs:comment>
        <rdfs:label xml:lang="en">isElementOf</rdfs:label>
    </owl:ObjectProperty>
    


    <!-- http://www.dronetology.net/dronetology#isExpressionOf -->

    <owl:ObjectProperty rdf:about="http://www.dronetology.net/dronetology#isExpressionOf">
        <rdfs:domain rdf:resource="http://www.dronetology.net/dronetology#Constraint"/>
        <rdfs:range rdf:resource="http://www.dronetology.net/dronetology#Requirement"/>
        <rdfs:comment xml:lang="en">isExpressionOf. Relates a constraint wit a requirement.</rdfs:comment>
        <rdfs:label xml:lang="en">isExpressionOf</rdfs:label>
    </owl:ObjectProperty>
    


    <!-- http://www.dronetology.net/dronetology#isFeatureOf -->

    <owl:ObjectProperty rdf:about="http://www.dronetology.net/dronetology#isFeatureOf">
        <rdfs:domain rdf:resource="http://www.dronetology.net/dronetology#Feature"/>
        <rdfs:range rdf:resource="http://www.dronetology.net/dronetology#Component"/>
        <rdfs:comment xml:lang="en">isFeatureOf. Relates a feature with the component.</rdfs:comment>
        <rdfs:label xml:lang="en">isFeatureOf</rdfs:label>
    </owl:ObjectProperty>
    


    <!-- http://www.dronetology.net/dronetology#isFulfilledBy -->

    <owl:ObjectProperty rdf:about="http://www.dronetology.net/dronetology#isFulfilledBy">
        <rdfs:domain rdf:resource="http://www.dronetology.net/dronetology#Regulation"/>
        <rdfs:range rdf:resource="http://www.dronetology.net/dronetology#Drone"/>
        <rdfs:comment xml:lang="en">isFulfilledBy. Relates a regulation with every drone that complies with.</rdfs:comment>
        <rdfs:label xml:lang="en">isFulfilledBy</rdfs:label>
    </owl:ObjectProperty>
    


    <!-- http://www.dronetology.net/dronetology#isFunctionOf -->

    <owl:ObjectProperty rdf:about="http://www.dronetology.net/dronetology#isFunctionOf">
        <rdfs:domain rdf:resource="http://www.dronetology.net/dronetology#Function"/>
        <rdfs:range rdf:resource="http://www.dronetology.net/dronetology#Component"/>
        <rdfs:comment xml:lang="en">isFunctionOf. Relates a function with a component.</rdfs:comment>
        <rdfs:label xml:lang="en">isFunctionOf</rdfs:label>
    </owl:ObjectProperty>
    


    <!-- http://www.dronetology.net/dronetology#isGeometryOf -->

    <owl:ObjectProperty rdf:about="http://www.dronetology.net/dronetology#isGeometryOf">
        <owl:inverseOf rdf:resource="http://www.opengis.net/ont/geosparql#hasGeometry"/>
        <rdfs:domain rdf:resource="http://www.opengis.net/ont/geosparql#Geometry"/>
        <rdfs:range>
            <owl:Class>
                <owl:unionOf rdf:parseType="Collection">
                    <rdf:Description rdf:about="http://www.dronetology.net/dronetology#MissionGeometryElement"/>
                    <rdf:Description rdf:about="http://www.dronetology.net/dronetology#MissionGeometryPointElement"/>
                </owl:unionOf>
            </owl:Class>
        </rdfs:range>
        <rdfs:comment xml:lang="en">isGeometryOf. Relates a geometry with a mission element with features.</rdfs:comment>
        <rdfs:label xml:lang="en">isGeometryOf</rdfs:label>
    </owl:ObjectProperty>
    


    <!-- http://www.dronetology.net/dronetology#isHeightOf -->

    <owl:ObjectProperty rdf:about="http://www.dronetology.net/dronetology#isHeightOf">
        <rdfs:domain rdf:resource="http://www.dronetology.net/dronetology#Height"/>
        <rdfs:range>
            <owl:Class>
                <owl:unionOf rdf:parseType="Collection">
                    <rdf:Description rdf:about="http://www.dronetology.net/dronetology#MissionGeometryElement"/>
                    <rdf:Description rdf:about="http://www.dronetology.net/dronetology#MissionGeometryPointElement"/>
                </owl:unionOf>
            </owl:Class>
        </rdfs:range>
        <rdfs:comment xml:lang="en">isHeightOf. Relates a height with a mission element with geometry</rdfs:comment>
        <rdfs:label xml:lang="en">isHeightOf</rdfs:label>
    </owl:ObjectProperty>
    


    <!-- http://www.dronetology.net/dronetology#isImpactOf -->

    <owl:ObjectProperty rdf:about="http://www.dronetology.net/dronetology#isImpactOf">
        <rdfs:domain rdf:resource="http://www.dronetology.net/dronetology#RiskImpact"/>
        <rdfs:range rdf:resource="http://www.dronetology.net/dronetology#Risk"/>
        <rdfs:comment xml:lang="en">isImpactOf. Relates a risk impact with the risk.</rdfs:comment>
        <rdfs:label xml:lang="en">isImpactOf</rdfs:label>
    </owl:ObjectProperty>
    


    <!-- http://www.dronetology.net/dronetology#isLicenceOf -->

    <owl:ObjectProperty rdf:about="http://www.dronetology.net/dronetology#isLicenceOf">
        <rdfs:domain rdf:resource="http://www.dronetology.net/dronetology#PilotLicence"/>
        <rdfs:range rdf:resource="http://www.dronetology.net/dronetology#MissionPilot"/>
        <rdfs:comment xml:lang="en">isLicenceOf. Relates a licence for drone flying with a mission pilot.</rdfs:comment>
        <rdfs:label xml:lang="en">isLicenceOf</rdfs:label>
    </owl:ObjectProperty>
    


    <!-- http://www.dronetology.net/dronetology#isLikelihoodOf -->

    <owl:ObjectProperty rdf:about="http://www.dronetology.net/dronetology#isLikelihoodOf">
        <rdfs:domain rdf:resource="http://www.dronetology.net/dronetology#RiskLikelihood"/>
        <rdfs:range rdf:resource="http://www.dronetology.net/dronetology#Risk"/>
        <rdfs:comment xml:lang="en">isLikelihood. Relates a likelihood with the risk,</rdfs:comment>
        <rdfs:label xml:lang="en">isLikelihood</rdfs:label>
    </owl:ObjectProperty>
    


    <!-- http://www.dronetology.net/dronetology#isMassOf -->

    <owl:ObjectProperty rdf:about="http://www.dronetology.net/dronetology#isMassOf">
        <rdfs:domain rdf:resource="http://www.dronetology.net/dronetology#Mass"/>
        <rdfs:range rdf:resource="http://www.dronetology.net/dronetology#Component"/>
        <rdfs:comment xml:lang="en">isMassOf. Relates a mass with the component.</rdfs:comment>
        <rdfs:label xml:lang="en">isMassOf</rdfs:label>
    </owl:ObjectProperty>
    


    <!-- http://www.dronetology.net/dronetology#isMissionModeOf -->

    <owl:ObjectProperty rdf:about="http://www.dronetology.net/dronetology#isMissionModeOf">
        <rdfs:domain rdf:resource="http://www.dronetology.net/dronetology#MissionMode"/>
        <rdfs:range rdf:resource="http://www.dronetology.net/dronetology#Mission"/>
        <rdfs:comment xml:lang="en">isMissionModeOf. Relates a mode with the mission</rdfs:comment>
        <rdfs:label xml:lang="en">isMissionModeOf</rdfs:label>
    </owl:ObjectProperty>
    


    <!-- http://www.dronetology.net/dronetology#isMissionOf -->

    <owl:ObjectProperty rdf:about="http://www.dronetology.net/dronetology#isMissionOf">
        <rdfs:domain rdf:resource="http://www.dronetology.net/dronetology#Mission"/>
        <rdfs:range rdf:resource="http://www.dronetology.net/dronetology#Drone"/>
        <rdfs:comment xml:lang="en">isMissionOf. Relates a mission with the drone.</rdfs:comment>
        <rdfs:label xml:lang="en">isMissionOf</rdfs:label>
    </owl:ObjectProperty>
    


    <!-- http://www.dronetology.net/dronetology#isMissionPriorityOf -->

    <owl:ObjectProperty rdf:about="http://www.dronetology.net/dronetology#isMissionPriorityOf">
        <rdfs:domain rdf:resource="http://www.dronetology.net/dronetology#MissionPriority"/>
        <rdfs:range rdf:resource="http://www.dronetology.net/dronetology#Mission"/>
        <rdfs:comment xml:lang="en">isMissionPriorityOf. Relates a priority with the mission.</rdfs:comment>
        <rdfs:label xml:lang="en">isMissionPriorityOf</rdfs:label>
    </owl:ObjectProperty>
    


    <!-- http://www.dronetology.net/dronetology#isMissionStatusOf -->

    <owl:ObjectProperty rdf:about="http://www.dronetology.net/dronetology#isMissionStatusOf">
        <rdfs:domain rdf:resource="http://www.dronetology.net/dronetology#MissionStatus"/>
        <rdfs:range rdf:resource="http://www.dronetology.net/dronetology#Mission"/>
        <rdfs:comment xml:lang="en">isMissionStatusOf. Relates a mission status with the mission.</rdfs:comment>
        <rdfs:label xml:lang="en">isMissionStatusOf</rdfs:label>
    </owl:ObjectProperty>
    


    <!-- http://www.dronetology.net/dronetology#isObjectiveOf -->

    <owl:ObjectProperty rdf:about="http://www.dronetology.net/dronetology#isObjectiveOf">
        <rdfs:domain rdf:resource="http://www.dronetology.net/dronetology#MissionObjective"/>
        <rdfs:range rdf:resource="http://www.dronetology.net/dronetology#Mission"/>
        <rdfs:comment xml:lang="en">isObjectiveOf. Relates a mission objective with the mission.</rdfs:comment>
        <rdfs:label xml:lang="en">isObjectiveOf</rdfs:label>
    </owl:ObjectProperty>
    


    <!-- http://www.dronetology.net/dronetology#isParameterOf -->

    <owl:ObjectProperty rdf:about="http://www.dronetology.net/dronetology#isParameterOf">
        <rdfs:domain rdf:resource="http://www.dronetology.net/dronetology#Parameter"/>
        <rdfs:range>
            <owl:Class>
                <owl:unionOf rdf:parseType="Collection">
                    <rdf:Description rdf:about="http://www.dronetology.net/dronetology#Component"/>
                    <rdf:Description rdf:about="http://www.opengis.net/ont/geosparql#Feature"/>
                </owl:unionOf>
            </owl:Class>
        </rdfs:range>
        <rdfs:comment xml:lang="en">isParameterOf. Relates a parameter with a component or feature.</rdfs:comment>
        <rdfs:label xml:lang="en">isParameterOf</rdfs:label>
    </owl:ObjectProperty>
    


    <!-- http://www.dronetology.net/dronetology#isParameterQuantityOf -->

    <owl:ObjectProperty rdf:about="http://www.dronetology.net/dronetology#isParameterQuantityOf">
        <rdfs:domain rdf:resource="http://qudt.org/schema/qudt/Quantity"/>
        <rdfs:range rdf:resource="http://www.dronetology.net/dronetology#Parameter"/>
        <rdfs:comment xml:lang="en">isParameterQuantityOf. Relates a quantity with a parameter</rdfs:comment>
        <rdfs:label xml:lang="en">isParameterQuantityOf</rdfs:label>
    </owl:ObjectProperty>
    


    <!-- http://www.dronetology.net/dronetology#isPartOf -->

    <owl:ObjectProperty rdf:about="http://www.dronetology.net/dronetology#isPartOf">
        <rdf:type rdf:resource="http://www.w3.org/2002/07/owl#TransitiveProperty"/>
        <rdfs:domain rdf:resource="http://www.dronetology.net/dronetology#Component"/>
        <rdfs:range rdf:resource="http://www.dronetology.net/dronetology#Component"/>
        <rdfs:comment xml:lang="en">isPartOf. Relates a part and its ancestor part.</rdfs:comment>
        <rdfs:label xml:lang="en">isPartOf</rdfs:label>
    </owl:ObjectProperty>
    


    <!-- http://www.dronetology.net/dronetology#isPilotOf -->

    <owl:ObjectProperty rdf:about="http://www.dronetology.net/dronetology#isPilotOf">
        <rdfs:domain rdf:resource="http://www.dronetology.net/dronetology#Pilot"/>
        <rdfs:range rdf:resource="http://www.dronetology.net/dronetology#Mission"/>
        <rdfs:comment xml:lang="en">isPilotOf. Relates a pilot with a mission</rdfs:comment>
        <rdfs:label xml:lang="en">isPilotOf</rdfs:label>
    </owl:ObjectProperty>
    


    <!-- http://www.dronetology.net/dronetology#isProductOf -->

    <owl:ObjectProperty rdf:about="http://www.dronetology.net/dronetology#isProductOf">
        <rdfs:domain rdf:resource="http://www.dronetology.net/dronetology#Product"/>
        <rdfs:range rdf:resource="http://www.dronetology.net/dronetology#Drone"/>
        <rdfs:comment xml:lang="en">isProductOf. Relates a product with the drone.</rdfs:comment>
        <rdfs:label xml:lang="en">isProductOf</rdfs:label>
    </owl:ObjectProperty>
    


    <!-- http://www.dronetology.net/dronetology#isQuantityOf -->

    <owl:ObjectProperty rdf:about="http://www.dronetology.net/dronetology#isQuantityOf">
        <rdfs:domain rdf:resource="http://qudt.org/schema/qudt/Quantity"/>
        <rdfs:range rdf:resource="http://www.dronetology.net/dronetology#Regulation"/>
        <rdfs:comment xml:lang="en">isQuantityOf. Relates a quantity with a drone regulation.</rdfs:comment>
        <rdfs:label xml:lang="en">isQuantityOf</rdfs:label>
    </owl:ObjectProperty>
    


    <!-- http://www.dronetology.net/dronetology#isRelatedWithMission -->

    <owl:ObjectProperty rdf:about="http://www.dronetology.net/dronetology#isRelatedWithMission">
        <owl:inverseOf rdf:resource="http://www.dronetology.net/dronetology#relatedWithAMission"/>
        <rdfs:domain rdf:resource="http://www.dronetology.net/dronetology#Mission"/>
        <rdfs:range rdf:resource="http://www.w3.org/2002/07/owl#Thing"/>
        <rdfs:comment xml:lang="en">isRelatedWithMission. Relates a mission with any instance of any type.</rdfs:comment>
        <rdfs:label xml:lang="en">isRelatedWithMission</rdfs:label>
    </owl:ObjectProperty>
    


    <!-- http://www.dronetology.net/dronetology#isRelationshipOf -->

    <owl:ObjectProperty rdf:about="http://www.dronetology.net/dronetology#isRelationshipOf">
        <rdfs:domain rdf:resource="http://www.dronetology.net/dronetology#Drone"/>
        <rdfs:range rdf:resource="http://www.dronetology.net/dronetology#Drone"/>
        <rdfs:comment xml:lang="en">isRelationshipOf. Relates a drone with another.</rdfs:comment>
        <rdfs:label xml:lang="en">isRelationshipOf</rdfs:label>
    </owl:ObjectProperty>
    


    <!-- http://www.dronetology.net/dronetology#isReqSatisfiedBy -->

    <owl:ObjectProperty rdf:about="http://www.dronetology.net/dronetology#isReqSatisfiedBy">
        <owl:inverseOf rdf:resource="http://www.dronetology.net/dronetology#satisfiesReq"/>
        <rdfs:domain rdf:resource="http://www.dronetology.net/dronetology#Requirement"/>
        <rdfs:range rdf:resource="http://www.dronetology.net/dronetology#Component"/>
        <rdfs:comment xml:lang="en">isReqSatisfiedBy. Relates a requirement with a component.</rdfs:comment>
        <rdfs:label xml:lang="en">isReqSatisfiedBy</rdfs:label>
    </owl:ObjectProperty>
    


    <!-- http://www.dronetology.net/dronetology#isSensedQuantityOf -->

    <owl:ObjectProperty rdf:about="http://www.dronetology.net/dronetology#isSensedQuantityOf">
        <rdfs:domain rdf:resource="http://qudt.org/schema/qudt/Quantity"/>
        <rdfs:range rdf:resource="http://www.dronetology.net/dronetology#MissionSensorData"/>
        <rdfs:comment xml:lang="en">isSensedQuantityOf. Relates a quantity with the sensor that provided the measurement.</rdfs:comment>
        <rdfs:label xml:lang="en">isSensedQuantityOf</rdfs:label>
    </owl:ObjectProperty>
    


    <!-- http://www.dronetology.net/dronetology#isSensorOf -->

    <owl:ObjectProperty rdf:about="http://www.dronetology.net/dronetology#isSensorOf">
        <rdfs:domain rdf:resource="http://www.w3.org/ns/sosa#Sensor"/>
        <rdfs:range rdf:resource="http://www.dronetology.net/dronetology#MissionSensorData"/>
        <rdfs:comment xml:lang="en">isSensorOf. Relates a sensor with the data measured during a mission.</rdfs:comment>
        <rdfs:label xml:lang="en">isSensorOf</rdfs:label>
    </owl:ObjectProperty>
    


    <!-- http://www.dronetology.net/dronetology#isStoredIn -->

    <owl:ObjectProperty rdf:about="http://www.dronetology.net/dronetology#isStoredIn">
        <owl:inverseOf rdf:resource="http://www.dronetology.net/dronetology#stores"/>
        <rdfs:domain>
            <owl:Class>
                <owl:unionOf rdf:parseType="Collection">
                    <rdf:Description rdf:about="http://www.dronetology.net/dronetology#Photograph"/>
                    <rdf:Description rdf:about="http://www.dronetology.net/dronetology#Video"/>
                </owl:unionOf>
            </owl:Class>
        </rdfs:domain>
        <rdfs:range rdf:resource="http://www.dronetology.net/dronetology#DataStorageDevice"/>
        <rdfs:comment xml:lang="en">isStoredIn. Relates a digital content like a photograph or video with a data storage device.</rdfs:comment>
        <rdfs:label xml:lang="en">isStoredIn</rdfs:label>
    </owl:ObjectProperty>
    


    <!-- http://www.dronetology.net/dronetology#isTelemetryQuantityOf -->

    <owl:ObjectProperty rdf:about="http://www.dronetology.net/dronetology#isTelemetryQuantityOf">
        <rdfs:domain rdf:resource="http://qudt.org/schema/qudt/Quantity"/>
        <rdfs:range rdf:resource="http://www.dronetology.net/dronetology#Telemetry"/>
        <rdfs:comment xml:lang="en">isTelemetryQuantityOf. Relates a quantity with the telemetry.</rdfs:comment>
        <rdfs:label xml:lang="en">isTelemetryQuantityOf</rdfs:label>
    </owl:ObjectProperty>
    


    <!-- http://www.dronetology.net/dronetology#isTimeIntervalOf -->

    <owl:ObjectProperty rdf:about="http://www.dronetology.net/dronetology#isTimeIntervalOf">
        <rdfs:subPropertyOf rdf:resource="http://www.w3.org/2002/07/owl#topObjectProperty"/>
        <rdfs:domain rdf:resource="http://www.w3.org/2006/time#TemporalEntity"/>
        <rdfs:range rdf:resource="http://www.dronetology.net/dronetology#MissionTemporalElement"/>
        <rdfs:comment xml:lang="en">isTimeIntervalOf. Relates a temporal entity with a mission element that varies during the mission execution.</rdfs:comment>
        <rdfs:label xml:lang="en">isTimeIntervalOf</rdfs:label>
    </owl:ObjectProperty>
    


    <!-- http://www.dronetology.net/dronetology#isUnitOf -->

    <owl:ObjectProperty rdf:about="http://www.dronetology.net/dronetology#isUnitOf">
        <rdfs:domain rdf:resource="http://qudt.org/schema/qudt/Unit"/>
        <rdfs:range rdf:resource="http://qudt.org/schema/qudt/Quantity"/>
    </owl:ObjectProperty>
    


    <!-- http://www.dronetology.net/dronetology#isWaypointOf -->

    <owl:ObjectProperty rdf:about="http://www.dronetology.net/dronetology#isWaypointOf">
        <rdfs:domain rdf:resource="http://www.dronetology.net/dronetology#Waypoint"/>
        <rdfs:range>
            <owl:Class>
                <owl:unionOf rdf:parseType="Collection">
                    <rdf:Description rdf:about="http://www.dronetology.net/dronetology#FlightPlan"/>
                    <rdf:Description rdf:about="http://www.dronetology.net/dronetology#FlightSegments"/>
                </owl:unionOf>
            </owl:Class>
        </rdfs:range>
        <rdfs:comment xml:lang="en">isWaypointOf. Relates a waypoint with a flight plan.</rdfs:comment>
        <rdfs:label xml:lang="en">isWaypointOf</rdfs:label>
    </owl:ObjectProperty>
    


    <!-- http://www.dronetology.net/dronetology#isWeatherParameterOf -->

    <owl:ObjectProperty rdf:about="http://www.dronetology.net/dronetology#isWeatherParameterOf">
        <rdfs:domain rdf:resource="http://qudt.org/schema/qudt/Quantity"/>
        <rdfs:range rdf:resource="http://www.dronetology.net/dronetology#MissionWeatherReport"/>
        <rdfs:comment xml:lang="en">isWeatherParameterOf. Relates a quantity with a weather report.</rdfs:comment>
        <rdfs:label xml:lang="en">isWeatherParameterOf</rdfs:label>
    </owl:ObjectProperty>
    


    <!-- http://www.dronetology.net/dronetology#relatedWithAMission -->

    <owl:ObjectProperty rdf:about="http://www.dronetology.net/dronetology#relatedWithAMission">
        <rdfs:domain rdf:resource="http://www.w3.org/2002/07/owl#Thing"/>
        <rdfs:range rdf:resource="http://www.dronetology.net/dronetology#Mission"/>
        <rdfs:comment xml:lang="en">relatedWithAMission. Relates any instance of any class with a drone mission.</rdfs:comment>
        <rdfs:label xml:lang="en">relatedWithAMission</rdfs:label>
    </owl:ObjectProperty>
    


    <!-- http://www.dronetology.net/dronetology#relatedWithAMissionElement -->

    <owl:ObjectProperty rdf:about="http://www.dronetology.net/dronetology#relatedWithAMissionElement">
        <rdfs:domain rdf:resource="http://www.w3.org/2002/07/owl#Thing"/>
        <rdfs:range rdf:resource="http://www.dronetology.net/dronetology#MissionElement"/>
        <rdfs:comment xml:lang="en">relatedWithAMissionElement. Relates any instance of any class with a mission element.</rdfs:comment>
        <rdfs:label xml:lang="en">relatedWithAMissionElement</rdfs:label>
    </owl:ObjectProperty>
    


    <!-- http://www.dronetology.net/dronetology#replacedBy -->

    <owl:ObjectProperty rdf:about="http://www.dronetology.net/dronetology#replacedBy">
        <owl:inverseOf rdf:resource="http://www.dronetology.net/dronetology#replaces"/>
        <rdfs:domain rdf:resource="http://www.dronetology.net/dronetology#Component"/>
        <rdfs:range rdf:resource="http://www.dronetology.net/dronetology#Component"/>
        <rdfs:comment xml:lang="en">replacedBy. Relates a component with another after a replacement after a required maintenance task.</rdfs:comment>
        <rdfs:label xml:lang="en">replacedBy</rdfs:label>
    </owl:ObjectProperty>
    


    <!-- http://www.dronetology.net/dronetology#replaces -->

    <owl:ObjectProperty rdf:about="http://www.dronetology.net/dronetology#replaces">
        <rdfs:domain rdf:resource="http://www.dronetology.net/dronetology#Component"/>
        <rdfs:range rdf:resource="http://www.dronetology.net/dronetology#Component"/>
        <rdfs:comment xml:lang="en">replaces. Relates a component with another after a maintenance.</rdfs:comment>
        <rdfs:label xml:lang="en">replaces</rdfs:label>
    </owl:ObjectProperty>
    


    <!-- http://www.dronetology.net/dronetology#satisfiedBy -->

    <owl:ObjectProperty rdf:about="http://www.dronetology.net/dronetology#satisfiedBy">
        <owl:inverseOf rdf:resource="http://www.dronetology.net/dronetology#satisfies"/>
        <rdfs:domain rdf:resource="http://www.dronetology.net/dronetology#Requirement"/>
        <rdfs:range rdf:resource="http://www.dronetology.net/dronetology#Function"/>
        <rdfs:comment xml:lang="en">satisfiedBy. Relates a requirement with a function.</rdfs:comment>
        <rdfs:label xml:lang="en">satisfiedBy</rdfs:label>
    </owl:ObjectProperty>
    


    <!-- http://www.dronetology.net/dronetology#satisfies -->

    <owl:ObjectProperty rdf:about="http://www.dronetology.net/dronetology#satisfies">
        <rdfs:domain rdf:resource="http://www.dronetology.net/dronetology#Function"/>
        <rdfs:range rdf:resource="http://www.dronetology.net/dronetology#Requirement"/>
        <rdfs:comment xml:lang="en">satisfies. Relates a function with a requirement.</rdfs:comment>
        <rdfs:label xml:lang="en">satisfies</rdfs:label>
    </owl:ObjectProperty>
    


    <!-- http://www.dronetology.net/dronetology#satisfiesReq -->

    <owl:ObjectProperty rdf:about="http://www.dronetology.net/dronetology#satisfiesReq">
        <rdfs:domain rdf:resource="http://www.dronetology.net/dronetology#Component"/>
        <rdfs:range rdf:resource="http://www.dronetology.net/dronetology#Requirement"/>
        <rdfs:comment xml:lang="en">satisfiesReq. Relates a component with a requirement.</rdfs:comment>
        <rdfs:label xml:lang="en">satisfiesReq</rdfs:label>
    </owl:ObjectProperty>
    


    <!-- http://www.dronetology.net/dronetology#stores -->

    <owl:ObjectProperty rdf:about="http://www.dronetology.net/dronetology#stores">
        <rdfs:domain rdf:resource="http://www.dronetology.net/dronetology#DataStorageDevice"/>
        <rdfs:range>
            <owl:Class>
                <owl:unionOf rdf:parseType="Collection">
                    <rdf:Description rdf:about="http://www.dronetology.net/dronetology#Photograph"/>
                    <rdf:Description rdf:about="http://www.dronetology.net/dronetology#Video"/>
                </owl:unionOf>
            </owl:Class>
        </rdfs:range>
        <rdfs:comment xml:lang="en">stores. Relates a storage device with a digital content.</rdfs:comment>
        <rdfs:label xml:lang="en">stores</rdfs:label>
    </owl:ObjectProperty>
    


    <!-- http://www.dronetology.net/dronetology#usedInComprehension -->

    <owl:ObjectProperty rdf:about="http://www.dronetology.net/dronetology#usedInComprehension">
        <rdfs:domain rdf:resource="http://www.dronetology.net/dronetology#MissionElement"/>
        <rdfs:range rdf:resource="http://www.dronetology.net/dronetology#SituationalAwareness"/>
        <rdfs:comment xml:lang="en">usedInComprehension. Relates a mission element that provides situational awareness at the comprehension layer.</rdfs:comment>
        <rdfs:label xml:lang="en">usedInComprehension</rdfs:label>
    </owl:ObjectProperty>
    


    <!-- http://www.dronetology.net/dronetology#usedInPerception -->

    <owl:ObjectProperty rdf:about="http://www.dronetology.net/dronetology#usedInPerception">
        <rdfs:domain rdf:resource="http://www.dronetology.net/dronetology#MissionElement"/>
        <rdfs:range rdf:resource="http://www.dronetology.net/dronetology#SituationalAwareness"/>
        <rdfs:comment xml:lang="en">usedInPerception. Relates a mission element with situational awareness at the perception layer.</rdfs:comment>
        <rdfs:label xml:lang="en">usedInPerception</rdfs:label>
    </owl:ObjectProperty>
    


    <!-- http://www.dronetology.net/dronetology#usedInProjection -->

    <owl:ObjectProperty rdf:about="http://www.dronetology.net/dronetology#usedInProjection">
        <rdfs:domain rdf:resource="http://www.dronetology.net/dronetology#MissionElement"/>
        <rdfs:range rdf:resource="http://www.dronetology.net/dronetology#SituationalAwareness"/>
        <rdfs:comment xml:lang="en">usedInProjection. Relates a mission element with situational awareness at the projection layer.</rdfs:comment>
        <rdfs:label xml:lang="en">usedInProjection</rdfs:label>
    </owl:ObjectProperty>
    


    <!-- http://www.ontologydesignpatterns.org/ont/dul/DUL.owl#hasPart -->

    <owl:ObjectProperty rdf:about="http://www.ontologydesignpatterns.org/ont/dul/DUL.owl#hasPart"/>
    


    <!-- http://www.opengis.net/ont/geosparql#hasGeometry -->

    <owl:ObjectProperty rdf:about="http://www.opengis.net/ont/geosparql#hasGeometry">
        <rdfs:domain rdf:resource="http://www.dronetology.net/dronetology#Feature"/>
        <rdfs:range rdf:resource="http://www.opengis.net/ont/geosparql#Geometry"/>
    </owl:ObjectProperty>
    


    <!-- 
    ///////////////////////////////////////////////////////////////////////////////////////
    //
    // Data properties
    //
    ///////////////////////////////////////////////////////////////////////////////////////
     -->

    


    <!-- http://www.dronetology.net/dronetology#hasAlarmLevel -->

    <owl:DatatypeProperty rdf:about="http://www.dronetology.net/dronetology#hasAlarmLevel">
        <rdfs:domain rdf:resource="http://www.dronetology.net/dronetology#Alarm"/>
        <rdfs:range rdf:resource="http://www.w3.org/2001/XMLSchema#int"/>
        <rdfs:comment xml:lang="en">hasAlarmLevel. Defines the alarm level as an integer.</rdfs:comment>
        <rdfs:label xml:lang="en">hasAlarmLevel</rdfs:label>
    </owl:DatatypeProperty>
    


    <!-- http://www.dronetology.net/dronetology#hasAltitude -->

    <owl:DatatypeProperty rdf:about="http://www.dronetology.net/dronetology#hasAltitude">
        <rdfs:domain>
            <owl:Class>
                <owl:unionOf rdf:parseType="Collection">
                    <rdf:Description rdf:about="http://www.dronetology.net/dronetology#MissionGeometryElement"/>
                    <rdf:Description rdf:about="http://www.dronetology.net/dronetology#MissionGeometryPointElement"/>
                </owl:unionOf>
            </owl:Class>
        </rdfs:domain>
        <rdfs:range rdf:resource="http://www.w3.org/2001/XMLSchema#float"/>
        <rdfs:comment xml:lang="en">hasAltitude. Defines the altitude from the terrain surface.</rdfs:comment>
        <rdfs:label xml:lang="en">hasAltitude</rdfs:label>
    </owl:DatatypeProperty>
    


    <!-- http://www.dronetology.net/dronetology#hasComponentDescription -->

    <owl:DatatypeProperty rdf:about="http://www.dronetology.net/dronetology#hasComponentDescription">
        <rdfs:domain rdf:resource="http://www.dronetology.net/dronetology#Component"/>
        <rdfs:range rdf:resource="http://www.w3.org/2001/XMLSchema#string"/>
        <rdfs:comment xml:lang="en">hasComponentDescription. Defines a description for the component.</rdfs:comment>
        <rdfs:label xml:lang="en">hasComponentDescription</rdfs:label>
    </owl:DatatypeProperty>
    


    <!-- http://www.dronetology.net/dronetology#hasConstraintDescription -->

    <owl:DatatypeProperty rdf:about="http://www.dronetology.net/dronetology#hasConstraintDescription">
        <rdfs:domain rdf:resource="http://www.dronetology.net/dronetology#Constraint"/>
        <rdfs:range rdf:resource="http://www.w3.org/2001/XMLSchema#string"/>
        <rdfs:comment xml:lang="en">hasConstraintDescription. Defines a description for a constraint.</rdfs:comment>
        <rdfs:label xml:lang="en">hasConstraintDescription</rdfs:label>
    </owl:DatatypeProperty>
    


    <!-- http://www.dronetology.net/dronetology#hasConstraintPostedBy -->

    <owl:DatatypeProperty rdf:about="http://www.dronetology.net/dronetology#hasConstraintPostedBy">
        <rdfs:domain rdf:resource="http://www.dronetology.net/dronetology#Constraint"/>
        <rdfs:range rdf:resource="http://www.w3.org/2001/XMLSchema#string"/>
        <rdfs:comment xml:lang="en">hasConstraintPostedBy. Defines the origin of a constraint.</rdfs:comment>
        <rdfs:label xml:lang="en">hasConstraintPostedBy</rdfs:label>
    </owl:DatatypeProperty>
    


    <!-- http://www.dronetology.net/dronetology#hasConstraintStatus -->

    <owl:DatatypeProperty rdf:about="http://www.dronetology.net/dronetology#hasConstraintStatus">
        <rdfs:domain rdf:resource="http://www.dronetology.net/dronetology#Constraint"/>
        <rdfs:range rdf:resource="http://www.w3.org/2001/XMLSchema#string"/>
        <rdfs:comment xml:lang="en">hasConstraintStatus. Defines the status of a constraint.</rdfs:comment>
        <rdfs:label xml:lang="en">hasConstraintStatus</rdfs:label>
    </owl:DatatypeProperty>
    


    <!-- http://www.dronetology.net/dronetology#hasFeatureDescription -->

    <owl:DatatypeProperty rdf:about="http://www.dronetology.net/dronetology#hasFeatureDescription">
        <rdfs:domain rdf:resource="http://www.dronetology.net/dronetology#Feature"/>
        <rdfs:range rdf:resource="http://www.w3.org/2001/XMLSchema#string"/>
        <rdfs:comment xml:lang="en">hasFeatureDescription. Defines the description of a feature.</rdfs:comment>
        <rdfs:label xml:lang="en">hasFeatureDescription</rdfs:label>
    </owl:DatatypeProperty>
    


    <!-- http://www.dronetology.net/dronetology#hasFeatureType -->

    <owl:DatatypeProperty rdf:about="http://www.dronetology.net/dronetology#hasFeatureType">
        <rdfs:domain rdf:resource="http://www.dronetology.net/dronetology#Feature"/>
        <rdfs:range rdf:resource="http://www.w3.org/2001/XMLSchema#string"/>
        <rdfs:comment xml:lang="en">hasFeatureType. Defines the type of a feature.</rdfs:comment>
        <rdfs:label xml:lang="en">hasFeatureType</rdfs:label>
    </owl:DatatypeProperty>
    


    <!-- http://www.dronetology.net/dronetology#hasFlightAuthorization -->

    <owl:DatatypeProperty rdf:about="http://www.dronetology.net/dronetology#hasFlightAuthorization">
        <rdfs:domain rdf:resource="http://www.dronetology.net/dronetology#Mission"/>
        <rdfs:range rdf:resource="http://www.w3.org/2001/XMLSchema#string"/>
        <rdfs:comment xml:lang="en">hasFlightAuthorization. Defines the authorization given by an Agency for a drone flight.</rdfs:comment>
        <rdfs:label xml:lang="en">hasFlightAuthorization</rdfs:label>
    </owl:DatatypeProperty>
    


    <!-- http://www.dronetology.net/dronetology#hasFunctionNoun -->

    <owl:DatatypeProperty rdf:about="http://www.dronetology.net/dronetology#hasFunctionNoun">
        <rdfs:domain rdf:resource="http://www.dronetology.net/dronetology#Function"/>
        <rdfs:range rdf:resource="http://www.w3.org/2001/XMLSchema#string"/>
        <rdfs:comment xml:lang="en">hasFunctionNoun. Defines the noun of the function.</rdfs:comment>
        <rdfs:label xml:lang="en">hasFunctionNoun</rdfs:label>
    </owl:DatatypeProperty>
    


    <!-- http://www.dronetology.net/dronetology#hasFunctionVerb -->

    <owl:DatatypeProperty rdf:about="http://www.dronetology.net/dronetology#hasFunctionVerb">
        <rdfs:domain rdf:resource="http://www.dronetology.net/dronetology#Function"/>
        <rdfs:range rdf:resource="http://www.w3.org/2001/XMLSchema#string"/>
        <rdfs:comment xml:lang="en">hasFunctionVerb. Provides the verb of the function.</rdfs:comment>
        <rdfs:label xml:lang="en">hasFunctionVerb</rdfs:label>
    </owl:DatatypeProperty>
    


    <!-- http://www.dronetology.net/dronetology#hasIdentificator -->

    <owl:DatatypeProperty rdf:about="http://www.dronetology.net/dronetology#hasIdentificator">
        <rdfs:domain rdf:resource="http://www.dronetology.net/dronetology#Drone"/>
        <rdfs:range rdf:resource="http://www.w3.org/2001/XMLSchema#string"/>
        <rdfs:comment xml:lang="en">hasIdentificator. Provides the drone identificator</rdfs:comment>
        <rdfs:label xml:lang="en">hasIdentificator</rdfs:label>
    </owl:DatatypeProperty>
    


    <!-- http://www.dronetology.net/dronetology#hasMissionId -->

    <owl:DatatypeProperty rdf:about="http://www.dronetology.net/dronetology#hasMissionId">
        <rdfs:domain rdf:resource="http://www.dronetology.net/dronetology#Mission"/>
        <rdfs:range rdf:resource="http://www.w3.org/2001/XMLSchema#string"/>
        <rdfs:comment xml:lang="en">hasMissionId. Provides the identificator of a drone mission.</rdfs:comment>
        <rdfs:label xml:lang="en">hasMissionId</rdfs:label>
    </owl:DatatypeProperty>
    


    <!-- http://www.dronetology.net/dronetology#hasParameterDescription -->

    <owl:DatatypeProperty rdf:about="http://www.dronetology.net/dronetology#hasParameterDescription">
        <rdfs:domain rdf:resource="http://www.dronetology.net/dronetology#Parameter"/>
        <rdfs:range rdf:resource="http://www.w3.org/2001/XMLSchema#string"/>
        <rdfs:comment xml:lang="en">hasParameterDescription. Provides the description of a parameter.</rdfs:comment>
        <rdfs:label xml:lang="en">hasParameterDescription</rdfs:label>
    </owl:DatatypeProperty>
    


    <!-- http://www.dronetology.net/dronetology#hasRawHEXContent -->

    <owl:DatatypeProperty rdf:about="http://www.dronetology.net/dronetology#hasRawHEXContent">
        <rdfs:domain rdf:resource="http://www.dronetology.net/dronetology#CommunicationMessage"/>
        <rdfs:range rdf:resource="http://www.w3.org/2001/XMLSchema#string"/>
        <rdfs:comment xml:lang="en">hasRawHexContent. Provides the raw content of a communication message.</rdfs:comment>
        <rdfs:label xml:lang="en">hasRawHEXContent</rdfs:label>
    </owl:DatatypeProperty>
    


    <!-- http://www.dronetology.net/dronetology#hasRequirementDescription -->

    <owl:DatatypeProperty rdf:about="http://www.dronetology.net/dronetology#hasRequirementDescription">
        <rdfs:domain rdf:resource="http://www.dronetology.net/dronetology#Requirement"/>
        <rdfs:range rdf:resource="http://www.w3.org/2001/XMLSchema#string"/>
        <rdfs:comment xml:lang="en">hasRequirementDescription. Defines the description of a requirement.</rdfs:comment>
        <rdfs:label xml:lang="en">hasRequirementDescription</rdfs:label>
    </owl:DatatypeProperty>
    


    <!-- http://www.dronetology.net/dronetology#hasRequirementPostedBy -->

    <owl:DatatypeProperty rdf:about="http://www.dronetology.net/dronetology#hasRequirementPostedBy">
        <rdfs:domain rdf:resource="http://www.dronetology.net/dronetology#Requirement"/>
        <rdfs:range rdf:resource="http://www.w3.org/2001/XMLSchema#string"/>
        <rdfs:comment xml:lang="en">hasRequirementPostedBy. Provides the origin of a requirement.</rdfs:comment>
        <rdfs:label xml:lang="en">hasRequirementPostedBy</rdfs:label>
    </owl:DatatypeProperty>
    


    <!-- http://www.dronetology.net/dronetology#hasRequirementStatus -->

    <owl:DatatypeProperty rdf:about="http://www.dronetology.net/dronetology#hasRequirementStatus">
        <rdfs:domain rdf:resource="http://www.dronetology.net/dronetology#Requirement"/>
        <rdfs:range rdf:resource="http://www.w3.org/2001/XMLSchema#string"/>
        <rdfs:comment xml:lang="en">hasRequirementStatus. Defines the status of the requirement.</rdfs:comment>
        <rdfs:label xml:lang="en">hasRequirementStatus</rdfs:label>
    </owl:DatatypeProperty>
    


    <!-- http://www.dronetology.net/dronetology#hasRequirementValue -->

    <owl:DatatypeProperty rdf:about="http://www.dronetology.net/dronetology#hasRequirementValue">
        <rdfs:domain rdf:resource="http://www.dronetology.net/dronetology#Requirement"/>
        <rdfs:range rdf:resource="http://www.w3.org/2001/XMLSchema#float"/>
        <rdfs:comment xml:lang="en">hasRequirementValue. Provides the value of the requirement.</rdfs:comment>
        <rdfs:label xml:lang="en">hasRequirementValue</rdfs:label>
    </owl:DatatypeProperty>
    


    <!-- http://www.dronetology.net/dronetology#hasSKU -->

    <owl:DatatypeProperty rdf:about="http://www.dronetology.net/dronetology#hasSKU">
        <rdfs:domain rdf:resource="http://www.dronetology.net/dronetology#Component"/>
        <rdfs:range rdf:resource="http://www.w3.org/2001/XMLSchema#string"/>
        <rdfs:comment xml:lang="en">hasSKU. Provides the SKU identificator of a drone component.</rdfs:comment>
        <rdfs:label xml:lang="en">hasSKU</rdfs:label>
    </owl:DatatypeProperty>
    


    <!-- http://www.dronetology.net/dronetology#hasSerialNumber -->

    <owl:DatatypeProperty rdf:about="http://www.dronetology.net/dronetology#hasSerialNumber">
        <rdfs:domain rdf:resource="http://www.dronetology.net/dronetology#Drone"/>
        <rdfs:range rdf:resource="http://www.w3.org/2001/XMLSchema#string"/>
        <rdfs:comment xml:lang="en">hasSerialNumber. Provides the serial number of a drone.</rdfs:comment>
        <rdfs:label xml:lang="en">hasSerialNumber</rdfs:label>
    </owl:DatatypeProperty>
    


    <!-- http://www.dronetology.net/dronetology#hasVerifyMethod -->

    <owl:DatatypeProperty rdf:about="http://www.dronetology.net/dronetology#hasVerifyMethod">
        <rdfs:domain rdf:resource="http://www.dronetology.net/dronetology#Requirement"/>
        <rdfs:range rdf:resource="http://www.w3.org/2001/XMLSchema#string"/>
        <rdfs:comment xml:lang="en">hasVerifyMethod. Describes the method used to verify the requirement.</rdfs:comment>
        <rdfs:label xml:lang="en">hasVerifyMethod</rdfs:label>
    </owl:DatatypeProperty>
    


    <!-- http://www.dronetology.net/dronetology#hasVersionNumber -->

    <owl:DatatypeProperty rdf:about="http://www.dronetology.net/dronetology#hasVersionNumber">
        <rdfs:domain rdf:resource="http://www.dronetology.net/dronetology#Component"/>
        <rdfs:range rdf:resource="http://www.w3.org/2001/XMLSchema#string"/>
        <rdfs:comment xml:lang="en">hasVersionNumber. Provides the serial number of a drone component.</rdfs:comment>
        <rdfs:label xml:lang="en">hasVersionNumber</rdfs:label>
    </owl:DatatypeProperty>
    


    <!-- http://www.dronetology.net/dronetology#hasWeatherProvider -->

    <owl:DatatypeProperty rdf:about="http://www.dronetology.net/dronetology#hasWeatherProvider">
        <rdfs:domain rdf:resource="http://www.dronetology.net/dronetology#MissionWeatherReport"/>
        <rdfs:range rdf:resource="http://www.w3.org/2001/XMLSchema#string"/>
        <rdfs:comment xml:lang="en">hasWeatherProvider. Defines the weather report provider.</rdfs:comment>
        <rdfs:label xml:lang="en">hasWeatherProvider</rdfs:label>
    </owl:DatatypeProperty>
    


    <!-- http://www.dronetology.net/dronetology#inferred -->

    <owl:DatatypeProperty rdf:about="http://www.dronetology.net/dronetology#inferred">
        <rdfs:domain rdf:resource="http://www.dronetology.net/dronetology#Command"/>
        <rdfs:range rdf:resource="http://www.w3.org/2001/XMLSchema#boolean"/>
        <rdfs:comment xml:lang="en">inferred. Defines if the command has been obtained from an inference.</rdfs:comment>
        <rdfs:label xml:lang="en">inferred</rdfs:label>
    </owl:DatatypeProperty>
    


    <!-- 
    ///////////////////////////////////////////////////////////////////////////////////////
    //
    // Classes
    //
    ///////////////////////////////////////////////////////////////////////////////////////
     -->

    


    <!-- http://purl.org/dc/terms/LicenseDocument -->

    <owl:Class rdf:about="http://purl.org/dc/terms/LicenseDocument">
        <rdfs:comment xml:lang="en">LicenseDocument</rdfs:comment>
        <rdfs:label xml:lang="en">LicenseDocument</rdfs:label>
    </owl:Class>
    


    <!-- http://qudt.org/schema/qudt/Quantity -->

    <owl:Class rdf:about="http://qudt.org/schema/qudt/Quantity"/>
    


    <!-- http://qudt.org/schema/qudt/Unit -->

    <owl:Class rdf:about="http://qudt.org/schema/qudt/Unit"/>
    


    <!-- http://www.dronetology.net/DroneRegulation_EU_2019_945 -->

    <owl:Class rdf:about="http://www.dronetology.net/DroneRegulation_EU_2019_945">
        <rdfs:subClassOf rdf:resource="http://www.dronetology.net/dronetology#Regulation"/>
        <rdfs:comment xml:lang="en">DroneRegulation_EU_2019_945. EU regulation approved at 2019.</rdfs:comment>
        <rdfs:label xml:lang="en">DroneRegulation_EU_2019_945</rdfs:label>
    </owl:Class>
    


    <!-- http://www.dronetology.net/dronetology#AA -->

    <owl:Class rdf:about="http://www.dronetology.net/dronetology#AA">
        <rdfs:subClassOf rdf:resource="http://www.dronetology.net/dronetology#Drone"/>
        <owl:disjointWith rdf:resource="http://www.dronetology.net/dronetology#RPA"/>
        <rdfs:comment xml:lang="en">AA. Autonomous Aircraft</rdfs:comment>
        <rdfs:label xml:lang="en">AA</rdfs:label>
    </owl:Class>
    


    <!-- http://www.dronetology.net/dronetology#AAS -->

    <owl:Class rdf:about="http://www.dronetology.net/dronetology#AAS">
        <rdfs:subClassOf rdf:resource="http://www.dronetology.net/dronetology#AA"/>
        <rdfs:comment xml:lang="en">AAS. Autonomous Aerial System</rdfs:comment>
        <rdfs:label xml:lang="en">AAS</rdfs:label>
    </owl:Class>
    


    <!-- http://www.dronetology.net/dronetology#ADSB -->

    <owl:Class rdf:about="http://www.dronetology.net/dronetology#ADSB">
        <rdfs:subClassOf rdf:resource="http://www.dronetology.net/dronetology#MessageReceived"/>
        <owl:disjointWith rdf:resource="http://www.dronetology.net/dronetology#RemoteId"/>
        <rdfs:isDefinedBy xml:lang="en">ADSB. Messages received from an ADSB Automatic Dependent Surveillance Broadcast transponder.</rdfs:isDefinedBy>
        <rdfs:label xml:lang="en">ADSB</rdfs:label>
    </owl:Class>
    


    <!-- http://www.dronetology.net/dronetology#AUAS -->

    <owl:Class rdf:about="http://www.dronetology.net/dronetology#AUAS">
        <rdfs:subClassOf>
            <owl:Class>
                <owl:intersectionOf rdf:parseType="Collection">
                    <rdf:Description rdf:about="http://www.dronetology.net/dronetology#UAS"/>
                    <owl:Restriction>
                        <owl:onProperty rdf:resource="http://www.dronetology.net/dronetology#hasMission"/>
                        <owl:someValuesFrom rdf:resource="http://www.dronetology.net/dronetology#AutonomousMission"/>
                    </owl:Restriction>
                </owl:intersectionOf>
            </owl:Class>
        </rdfs:subClassOf>
        <rdfs:comment>Autonomous Unmanned Aircraft System</rdfs:comment>
        <rdfs:label xml:lang="en">AUAS</rdfs:label>
    </owl:Class>
    


    <!-- http://www.dronetology.net/dronetology#Acceleration -->

    <owl:Class rdf:about="http://www.dronetology.net/dronetology#Acceleration">
        <rdfs:subClassOf rdf:resource="http://qudt.org/schema/qudt/Quantity"/>
        <rdfs:comment xml:lang="en">Acceleration. A drone capacity to gain speed.</rdfs:comment>
        <rdfs:label xml:lang="en">Acceleration</rdfs:label>
    </owl:Class>
    


    <!-- http://www.dronetology.net/dronetology#Accelerometer -->

    <owl:Class rdf:about="http://www.dronetology.net/dronetology#Accelerometer">
        <rdfs:subClassOf rdf:resource="http://www.dronetology.net/dronetology#InertialNavigationUnit"/>
        <rdfs:comment xml:lang="en">Accelerometer. Accelerometers are used for flight stabilisation in UAVs and drones, being able to measure the orientation of the aircraft as well as the effects of sudden acceleration due to wind or sharp turns.</rdfs:comment>
        <rdfs:label xml:lang="en">Accelerometer</rdfs:label>
    </owl:Class>
    


    <!-- http://www.dronetology.net/dronetology#Advisory -->

    <owl:Class rdf:about="http://www.dronetology.net/dronetology#Advisory">
        <rdfs:comment xml:lang="en">Advisory. An official announcement or warning about air traffic.</rdfs:comment>
        <rdfs:label xml:lang="en">Advisory</rdfs:label>
    </owl:Class>
    


    <!-- http://www.dronetology.net/dronetology#AerialDevelopmentFramework -->

    <owl:Class rdf:about="http://www.dronetology.net/dronetology#AerialDevelopmentFramework">
        <rdfs:subClassOf rdf:resource="http://www.dronetology.net/dronetology#SoftwareComponent"/>
        <rdfs:comment xml:lang="en">AerialDevelopmentFramework. A framework that helps researchers and developers build and reuse code between drone applications.</rdfs:comment>
        <rdfs:label xml:lang="en">AerialDevelopmentFramework</rdfs:label>
    </owl:Class>
    


    <!-- http://www.dronetology.net/dronetology#AerialVehicle -->

    <owl:Class rdf:about="http://www.dronetology.net/dronetology#AerialVehicle">
        <rdfs:subClassOf>
            <owl:Class>
                <owl:intersectionOf rdf:parseType="Collection">
                    <rdf:Description rdf:about="http://www.dronetology.net/dronetology#HardwareComponent"/>
                    <owl:Restriction>
                        <owl:onProperty rdf:resource="http://www.dronetology.net/dronetology#hasDirectPart"/>
                        <owl:someValuesFrom rdf:resource="http://www.dronetology.net/dronetology#AircraftComponent"/>
                    </owl:Restriction>
                </owl:intersectionOf>
            </owl:Class>
        </rdfs:subClassOf>
        <owl:disjointWith rdf:resource="http://www.dronetology.net/dronetology#GroundStation"/>
        <owl:disjointWith rdf:resource="http://www.dronetology.net/dronetology#GroundStationComponent"/>
        <owl:disjointWith rdf:resource="http://www.dronetology.net/dronetology#LaunchSystem"/>
        <rdfs:comment xml:lang="en">AerialVehicle. Pilotless Aircraft</rdfs:comment>
        <rdfs:label xml:lang="en">AerialVehicle</rdfs:label>
    </owl:Class>
    


    <!-- http://www.dronetology.net/dronetology#Ailerons -->

    <owl:Class rdf:about="http://www.dronetology.net/dronetology#Ailerons">
        <rdfs:subClassOf rdf:resource="http://www.dronetology.net/dronetology#WingComponent"/>
        <rdfs:comment xml:lang="en">Aileron. Located near the outer edge of the wing, ailerons are used to control the roll of the aircraft. By moving the ailerons up or down, the pilot can bank the aircraft, enabling it to turn left or right.</rdfs:comment>
        <rdfs:label xml:lang="en">Aileron</rdfs:label>
    </owl:Class>
    


    <!-- http://www.dronetology.net/dronetology#AirSpaceVolume -->

    <owl:Class rdf:about="http://www.dronetology.net/dronetology#AirSpaceVolume">
        <rdfs:subClassOf rdf:resource="http://www.opengis.net/ont/geosparql#Feature"/>
        <rdfs:comment xml:lang="en">AirSpaceVolume. The airspace is the portion of the atmosphere controlled by a country above its territory, including its territorial waters or, more generally, any specific three-dimensional portion of the atmosphere.</rdfs:comment>
        <rdfs:label xml:lang="en">AirSpaceVolume</rdfs:label>
    </owl:Class>
    


    <!-- http://www.dronetology.net/dronetology#AirSpeed -->

    <owl:Class rdf:about="http://www.dronetology.net/dronetology#AirSpeed">
        <rdfs:subClassOf rdf:resource="http://www.dronetology.net/dronetology#Speed"/>
        <rdfs:comment xml:lang="en">Airspeed. The speed that the drone is facing the air which is moving over the wings.</rdfs:comment>
        <rdfs:label xml:lang="en">Airspeed</rdfs:label>
    </owl:Class>
    


    <!-- http://www.dronetology.net/dronetology#AircraftComponent -->

    <owl:Class rdf:about="http://www.dronetology.net/dronetology#AircraftComponent">
        <rdfs:subClassOf rdf:resource="http://www.dronetology.net/dronetology#HardwareComponent"/>
        <owl:disjointWith rdf:resource="http://www.dronetology.net/dronetology#GroundStation"/>
        <owl:disjointWith rdf:resource="http://www.dronetology.net/dronetology#GroundStationComponent"/>
        <owl:disjointWith rdf:resource="http://www.dronetology.net/dronetology#LaunchSystem"/>
        <rdfs:comment xml:lang="en">AircraftComponent. Aircraft component.</rdfs:comment>
        <rdfs:label xml:lang="en">AircraftComponent</rdfs:label>
    </owl:Class>
    


    <!-- http://www.dronetology.net/dronetology#AirportNoFlyZone -->

    <owl:Class rdf:about="http://www.dronetology.net/dronetology#AirportNoFlyZone">
        <rdfs:subClassOf rdf:resource="http://www.dronetology.net/dronetology#NoFlyZone"/>
        <rdfs:comment xml:lang="en">AirportNoFlyZone. Restricted fly zone around an airport.</rdfs:comment>
        <rdfs:label xml:lang="en">AirportNoFlyZone</rdfs:label>
    </owl:Class>
    


    <!-- http://www.dronetology.net/dronetology#AirportSecurityNoFlyDistance -->

    <owl:Class rdf:about="http://www.dronetology.net/dronetology#AirportSecurityNoFlyDistance">
        <rdfs:subClassOf rdf:resource="http://www.dronetology.net/dronetology#Distance"/>
        <rdfs:comment xml:lang="en">AirportSecurityNoFlyDistance. Minimum distance to an airport that is required for flying a drone.</rdfs:comment>
        <rdfs:label xml:lang="en">AirportSecurityNoFlyDistance</rdfs:label>
    </owl:Class>
    


    <!-- http://www.dronetology.net/dronetology#Alarm -->

    <owl:Class rdf:about="http://www.dronetology.net/dronetology#Alarm">
        <rdfs:subClassOf rdf:resource="http://www.w3.org/2002/07/owl#Thing"/>
        <rdfs:comment xml:lang="en">Alarm. A warning of danger.</rdfs:comment>
        <rdfs:label xml:lang="en">Alarm</rdfs:label>
    </owl:Class>
    


    <!-- http://www.dronetology.net/dronetology#Antenna -->

    <owl:Class rdf:about="http://www.dronetology.net/dronetology#Antenna">
        <rdfs:subClassOf rdf:resource="http://www.dronetology.net/dronetology#AircraftComponent"/>
        <owl:disjointWith rdf:resource="http://www.dronetology.net/dronetology#CommunicationSystem"/>
        <owl:disjointWith rdf:resource="http://www.dronetology.net/dronetology#DataProcessingBoard"/>
        <owl:disjointWith rdf:resource="http://www.dronetology.net/dronetology#DataStorageDevice"/>
        <owl:disjointWith rdf:resource="http://www.dronetology.net/dronetology#EnergyStorageComponent"/>
        <owl:disjointWith rdf:resource="http://www.dronetology.net/dronetology#Engine"/>
        <owl:disjointWith rdf:resource="http://www.dronetology.net/dronetology#FlightControllerUnit"/>
        <owl:disjointWith rdf:resource="http://www.dronetology.net/dronetology#Fuselage"/>
        <owl:disjointWith rdf:resource="http://www.dronetology.net/dronetology#InertialNavigationUnit"/>
        <owl:disjointWith rdf:resource="http://www.dronetology.net/dronetology#LandingComponent"/>
        <owl:disjointWith rdf:resource="http://www.dronetology.net/dronetology#LiftGeneratorComponent"/>
        <owl:disjointWith rdf:resource="http://www.dronetology.net/dronetology#Payload"/>
        <rdfs:comment xml:lang="en">Antenna. A rod, wire, or other device used to transmit or receive radio signals.</rdfs:comment>
        <rdfs:label xml:lang="en">Antenna</rdfs:label>
    </owl:Class>
    


    <!-- http://www.dronetology.net/dronetology#AntiDroneWeapon -->

    <owl:Class rdf:about="http://www.dronetology.net/dronetology#AntiDroneWeapon">
        <rdfs:subClassOf rdf:resource="http://www.dronetology.net/dronetology#AuxiliaryComponent"/>
        <rdfs:comment xml:lang="en">AntiDroneWeapon.  Used to detect and/or intercept unwanted drones and unmanned aerial vehicles (UAVs).</rdfs:comment>
        <rdfs:label xml:lang="en">AntiDroneWeapon or C-UAS</rdfs:label>
    </owl:Class>
    


    <!-- http://www.dronetology.net/dronetology#AntiVibrationComponent -->

    <owl:Class rdf:about="http://www.dronetology.net/dronetology#AntiVibrationComponent">
        <rdfs:subClassOf rdf:resource="http://www.dronetology.net/dronetology#AircraftComponent"/>
        <rdfs:comment xml:lang="en">AntiVibrationComponent.  A flexible support for an engine that reduces the amount of noise and vibration that passes to the vehicle chassis.</rdfs:comment>
        <rdfs:label xml:lang="en">AntiVibrationComponent</rdfs:label>
    </owl:Class>
    


    <!-- http://www.dronetology.net/dronetology#Arm -->

    <owl:Class rdf:about="http://www.dronetology.net/dronetology#Arm">
        <rdfs:subClassOf rdf:resource="http://www.dronetology.net/dronetology#Fuselage"/>
        <rdfs:comment xml:lang="en">Arm. The arms of a drone are the components that support the motors and are attached to the frame or base structure of the drone.</rdfs:comment>
        <rdfs:label xml:lang="en">Arm</rdfs:label>
    </owl:Class>
    


    <!-- http://www.dronetology.net/dronetology#Authorization -->

    <owl:Class rdf:about="http://www.dronetology.net/dronetology#Authorization">
        <rdfs:subClassOf rdf:resource="http://www.dronetology.net/dronetology#RegulationRequirement"/>
        <rdfs:comment xml:lang="en">Authorization. A requirement that identifies the drone and the drone operator before a fly.</rdfs:comment>
        <rdfs:label xml:lang="en">Authorization</rdfs:label>
    </owl:Class>
    


    <!-- http://www.dronetology.net/dronetology#AutonomousMission -->

    <owl:Class rdf:about="http://www.dronetology.net/dronetology#AutonomousMission">
        <rdfs:subClassOf rdf:resource="http://www.dronetology.net/dronetology#Mission"/>
        <rdfs:subClassOf>
            <owl:Restriction>
                <owl:onProperty rdf:resource="http://www.dronetology.net/dronetology#hasElement"/>
                <owl:qualifiedCardinality rdf:datatype="http://www.w3.org/2001/XMLSchema#nonNegativeInteger">1</owl:qualifiedCardinality>
                <owl:onClass rdf:resource="http://www.dronetology.net/dronetology#FlightPlan"/>
            </owl:Restriction>
        </rdfs:subClassOf>
        <owl:disjointWith rdf:resource="http://www.dronetology.net/dronetology#RemoteGuided"/>
        <rdfs:comment xml:lang="en">AutonomousMission. A mission performed independently, without direct pilot involvement.</rdfs:comment>
        <rdfs:label xml:lang="en">AutonomousMission</rdfs:label>
    </owl:Class>
    


    <!-- http://www.dronetology.net/dronetology#AuxiliaryCommand -->

    <owl:Class rdf:about="http://www.dronetology.net/dronetology#AuxiliaryCommand">
        <rdfs:subClassOf rdf:resource="http://www.dronetology.net/dronetology#Command"/>
        <owl:disjointWith>
            <owl:Class>
                <owl:unionOf rdf:parseType="Collection">
                    <rdf:Description rdf:about="http://www.dronetology.net/dronetology#GoToCommand"/>
                    <rdf:Description rdf:about="http://www.dronetology.net/dronetology#NEDVelocityCommand"/>
                </owl:unionOf>
            </owl:Class>
        </owl:disjointWith>
        <rdfs:comment xml:lang="en">AuxiliaryCommand. Any command that controls the payload and functions that does not relate with drone movement</rdfs:comment>
        <rdfs:label xml:lang="en">AuxiliaryCommand</rdfs:label>
    </owl:Class>
    


    <!-- http://www.dronetology.net/dronetology#AuxiliaryComponent -->

    <owl:Class rdf:about="http://www.dronetology.net/dronetology#AuxiliaryComponent">
        <rdfs:subClassOf rdf:resource="http://www.dronetology.net/dronetology#Component"/>
        <owl:disjointWith rdf:resource="http://www.dronetology.net/dronetology#DataLink"/>
        <owl:disjointWith rdf:resource="http://www.dronetology.net/dronetology#SoftwareComponent"/>
        <rdfs:comment xml:lang="en">AuxiliaryComponent.  Any device, materials or equipment which is used to give assistance or aid to the drone but is not a permanent or enclosed part of the drone.</rdfs:comment>
        <rdfs:label xml:lang="en">AuxiliaryComponent</rdfs:label>
    </owl:Class>
    


    <!-- http://www.dronetology.net/dronetology#BVLOSMission -->

    <owl:Class rdf:about="http://www.dronetology.net/dronetology#BVLOSMission">
        <rdfs:subClassOf>
            <owl:Class>
                <owl:intersectionOf rdf:parseType="Collection">
                    <rdf:Description rdf:about="http://www.dronetology.net/dronetology#Mission"/>
                    <owl:Restriction>
                        <owl:onProperty rdf:resource="http://www.dronetology.net/dronetology#hasElement"/>
                        <owl:qualifiedCardinality rdf:datatype="http://www.w3.org/2001/XMLSchema#nonNegativeInteger">1</owl:qualifiedCardinality>
                        <owl:onClass rdf:resource="http://www.dronetology.net/dronetology#NoFlyZone"/>
                    </owl:Restriction>
                </owl:intersectionOf>
            </owl:Class>
        </rdfs:subClassOf>
        <rdfs:comment xml:lang="en">BVLOSMission. A mission beyond the visual line of sight of the pilot.</rdfs:comment>
        <rdfs:label xml:lang="en">BVLOSMission</rdfs:label>
    </owl:Class>
    


    <!-- http://www.dronetology.net/dronetology#BarometricPressure -->

    <owl:Class rdf:about="http://www.dronetology.net/dronetology#BarometricPressure">
        <rdfs:subClassOf rdf:resource="http://qudt.org/schema/qudt/Quantity"/>
        <rdfs:comment xml:lang="en">BarometricPressure. The measurement of air pressure in the atmosphere.</rdfs:comment>
        <rdfs:label xml:lang="en">BarometricPressure</rdfs:label>
    </owl:Class>
    


    <!-- http://www.dronetology.net/dronetology#BasicComplaince -->

    <owl:Class rdf:about="http://www.dronetology.net/dronetology#BasicComplaince">
        <rdfs:subClassOf rdf:resource="http://www.dronetology.net/dronetology#Regulation"/>
        <rdfs:subClassOf>
            <owl:Class>
                <owl:intersectionOf rdf:parseType="Collection">
                    <owl:Restriction>
                        <owl:onProperty rdf:resource="http://www.dronetology.net/dronetology#hasPilot"/>
                        <owl:minQualifiedCardinality rdf:datatype="http://www.w3.org/2001/XMLSchema#nonNegativeInteger">1</owl:minQualifiedCardinality>
                        <owl:onClass rdf:resource="http://www.dronetology.net/dronetology#Pilot"/>
                    </owl:Restriction>
                    <owl:Restriction>
                        <owl:onProperty rdf:resource="http://www.dronetology.net/dronetology#isElementOf"/>
                        <owl:qualifiedCardinality rdf:datatype="http://www.w3.org/2001/XMLSchema#nonNegativeInteger">1</owl:qualifiedCardinality>
                        <owl:onClass rdf:resource="http://www.dronetology.net/dronetology#Mission"/>
                    </owl:Restriction>
                </owl:intersectionOf>
            </owl:Class>
        </rdfs:subClassOf>
        <rdfs:comment xml:lang="en">BasicComplaince. Basic and most common safety rules that apply to most countries.</rdfs:comment>
        <rdfs:label xml:lang="en">BasicComplaince</rdfs:label>
    </owl:Class>
    


    <!-- http://www.dronetology.net/dronetology#Battery -->

    <owl:Class rdf:about="http://www.dronetology.net/dronetology#Battery">
        <rdfs:subClassOf rdf:resource="http://www.dronetology.net/dronetology#EnergyStorageComponent"/>
        <owl:disjointWith rdf:resource="http://www.dronetology.net/dronetology#FuelTank"/>
        <rdfs:comment xml:lang="en">Battery. A container consisting of one or more cells, in which chemical energy is converted into electricity and used as a source of power.</rdfs:comment>
        <rdfs:label xml:lang="en">Battery</rdfs:label>
    </owl:Class>
    


    <!-- http://www.dronetology.net/dronetology#BatteryAlarm -->

    <owl:Class rdf:about="http://www.dronetology.net/dronetology#BatteryAlarm">
        <rdfs:subClassOf rdf:resource="http://www.dronetology.net/dronetology#Alarm"/>
        <owl:disjointWith rdf:resource="http://www.dronetology.net/dronetology#NoFlyZoneAlarm"/>
        <rdfs:comment xml:lang="en">BatteryAlarm. A warning provoked by a low battery level.</rdfs:comment>
        <rdfs:label xml:lang="en">BatteryAlarm</rdfs:label>
    </owl:Class>
    


    <!-- http://www.dronetology.net/dronetology#Beidou -->

    <owl:Class rdf:about="http://www.dronetology.net/dronetology#Beidou">
        <rdfs:subClassOf rdf:resource="http://www.dronetology.net/dronetology#GlobalNavigationSatelliteSystem"/>
        <rdfs:comment xml:lang="en">Beidu. BeiDou, or BDS, is a global GNSS owned and operated by the People&apos;s Republic of China.</rdfs:comment>
        <rdfs:label xml:lang="en">Beidu</rdfs:label>
    </owl:Class>
    


    <!-- http://www.dronetology.net/dronetology#Broadcast_Remote_ID -->

    <owl:Class rdf:about="http://www.dronetology.net/dronetology#Broadcast_Remote_ID">
        <rdfs:subClassOf rdf:resource="http://www.dronetology.net/dronetology#RemoteID"/>
        <rdfs:comment xml:lang="en">Broadcast_Remote_ID. RemoteID transmitted through a broadcast communication channel.</rdfs:comment>
        <rdfs:label xml:lang="en">Broadcast_Remote_ID</rdfs:label>
    </owl:Class>
    


    <!-- http://www.dronetology.net/dronetology#C2Link -->

    <owl:Class rdf:about="http://www.dronetology.net/dronetology#C2Link">
        <rdfs:subClassOf rdf:resource="http://www.dronetology.net/dronetology#DataLink"/>
    </owl:Class>
    


    <!-- http://www.dronetology.net/dronetology#Cabin -->

    <owl:Class rdf:about="http://www.dronetology.net/dronetology#Cabin">
        <rdfs:subClassOf rdf:resource="http://www.dronetology.net/dronetology#Fuselage"/>
        <rdfs:comment xml:lang="en">Cabin. A separate space in an aircraft for passengers.</rdfs:comment>
        <rdfs:label xml:lang="en">Cabin</rdfs:label>
    </owl:Class>
    


    <!-- http://www.dronetology.net/dronetology#Cable -->

    <owl:Class rdf:about="http://www.dronetology.net/dronetology#Cable">
        <rdfs:subClassOf rdf:resource="http://www.dronetology.net/dronetology#AuxiliaryComponent"/>
        <rdfs:comment xml:lang="en">Cable. A cable is a thick wire, or a group of wires inside a rubber or plastic covering, which is used to carry electricity or electronic signals.</rdfs:comment>
        <rdfs:label xml:lang="en">Cable</rdfs:label>
    </owl:Class>
    


    <!-- http://www.dronetology.net/dronetology#Camera -->

    <owl:Class rdf:about="http://www.dronetology.net/dronetology#Camera">
        <rdfs:subClassOf rdf:resource="http://www.dronetology.net/dronetology#Payload"/>
        <rdfs:comment xml:lang="en">Camera. A device for recording visual images in the form of photographs, film, or video signals.</rdfs:comment>
        <rdfs:label xml:lang="en">Camera</rdfs:label>
    </owl:Class>
    


    <!-- http://www.dronetology.net/dronetology#Capacity -->

    <owl:Class rdf:about="http://www.dronetology.net/dronetology#Capacity">
        <rdfs:subClassOf rdf:resource="http://qudt.org/schema/qudt/Quantity"/>
        <rdfs:comment xml:lang="en">Capacity. The total amount that can be contained in a drone.</rdfs:comment>
        <rdfs:label xml:lang="en">Capacity</rdfs:label>
    </owl:Class>
    


    <!-- http://www.dronetology.net/dronetology#Catapult -->

    <owl:Class rdf:about="http://www.dronetology.net/dronetology#Catapult">
        <rdfs:subClassOf rdf:resource="http://www.dronetology.net/dronetology#LaunchSystem"/>
        <rdfs:comment xml:lang="en">Catapult. A combination of rails, elastic bands, etc. used to launch a drone. It provides longer launch ranges by providing a initial boost of speed and altitude.</rdfs:comment>
        <rdfs:label xml:lang="en">Catapult</rdfs:label>
    </owl:Class>
    


    <!-- http://www.dronetology.net/dronetology#ChargingStation -->

    <owl:Class rdf:about="http://www.dronetology.net/dronetology#ChargingStation">
        <rdfs:subClassOf rdf:resource="http://www.dronetology.net/dronetology#AuxiliaryComponent"/>
        <owl:disjointWith rdf:resource="http://www.dronetology.net/dronetology#RefuelingSystem"/>
        <rdfs:comment xml:lang="en">ChargingStation. A power supply device that supplies electrical power for recharging plug-in electric vehicles.</rdfs:comment>
        <rdfs:label xml:lang="en">ChargingStation</rdfs:label>
    </owl:Class>
    


    <!-- http://www.dronetology.net/dronetology#CivilManufacturer -->

    <owl:Class rdf:about="http://www.dronetology.net/dronetology#CivilManufacturer">
        <rdfs:subClassOf rdf:resource="http://www.dronetology.net/dronetology#Manufacturer"/>
        <owl:disjointWith rdf:resource="http://www.dronetology.net/dronetology#MilitaryManufacturer"/>
        <rdfs:comment>Drone manufacturers of civil drones either produce drones for two types: commercial purposes (e.g. drones used in the energy, construction, agriculture or transport industry) and/or for private individuals for hobby flights.</rdfs:comment>
        <rdfs:label xml:lang="en">CivilManufacturer</rdfs:label>
    </owl:Class>
    


    <!-- http://www.dronetology.net/dronetology#CollaborativeDrone -->

    <owl:Class rdf:about="http://www.dronetology.net/dronetology#CollaborativeDrone">
        <rdfs:subClassOf rdf:resource="http://www.dronetology.net/dronetology#Drone"/>
        <rdfs:comment xml:lang="en">CollaborativeDrone. Drone with specific equipment that allows to collaborate with others.</rdfs:comment>
        <rdfs:label xml:lang="en">CollaborativeDrone</rdfs:label>
    </owl:Class>
    


    <!-- http://www.dronetology.net/dronetology#CollisionAlarm -->

    <owl:Class rdf:about="http://www.dronetology.net/dronetology#CollisionAlarm">
        <rdfs:subClassOf rdf:resource="http://www.dronetology.net/dronetology#Alarm"/>
        <rdfs:comment xml:lang="en">CollisionAlarm. A warning provoked when two aircraft are flying below a security distance.</rdfs:comment>
        <rdfs:label xml:lang="en">CollisionAlarm</rdfs:label>
    </owl:Class>
    


    <!-- http://www.dronetology.net/dronetology#CollisionRisk -->

    <owl:Class rdf:about="http://www.dronetology.net/dronetology#CollisionRisk">
        <rdfs:subClassOf rdf:resource="http://www.dronetology.net/dronetology#Risk"/>
        <rdfs:comment xml:lang="en">CollisionRisk. Collision risk can be defined as the potential for UAS  to encounter and collide with other UAS, aircraft or obstacle.</rdfs:comment>
        <rdfs:label xml:lang="en">CollisionRisk</rdfs:label>
    </owl:Class>
    


    <!-- http://www.dronetology.net/dronetology#CombustionEngine -->

    <owl:Class rdf:about="http://www.dronetology.net/dronetology#CombustionEngine">
        <rdfs:subClassOf rdf:resource="http://www.dronetology.net/dronetology#Engine"/>
        <owl:disjointWith rdf:resource="http://www.dronetology.net/dronetology#ElectricalEngine"/>
        <rdfs:comment xml:lang="en">CombustionEngine. A heat engine in which the combustion of a fuel occurs with an oxidizer (usually air).</rdfs:comment>
        <rdfs:label xml:lang="en">CombustionEngine</rdfs:label>
    </owl:Class>
    


    <!-- http://www.dronetology.net/dronetology#Command -->

    <owl:Class rdf:about="http://www.dronetology.net/dronetology#Command">
        <rdfs:comment xml:lang="en">Command. A logical order, instruction or signal causing a computer or control unit to perform one of its basic functions.</rdfs:comment>
        <rdfs:label xml:lang="en">Command</rdfs:label>
    </owl:Class>
    


    <!-- http://www.dronetology.net/dronetology#CommunicationMessage -->

    <owl:Class rdf:about="http://www.dronetology.net/dronetology#CommunicationMessage">
        <rdfs:comment xml:lang="en">CommunicationMessage. A formal description of format and rules that allows to transmit information via any variation of a physical quantity.</rdfs:comment>
        <rdfs:label xml:lang="en">CommunicationMessage</rdfs:label>
    </owl:Class>
    


    <!-- http://www.dronetology.net/dronetology#CommunicationSystem -->

    <owl:Class rdf:about="http://www.dronetology.net/dronetology#CommunicationSystem">
        <rdfs:subClassOf rdf:resource="http://www.dronetology.net/dronetology#AircraftComponent"/>
        <owl:disjointWith rdf:resource="http://www.dronetology.net/dronetology#DataProcessingBoard"/>
        <owl:disjointWith rdf:resource="http://www.dronetology.net/dronetology#DataStorageDevice"/>
        <owl:disjointWith rdf:resource="http://www.dronetology.net/dronetology#EnergyStorageComponent"/>
        <owl:disjointWith rdf:resource="http://www.dronetology.net/dronetology#Engine"/>
        <owl:disjointWith rdf:resource="http://www.dronetology.net/dronetology#FlightControllerUnit"/>
        <owl:disjointWith rdf:resource="http://www.dronetology.net/dronetology#Fuselage"/>
        <owl:disjointWith rdf:resource="http://www.dronetology.net/dronetology#InertialNavigationUnit"/>
        <owl:disjointWith rdf:resource="http://www.dronetology.net/dronetology#LandingComponent"/>
        <owl:disjointWith rdf:resource="http://www.dronetology.net/dronetology#LiftGeneratorComponent"/>
        <owl:disjointWith rdf:resource="http://www.dronetology.net/dronetology#Payload"/>
        <rdfs:comment xml:lang="en">CommunicationSystem. A system which describes the information exchange between two points.</rdfs:comment>
        <rdfs:label xml:lang="en">CommunicationSystem</rdfs:label>
    </owl:Class>
    


    <!-- http://www.dronetology.net/dronetology#Component -->

    <owl:Class rdf:about="http://www.dronetology.net/dronetology#Component">
        <rdfs:comment xml:lang="en">Component. A part of the artifact being designed.</rdfs:comment>
        <rdfs:label xml:lang="en">Component</rdfs:label>
    </owl:Class>
    


    <!-- http://www.dronetology.net/dronetology#ComponentMalfunctionRisk -->

    <owl:Class rdf:about="http://www.dronetology.net/dronetology#ComponentMalfunctionRisk">
        <rdfs:subClassOf rdf:resource="http://www.dronetology.net/dronetology#Risk"/>
        <rdfs:comment xml:lang="en">ComponentMalfunctionRisk. Component failures risk due to  poor design, incorrect material selection, manufacturing defects or environmental factors.</rdfs:comment>
        <rdfs:label xml:lang="en">ComponentMalfunctionRisk</rdfs:label>
    </owl:Class>
    


    <!-- http://www.dronetology.net/dronetology#ComponentTemperature -->

    <owl:Class rdf:about="http://www.dronetology.net/dronetology#ComponentTemperature">
        <rdfs:subClassOf rdf:resource="http://qudt.org/schema/qudt/Quantity"/>
        <rdfs:comment xml:lang="en">ComponentTemperature. The degree or intensity of heat present in a drone component.</rdfs:comment>
        <rdfs:label xml:lang="en">ComponentTemperature</rdfs:label>
    </owl:Class>
    


    <!-- http://www.dronetology.net/dronetology#Conflict -->

    <owl:Class rdf:about="http://www.dronetology.net/dronetology#Conflict">
        <rdfs:subClassOf rdf:resource="http://www.opengis.net/ont/geosparql#Feature"/>
        <rdfs:comment>Conflict. A conflict is an infringement, or potential infringement, of the required separation between aircraft.</rdfs:comment>
        <rdfs:label xml:lang="en">Conflict</rdfs:label>
    </owl:Class>
    


    <!-- http://www.dronetology.net/dronetology#Connector -->

    <owl:Class rdf:about="http://www.dronetology.net/dronetology#Connector">
        <rdfs:subClassOf rdf:resource="http://www.dronetology.net/dronetology#AuxiliaryComponent"/>
        <rdfs:comment xml:lang="en">Connector. A device for keeping two parts of an electric circuit in contact.</rdfs:comment>
        <rdfs:label xml:lang="en">Connector</rdfs:label>
    </owl:Class>
    


    <!-- http://www.dronetology.net/dronetology#Constraint -->

    <owl:Class rdf:about="http://www.dronetology.net/dronetology#Constraint">
        <rdfs:comment xml:lang="en">Constraint. The leaves of the requirement decomposition tree, and embody physical laws, equations etc.</rdfs:comment>
        <rdfs:label xml:lang="en">Constraint</rdfs:label>
    </owl:Class>
    


    <!-- http://www.dronetology.net/dronetology#CooperativeDrone -->

    <owl:Class rdf:about="http://www.dronetology.net/dronetology#CooperativeDrone">
        <rdfs:subClassOf rdf:resource="http://www.dronetology.net/dronetology#Drone"/>
        <rdfs:comment xml:lang="en">CooperativeDrone. Drone with equipment that allows to cooperate with others.</rdfs:comment>
        <rdfs:label xml:lang="en">CooperativeDrone</rdfs:label>
    </owl:Class>
    


    <!-- http://www.dronetology.net/dronetology#Copter -->

    <owl:Class rdf:about="http://www.dronetology.net/dronetology#Copter">
        <rdfs:subClassOf rdf:resource="http://www.dronetology.net/dronetology#VTOLCraft"/>
        <rdfs:subClassOf>
            <owl:Restriction>
                <owl:onProperty rdf:resource="http://www.dronetology.net/dronetology#hasComponent"/>
                <owl:minQualifiedCardinality rdf:datatype="http://www.w3.org/2001/XMLSchema#nonNegativeInteger">1</owl:minQualifiedCardinality>
                <owl:onClass rdf:resource="http://www.dronetology.net/dronetology#Rotor"/>
            </owl:Restriction>
        </rdfs:subClassOf>
        <owl:disjointWith rdf:resource="http://www.dronetology.net/dronetology#FixedWingCraft"/>
        <rdfs:comment xml:lang="en">Copter. A type of aircraft which derives both lift and propulsion from one or more sets of horizontally revolving overhead rotors.</rdfs:comment>
        <rdfs:label xml:lang="en">Copter</rdfs:label>
    </owl:Class>
    


    <!-- http://www.dronetology.net/dronetology#CruisePlan -->

    <owl:Class rdf:about="http://www.dronetology.net/dronetology#CruisePlan">
        <rdfs:subClassOf rdf:resource="http://www.dronetology.net/dronetology#FlightPlan"/>
        <owl:disjointWith rdf:resource="http://www.dronetology.net/dronetology#LandingPlan"/>
        <owl:disjointWith rdf:resource="http://www.dronetology.net/dronetology#TakeoffPlan"/>
        <rdfs:comment xml:lang="en">CruisePlan. A part of the flightplan that starts when the aircraft levels off after a climb, until it begins to descend for landing.</rdfs:comment>
        <rdfs:label xml:lang="en">CruisePlan</rdfs:label>
    </owl:Class>
    


    <!-- http://www.dronetology.net/dronetology#CruiseSpeed -->

    <owl:Class rdf:about="http://www.dronetology.net/dronetology#CruiseSpeed">
        <rdfs:subClassOf rdf:resource="http://www.dronetology.net/dronetology#Speed"/>
        <rdfs:comment xml:lang="en">CruiseSpeed. The maximum speed at which a drone is able to travel continuously without using a large amount of energy.</rdfs:comment>
        <rdfs:label xml:lang="en">CruiseSpeed</rdfs:label>
    </owl:Class>
    


    <!-- http://www.dronetology.net/dronetology#DataLink -->

    <owl:Class rdf:about="http://www.dronetology.net/dronetology#DataLink">
        <rdfs:subClassOf rdf:resource="http://www.dronetology.net/dronetology#Component"/>
        <owl:disjointWith rdf:resource="http://www.dronetology.net/dronetology#HardwareComponent"/>
        <owl:disjointWith rdf:resource="http://www.dronetology.net/dronetology#SoftwareComponent"/>
        <rdfs:comment xml:lang="en">DataLink. A telecommunications link over which data is transmitted.</rdfs:comment>
        <rdfs:label xml:lang="en">DataLink</rdfs:label>
    </owl:Class>
    


    <!-- http://www.dronetology.net/dronetology#DataProcessingBoard -->

    <owl:Class rdf:about="http://www.dronetology.net/dronetology#DataProcessingBoard">
        <rdfs:subClassOf rdf:resource="http://www.dronetology.net/dronetology#AircraftComponent"/>
        <owl:disjointWith rdf:resource="http://www.dronetology.net/dronetology#DataStorageDevice"/>
        <owl:disjointWith rdf:resource="http://www.dronetology.net/dronetology#EnergyStorageComponent"/>
        <owl:disjointWith rdf:resource="http://www.dronetology.net/dronetology#Engine"/>
        <owl:disjointWith rdf:resource="http://www.dronetology.net/dronetology#FlightControllerUnit"/>
        <owl:disjointWith rdf:resource="http://www.dronetology.net/dronetology#Fuselage"/>
        <owl:disjointWith rdf:resource="http://www.dronetology.net/dronetology#InertialNavigationUnit"/>
        <owl:disjointWith rdf:resource="http://www.dronetology.net/dronetology#LandingComponent"/>
        <owl:disjointWith rdf:resource="http://www.dronetology.net/dronetology#LiftGeneratorComponent"/>
        <owl:disjointWith rdf:resource="http://www.dronetology.net/dronetology#Payload"/>
        <rdfs:comment xml:lang="en">DataProcessingBoard. Hardware dedicated to data and information processing.</rdfs:comment>
        <rdfs:label xml:lang="en">DataProcessingBoard</rdfs:label>
    </owl:Class>
    


    <!-- http://www.dronetology.net/dronetology#DataProcessingSystem -->

    <owl:Class rdf:about="http://www.dronetology.net/dronetology#DataProcessingSystem">
        <rdfs:subClassOf rdf:resource="http://www.dronetology.net/dronetology#GroundStationComponent"/>
        <owl:disjointWith rdf:resource="http://www.dronetology.net/dronetology#DataStorageSystem"/>
        <owl:disjointWith rdf:resource="http://www.dronetology.net/dronetology#GroundStationAntenna"/>
        <owl:disjointWith rdf:resource="http://www.dronetology.net/dronetology#GroundStationCommunicationSystem"/>
        <owl:disjointWith rdf:resource="http://www.dronetology.net/dronetology#MissionCommanderStation"/>
        <owl:disjointWith rdf:resource="http://www.dronetology.net/dronetology#PayloadOperatorStation"/>
        <owl:disjointWith rdf:resource="http://www.dronetology.net/dronetology#RemotePilotConsole"/>
        <rdfs:comment xml:lang="en">DataProcessingSystem. The data processing system implements a series of steps where raw data (input) is fed into a system to produce actionable insights (output).</rdfs:comment>
        <rdfs:label xml:lang="en">DataProcessingSystem</rdfs:label>
    </owl:Class>
    


    <!-- http://www.dronetology.net/dronetology#DataStorageDevice -->

    <owl:Class rdf:about="http://www.dronetology.net/dronetology#DataStorageDevice">
        <rdfs:subClassOf rdf:resource="http://www.dronetology.net/dronetology#AircraftComponent"/>
        <owl:disjointWith rdf:resource="http://www.dronetology.net/dronetology#EnergyStorageComponent"/>
        <owl:disjointWith rdf:resource="http://www.dronetology.net/dronetology#Engine"/>
        <owl:disjointWith rdf:resource="http://www.dronetology.net/dronetology#FlightControllerUnit"/>
        <owl:disjointWith rdf:resource="http://www.dronetology.net/dronetology#Fuselage"/>
        <owl:disjointWith rdf:resource="http://www.dronetology.net/dronetology#InertialNavigationUnit"/>
        <owl:disjointWith rdf:resource="http://www.dronetology.net/dronetology#LandingComponent"/>
        <owl:disjointWith rdf:resource="http://www.dronetology.net/dronetology#LiftGeneratorComponent"/>
        <owl:disjointWith rdf:resource="http://www.dronetology.net/dronetology#Payload"/>
        <rdfs:comment xml:lang="en">DataStorageDevice. Hardware that is used for storing, porting or extracting data files and objects.</rdfs:comment>
        <rdfs:label xml:lang="en">DataStorageDevice</rdfs:label>
    </owl:Class>
    


    <!-- http://www.dronetology.net/dronetology#DataStorageSystem -->

    <owl:Class rdf:about="http://www.dronetology.net/dronetology#DataStorageSystem">
        <rdfs:subClassOf rdf:resource="http://www.dronetology.net/dronetology#GroundStationComponent"/>
        <owl:disjointWith rdf:resource="http://www.dronetology.net/dronetology#GroundStationAntenna"/>
        <owl:disjointWith rdf:resource="http://www.dronetology.net/dronetology#GroundStationCommunicationSystem"/>
        <owl:disjointWith rdf:resource="http://www.dronetology.net/dronetology#MissionCommanderStation"/>
        <owl:disjointWith rdf:resource="http://www.dronetology.net/dronetology#PayloadOperatorStation"/>
        <owl:disjointWith rdf:resource="http://www.dronetology.net/dronetology#RemotePilotConsole"/>
        <rdfs:comment xml:lang="en">DataStorageSystem. Refers to magnetic, optical or mechanical media that records and preserves digital information for ongoing or future operations.</rdfs:comment>
        <rdfs:label xml:lang="en">DataStorageSystem</rdfs:label>
    </owl:Class>
    


    <!-- http://www.dronetology.net/dronetology#Dimension -->

    <owl:Class rdf:about="http://www.dronetology.net/dronetology#Dimension">
        <rdfs:subClassOf rdf:resource="http://qudt.org/schema/qudt/Quantity"/>
        <rdfs:comment xml:lang="en">Dimension. A measurable extent of a particular kind, such as length, breadth, depth, or height.</rdfs:comment>
        <rdfs:label xml:lang="en">Dimension</rdfs:label>
    </owl:Class>
    


    <!-- http://www.dronetology.net/dronetology#Direct_Remote_ID -->

    <owl:Class rdf:about="http://www.dronetology.net/dronetology#Direct_Remote_ID">
        <rdfs:subClassOf rdf:resource="http://www.dronetology.net/dronetology#RemoteID"/>
        <rdfs:comment xml:lang="en">Direct_Remote_ID. Direct Remote Identification.</rdfs:comment>
        <rdfs:label xml:lang="en">Direct_Remote_ID</rdfs:label>
    </owl:Class>
    


    <!-- http://www.dronetology.net/dronetology#Distance -->

    <owl:Class rdf:about="http://www.dronetology.net/dronetology#Distance">
        <rdfs:subClassOf rdf:resource="http://qudt.org/schema/qudt/Quantity"/>
        <rdfs:comment xml:lang="en">Distance.The length of the space between two points.</rdfs:comment>
        <rdfs:label xml:lang="en">Distance</rdfs:label>
    </owl:Class>
    


    <!-- http://www.dronetology.net/dronetology#Drone -->

    <owl:Class rdf:about="http://www.dronetology.net/dronetology#Drone">
        <rdfs:subClassOf rdf:resource="http://www.ontologydesignpatterns.org/ont/dul/DUL.owl#PhysicalObject"/>
        <owl:disjointWith rdf:resource="http://www.dronetology.net/dronetology#MannedAircraft"/>
        <rdfs:comment xml:lang="en">Drone. Unmanned aircraf remotely piloted or controlled autonomously .</rdfs:comment>
        <rdfs:label xml:lang="en">Drone</rdfs:label>
    </owl:Class>
    


    <!-- http://www.dronetology.net/dronetology#DualManufacturer -->

    <owl:Class rdf:about="http://www.dronetology.net/dronetology#DualManufacturer">
        <rdfs:subClassOf rdf:resource="http://www.dronetology.net/dronetology#Manufacturer"/>
        <owl:disjointUnionOf rdf:parseType="Collection">
            <rdf:Description rdf:about="http://www.dronetology.net/dronetology#CivilManufacturer"/>
            <rdf:Description rdf:about="http://www.dronetology.net/dronetology#MilitaryManufacturer"/>
        </owl:disjointUnionOf>
        <rdfs:comment>Dual Use Drone Manufacturers, produce drones for commercial and military markets.</rdfs:comment>
        <rdfs:label xml:lang="en">DualManufacturer</rdfs:label>
    </owl:Class>
    


    <!-- http://www.dronetology.net/dronetology#ElectricalEngine -->

    <owl:Class rdf:about="http://www.dronetology.net/dronetology#ElectricalEngine">
        <rdfs:subClassOf rdf:resource="http://www.dronetology.net/dronetology#Engine"/>
        <rdfs:comment xml:lang="en">ElectricalEngine. An electrical machine that converts electrical energy into mechanical energy.</rdfs:comment>
        <rdfs:label xml:lang="en">ElectricalEngine</rdfs:label>
    </owl:Class>
    


    <!-- http://www.dronetology.net/dronetology#ElectronicSpeedController -->

    <owl:Class rdf:about="http://www.dronetology.net/dronetology#ElectronicSpeedController">
        <rdfs:subClassOf rdf:resource="http://www.dronetology.net/dronetology#AircraftComponent"/>
        <owl:disjointWith rdf:resource="http://www.dronetology.net/dronetology#Payload"/>
        <rdfs:comment xml:lang="en">ElectronicSpeedController. An electronic circuit that controls and regulates the speed of an electric motor.</rdfs:comment>
        <rdfs:label xml:lang="en">ElectronicSpeedController</rdfs:label>
    </owl:Class>
    


    <!-- http://www.dronetology.net/dronetology#Elevator -->

    <owl:Class rdf:about="http://www.dronetology.net/dronetology#Elevator">
        <rdfs:subClassOf rdf:resource="http://www.dronetology.net/dronetology#WingComponent"/>
        <rdfs:comment xml:lang="en">Elevator. Positioned at the trailing edge of the horizontal stabilizer, the elevators control the pitch of the aircraft. By moving the elevators up or down, the pilot can raise or lower the nose of the plane, controlling its altitude.</rdfs:comment>
        <rdfs:label xml:lang="en">Elevator</rdfs:label>
    </owl:Class>
    


    <!-- http://www.dronetology.net/dronetology#EmergencyMission -->

    <owl:Class rdf:about="http://www.dronetology.net/dronetology#EmergencyMission">
        <rdfs:subClassOf rdf:resource="http://www.dronetology.net/dronetology#Mission"/>
        <rdfs:comment xml:lang="en">EmergencyMission. A mission with high priority.</rdfs:comment>
        <rdfs:label xml:lang="en">EmergencyMission</rdfs:label>
    </owl:Class>
    


    <!-- http://www.dronetology.net/dronetology#EnergyStorageComponent -->

    <owl:Class rdf:about="http://www.dronetology.net/dronetology#EnergyStorageComponent">
        <rdfs:subClassOf rdf:resource="http://www.dronetology.net/dronetology#AircraftComponent"/>
        <owl:disjointWith rdf:resource="http://www.dronetology.net/dronetology#Engine"/>
        <owl:disjointWith rdf:resource="http://www.dronetology.net/dronetology#FlightControllerUnit"/>
        <owl:disjointWith rdf:resource="http://www.dronetology.net/dronetology#Fuselage"/>
        <owl:disjointWith rdf:resource="http://www.dronetology.net/dronetology#InertialNavigationUnit"/>
        <owl:disjointWith rdf:resource="http://www.dronetology.net/dronetology#LandingComponent"/>
        <owl:disjointWith rdf:resource="http://www.dronetology.net/dronetology#LiftGeneratorComponent"/>
        <owl:disjointWith rdf:resource="http://www.dronetology.net/dronetology#Payload"/>
        <rdfs:comment xml:lang="en">EnergyStorageComponent. A device or group of devices assembled together, capable of storing energy.</rdfs:comment>
        <rdfs:label xml:lang="en">EnergyStorageComponent</rdfs:label>
    </owl:Class>
    


    <!-- http://www.dronetology.net/dronetology#Engine -->

    <owl:Class rdf:about="http://www.dronetology.net/dronetology#Engine">
        <rdfs:subClassOf rdf:resource="http://www.dronetology.net/dronetology#AircraftComponent"/>
        <owl:disjointWith rdf:resource="http://www.dronetology.net/dronetology#FlightControllerUnit"/>
        <owl:disjointWith rdf:resource="http://www.dronetology.net/dronetology#Fuselage"/>
        <owl:disjointWith rdf:resource="http://www.dronetology.net/dronetology#InertialNavigationUnit"/>
        <owl:disjointWith rdf:resource="http://www.dronetology.net/dronetology#LandingComponent"/>
        <owl:disjointWith rdf:resource="http://www.dronetology.net/dronetology#LiftGeneratorComponent"/>
        <owl:disjointWith rdf:resource="http://www.dronetology.net/dronetology#Payload"/>
        <rdfs:comment xml:lang="en">Engine. A machine for converting any of various forms of energy into mechanical force and motion.</rdfs:comment>
        <rdfs:label xml:lang="en">Engine</rdfs:label>
    </owl:Class>
    


    <!-- http://www.dronetology.net/dronetology#ExternalSensor -->

    <owl:Class rdf:about="http://www.dronetology.net/dronetology#ExternalSensor">
        <rdfs:subClassOf rdf:resource="http://www.w3.org/ns/ssn/SensingDevice"/>
        <owl:disjointWith rdf:resource="http://www.dronetology.net/dronetology#OnboardSensor"/>
        <rdfs:comment>Sensors located outside the aircraft.</rdfs:comment>
        <rdfs:label xml:lang="en">ExternalSensor</rdfs:label>
    </owl:Class>
    


    <!-- http://www.dronetology.net/dronetology#Feature -->

    <owl:Class rdf:about="http://www.dronetology.net/dronetology#Feature">
        <rdfs:comment xml:lang="en">Feature. A feature is used to describe geometrical, functional and other characteristics associated with a part.</rdfs:comment>
        <rdfs:label xml:lang="en">Feature</rdfs:label>
    </owl:Class>
    


    <!-- http://www.dronetology.net/dronetology#FireRisk -->

    <owl:Class rdf:about="http://www.dronetology.net/dronetology#FireRisk">
        <rdfs:subClassOf rdf:resource="http://www.dronetology.net/dronetology#Risk"/>
        <rdfs:isDefinedBy xml:lang="en">FireRisk. Risk of harm to property or people due to fire provoked by a UAS</rdfs:isDefinedBy>
        <rdfs:label xml:lang="en">FireRisk</rdfs:label>
    </owl:Class>
    


    <!-- http://www.dronetology.net/dronetology#FixedWingCraft -->

    <owl:Class rdf:about="http://www.dronetology.net/dronetology#FixedWingCraft">
        <rdfs:subClassOf rdf:resource="http://www.dronetology.net/dronetology#Drone"/>
        <rdfs:subClassOf>
            <owl:Restriction>
                <owl:onProperty rdf:resource="http://www.dronetology.net/dronetology#hasComponent"/>
                <owl:minQualifiedCardinality rdf:datatype="http://www.w3.org/2001/XMLSchema#nonNegativeInteger">1</owl:minQualifiedCardinality>
                <owl:onClass rdf:resource="http://www.dronetology.net/dronetology#Wing"/>
            </owl:Restriction>
        </rdfs:subClassOf>
        <rdfs:comment xml:lang="en">FixedWingCraft. An aircraft with wings that stay in the same position.</rdfs:comment>
        <rdfs:label xml:lang="en">FixedWingCraft</rdfs:label>
    </owl:Class>
    


    <!-- http://www.dronetology.net/dronetology#FixedWingVTOLCraft -->

    <owl:Class rdf:about="http://www.dronetology.net/dronetology#FixedWingVTOLCraft">
        <rdfs:subClassOf rdf:resource="http://www.dronetology.net/dronetology#FixedWingCraft"/>
        <rdfs:subClassOf rdf:resource="http://www.dronetology.net/dronetology#VTOLCraft"/>
        <rdfs:comment xml:lang="en">FixedWingVTOLCraft. An aircraft with wings that stay in the same position but can take off and land vertically without relying on a runway.</rdfs:comment>
        <rdfs:label xml:lang="en">FixedWingVTOLCraft</rdfs:label>
    </owl:Class>
    


    <!-- http://www.dronetology.net/dronetology#Flap -->

    <owl:Class rdf:about="http://www.dronetology.net/dronetology#Flap">
        <rdfs:subClassOf rdf:resource="http://www.dronetology.net/dronetology#WingComponent"/>
        <rdfs:comment xml:lang="en">Flap. The flaps are found along the trailing edge of the wing, closer to the fuselage. They are used to increase the lift of the wing during takeoff and landing, allowing the aircraft to fly at slower speeds.</rdfs:comment>
        <rdfs:label xml:lang="en">Flap</rdfs:label>
    </owl:Class>
    


    <!-- http://www.dronetology.net/dronetology#FlightAreaMission -->

    <owl:Class rdf:about="http://www.dronetology.net/dronetology#FlightAreaMission">
        <rdfs:subClassOf rdf:resource="http://www.dronetology.net/dronetology#Mission"/>
        <rdfs:comment xml:lang="en">FlightAreaMission. A mission defined by a fligh area.</rdfs:comment>
        <rdfs:label xml:lang="en">FlightAreaMission</rdfs:label>
    </owl:Class>
    


    <!-- http://www.dronetology.net/dronetology#FlightControlApp -->

    <owl:Class rdf:about="http://www.dronetology.net/dronetology#FlightControlApp">
        <rdfs:subClassOf rdf:resource="http://www.dronetology.net/dronetology#SoftwareComponent"/>
        <rdfs:comment xml:lang="en">FlightControlApp. A software installed on a mobile device that allows the pilot to control the drone and to manage data from the mission.</rdfs:comment>
        <rdfs:label xml:lang="en">FlightControlApp</rdfs:label>
    </owl:Class>
    


    <!-- http://www.dronetology.net/dronetology#FlightControlFirmware -->

    <owl:Class rdf:about="http://www.dronetology.net/dronetology#FlightControlFirmware">
        <rdfs:subClassOf rdf:resource="http://www.dronetology.net/dronetology#SoftwareComponent"/>
        <rdfs:comment xml:lang="en">FlightControlFirmware. The software that runs on the drone flight controller and defines its features, settings, and capabilities.</rdfs:comment>
        <rdfs:label xml:lang="en">FlightControlFirmware</rdfs:label>
    </owl:Class>
    


    <!-- http://www.dronetology.net/dronetology#FlightControllerUnit -->

    <owl:Class rdf:about="http://www.dronetology.net/dronetology#FlightControllerUnit">
        <rdfs:subClassOf rdf:resource="http://www.dronetology.net/dronetology#AircraftComponent"/>
        <owl:disjointWith rdf:resource="http://www.dronetology.net/dronetology#Fuselage"/>
        <owl:disjointWith rdf:resource="http://www.dronetology.net/dronetology#InertialNavigationUnit"/>
        <owl:disjointWith rdf:resource="http://www.dronetology.net/dronetology#LandingComponent"/>
        <owl:disjointWith rdf:resource="http://www.dronetology.net/dronetology#LiftGeneratorComponent"/>
        <owl:disjointWith rdf:resource="http://www.dronetology.net/dronetology#Payload"/>
        <rdfs:comment xml:lang="en">FlightControllerUnit. Controls the motors and ESCs in the drone to fly following the pilot commands or a stored flight plan.</rdfs:comment>
        <rdfs:label xml:lang="en">FlighControllerUnit</rdfs:label>
    </owl:Class>
    


    <!-- http://www.dronetology.net/dronetology#FlightPlan -->

    <owl:Class rdf:about="http://www.dronetology.net/dronetology#FlightPlan">
        <rdfs:subClassOf>
            <owl:Class>
                <owl:intersectionOf rdf:parseType="Collection">
                    <owl:Restriction>
                        <owl:onProperty rdf:resource="http://www.dronetology.net/dronetology#hasWaypoint"/>
                        <owl:minQualifiedCardinality rdf:datatype="http://www.w3.org/2001/XMLSchema#nonNegativeInteger">1</owl:minQualifiedCardinality>
                        <owl:onClass rdf:resource="http://www.dronetology.net/dronetology#Waypoint"/>
                    </owl:Restriction>
                    <owl:Restriction>
                        <owl:onProperty rdf:resource="http://www.dronetology.net/dronetology#hasWaypoint"/>
                        <owl:qualifiedCardinality rdf:datatype="http://www.w3.org/2001/XMLSchema#nonNegativeInteger">1</owl:qualifiedCardinality>
                        <owl:onClass rdf:resource="http://www.dronetology.net/dronetology#HomeLocation"/>
                    </owl:Restriction>
                </owl:intersectionOf>
            </owl:Class>
        </rdfs:subClassOf>
        <rdfs:comment xml:lang="en">FlightPlan. A flightplan defines the details of an intended flight.</rdfs:comment>
        <rdfs:label xml:lang="en">FlightPlan</rdfs:label>
    </owl:Class>
    


    <!-- http://www.dronetology.net/dronetology#FlightSegments -->

    <owl:Class rdf:about="http://www.dronetology.net/dronetology#FlightSegments">
        <rdfs:subClassOf rdf:resource="http://www.dronetology.net/dronetology#MissionGeometryElement"/>
        <rdfs:subClassOf>
            <owl:Restriction>
                <owl:onProperty rdf:resource="http://www.dronetology.net/dronetology#hasWaypoint"/>
                <owl:minQualifiedCardinality rdf:datatype="http://www.w3.org/2001/XMLSchema#nonNegativeInteger">2</owl:minQualifiedCardinality>
                <owl:onClass rdf:resource="http://www.dronetology.net/dronetology#Waypoint"/>
            </owl:Restriction>
        </rdfs:subClassOf>
        <rdfs:comment xml:lang="en">FlightSegments. The fly path between two wayopints.</rdfs:comment>
        <rdfs:label xml:lang="en">FlightSegments</rdfs:label>
    </owl:Class>
    


    <!-- http://www.dronetology.net/dronetology#FlightTime -->

    <owl:Class rdf:about="http://www.dronetology.net/dronetology#FlightTime">
        <rdfs:subClassOf rdf:resource="http://qudt.org/schema/qudt/Quantity"/>
        <rdfs:comment xml:lang="en">FlightTime. The time from the moment a drone leaves the surface until it comes into contact with the surface at the next point of landing</rdfs:comment>
        <rdfs:label xml:lang="en">FlighTime</rdfs:label>
    </owl:Class>
    


    <!-- http://www.dronetology.net/dronetology#FlyZone -->

    <owl:Class rdf:about="http://www.dronetology.net/dronetology#FlyZone">
        <rdfs:subClassOf rdf:resource="http://www.dronetology.net/dronetology#AirSpaceVolume"/>
        <owl:disjointWith rdf:resource="http://www.dronetology.net/dronetology#NoFlyZone"/>
        <rdfs:comment xml:lang="en">FlyZone. Part of the airspace available to aircraft to fly in.</rdfs:comment>
        <rdfs:label xml:lang="en">FlyZone</rdfs:label>
    </owl:Class>
    


    <!-- http://www.dronetology.net/dronetology#ForcedLandingRisk -->

    <owl:Class rdf:about="http://www.dronetology.net/dronetology#ForcedLandingRisk">
        <rdfs:subClassOf rdf:resource="http://www.dronetology.net/dronetology#Risk"/>
        <rdfs:comment xml:lang="en">ForcedLandingRisk. A forced landing, on or off an airport, necessitated by the inability to continue further flight.</rdfs:comment>
        <rdfs:label xml:lang="en">ForcedLandingRisk</rdfs:label>
    </owl:Class>
    


    <!-- http://www.dronetology.net/dronetology#FrameKit -->

    <owl:Class rdf:about="http://www.dronetology.net/dronetology#FrameKit">
        <rdfs:subClassOf rdf:resource="http://www.dronetology.net/dronetology#Fuselage"/>
        <owl:disjointWith rdf:resource="http://www.dronetology.net/dronetology#Nose"/>
        <owl:disjointWith rdf:resource="http://www.dronetology.net/dronetology#Tail"/>
        <rdfs:comment xml:lang="en">FrameKit. The main structure in a drone where the rest of the components are installed.</rdfs:comment>
        <rdfs:label xml:lang="en">FrameKit</rdfs:label>
    </owl:Class>
    


    <!-- http://www.dronetology.net/dronetology#FuelTank -->

    <owl:Class rdf:about="http://www.dronetology.net/dronetology#FuelTank">
        <rdfs:subClassOf rdf:resource="http://www.dronetology.net/dronetology#EnergyStorageComponent"/>
        <rdfs:comment xml:lang="en">FuelTank. A container inside a vehicle that holds fuel.</rdfs:comment>
        <rdfs:label xml:lang="en">FuelTank</rdfs:label>
    </owl:Class>
    


    <!-- http://www.dronetology.net/dronetology#Function -->

    <owl:Class rdf:about="http://www.dronetology.net/dronetology#Function">
        <rdfs:comment xml:lang="en">Function. Drones have many functions, ranging from monitoring climate change to carrying out search operations after natural disasters, photography, filming, etc.</rdfs:comment>
        <rdfs:label xml:lang="en">Function</rdfs:label>
    </owl:Class>
    


    <!-- http://www.dronetology.net/dronetology#Fuselage -->

    <owl:Class rdf:about="http://www.dronetology.net/dronetology#Fuselage">
        <rdfs:subClassOf rdf:resource="http://www.dronetology.net/dronetology#AircraftComponent"/>
        <owl:disjointWith rdf:resource="http://www.dronetology.net/dronetology#InertialNavigationUnit"/>
        <owl:disjointWith rdf:resource="http://www.dronetology.net/dronetology#LandingComponent"/>
        <owl:disjointWith rdf:resource="http://www.dronetology.net/dronetology#LiftGeneratorComponent"/>
        <owl:disjointWith rdf:resource="http://www.dronetology.net/dronetology#Payload"/>
        <rdfs:comment xml:lang="en">Fuselage. The central body portion of an aircraft.</rdfs:comment>
        <rdfs:label xml:lang="en">Fuselage</rdfs:label>
    </owl:Class>
    


    <!-- http://www.dronetology.net/dronetology#GLONASS -->

    <owl:Class rdf:about="http://www.dronetology.net/dronetology#GLONASS">
        <rdfs:subClassOf rdf:resource="http://www.dronetology.net/dronetology#GlobalNavigationSatelliteSystem"/>
        <rdfs:comment>GLONASS. GLONASS (Globalnaya Navigazionnaya Sputnikovaya Sistema, or Global Navigation Satellite System) is a global GNSS owned and operated by the Russian Federation. The fully operational system consists of 24+ satellites.</rdfs:comment>
        <rdfs:label xml:lang="en">GLONASS</rdfs:label>
    </owl:Class>
    


    <!-- http://www.dronetology.net/dronetology#GPS -->

    <owl:Class rdf:about="http://www.dronetology.net/dronetology#GPS">
        <rdfs:subClassOf rdf:resource="http://www.dronetology.net/dronetology#GlobalNavigationSatelliteSystem"/>
        <rdfs:comment xml:lang="en">GPS. Global positioning system is a space-based navigation system owned by the US government and operated by the US Air Force that consists of satellites, receivers and other technologies that provide accurate location and time information for civil and military use.</rdfs:comment>
        <rdfs:label xml:lang="en">GPS</rdfs:label>
    </owl:Class>
    


    <!-- http://www.dronetology.net/dronetology#Galileo -->

    <owl:Class rdf:about="http://www.dronetology.net/dronetology#Galileo">
        <rdfs:subClassOf rdf:resource="http://www.dronetology.net/dronetology#GlobalNavigationSatelliteSystem"/>
        <rdfs:comment xml:lang="en">Galileo. Galileo is a global GNSS owned and operated by the European Union.</rdfs:comment>
        <rdfs:label xml:lang="en">Galileo</rdfs:label>
    </owl:Class>
    


    <!-- http://www.dronetology.net/dronetology#GearBox -->

    <owl:Class rdf:about="http://www.dronetology.net/dronetology#GearBox">
        <rdfs:subClassOf rdf:resource="http://www.dronetology.net/dronetology#RotorComponent"/>
        <owl:disjointWith rdf:resource="http://www.dronetology.net/dronetology#Propeller"/>
        <owl:disjointWith rdf:resource="http://www.dronetology.net/dronetology#Rotor"/>
        <rdfs:comment xml:lang="en">GearBox.  A set of gears and their casing to transferr energy from one device to another.</rdfs:comment>
        <rdfs:label xml:lang="en">GearBox</rdfs:label>
    </owl:Class>
    


    <!-- http://www.dronetology.net/dronetology#Gimbal -->

    <owl:Class rdf:about="http://www.dronetology.net/dronetology#Gimbal">
        <rdfs:subClassOf rdf:resource="http://www.dronetology.net/dronetology#Payload"/>
        <rdfs:comment xml:lang="en">Gimbal.  This part of the drone is for stabilising the camera during drone flight to prevent the vibrations of the motors from affecting the quality of the images captured with the drone.</rdfs:comment>
        <rdfs:label xml:lang="en">Gimbal</rdfs:label>
    </owl:Class>
    


    <!-- http://www.dronetology.net/dronetology#GlobalNavigationSatelliteSystem -->

    <owl:Class rdf:about="http://www.dronetology.net/dronetology#GlobalNavigationSatelliteSystem">
        <rdfs:subClassOf rdf:resource="http://www.dronetology.net/dronetology#AircraftComponent"/>
        <rdfs:comment xml:lang="en">GlobalNavigationSatelliteSystem. Global navigation satellite system (GNSS) is a general term describing any satellite constellation that provides positioning, navigation, and timing (PNT) services on a global or regional basis.</rdfs:comment>
        <rdfs:label xml:lang="en">GlobalNavigationSatelliteSystem</rdfs:label>
    </owl:Class>
    


    <!-- http://www.dronetology.net/dronetology#GoToCommand -->

    <owl:Class rdf:about="http://www.dronetology.net/dronetology#GoToCommand">
        <rdfs:subClassOf rdf:resource="http://www.dronetology.net/dronetology#Command"/>
        <owl:disjointWith>
            <owl:Class>
                <owl:unionOf rdf:parseType="Collection">
                    <rdf:Description rdf:about="http://www.dronetology.net/dronetology#AuxiliaryCommand"/>
                    <rdf:Description rdf:about="http://www.dronetology.net/dronetology#NEDVelocityCommand"/>
                </owl:unionOf>
            </owl:Class>
        </owl:disjointWith>
        <rdfs:comment xml:lang="en">GoToCommand. A command that order the UAS to go a specific location.</rdfs:comment>
        <rdfs:label xml:lang="en">GoToCommand</rdfs:label>
    </owl:Class>
    


    <!-- http://www.dronetology.net/dronetology#GroundStation -->

    <owl:Class rdf:about="http://www.dronetology.net/dronetology#GroundStation">
        <rdfs:subClassOf rdf:resource="http://www.dronetology.net/dronetology#HardwareComponent"/>
        <owl:disjointWith rdf:resource="http://www.dronetology.net/dronetology#GroundStationComponent"/>
        <owl:disjointWith rdf:resource="http://www.dronetology.net/dronetology#LaunchSystem"/>
        <rdfs:comment xml:lang="en">GroundStation. Land-based communications and control systems typically used for direct piloting and communication between the crew and a UAV.</rdfs:comment>
        <rdfs:label xml:lang="en">GroundStation</rdfs:label>
    </owl:Class>
    


    <!-- http://www.dronetology.net/dronetology#GroundStationAntenna -->

    <owl:Class rdf:about="http://www.dronetology.net/dronetology#GroundStationAntenna">
        <rdfs:subClassOf rdf:resource="http://www.dronetology.net/dronetology#GroundStationComponent"/>
        <owl:disjointWith rdf:resource="http://www.dronetology.net/dronetology#GroundStationCommunicationSystem"/>
        <owl:disjointWith rdf:resource="http://www.dronetology.net/dronetology#MissionCommanderStation"/>
        <owl:disjointWith rdf:resource="http://www.dronetology.net/dronetology#PayloadOperatorStation"/>
        <owl:disjointWith rdf:resource="http://www.dronetology.net/dronetology#RemotePilotConsole"/>
        <rdfs:comment xml:lang="en">GroundStationAntenna. Antenna installed in the ground station.</rdfs:comment>
        <rdfs:label xml:lang="en">GroundStationAntenna</rdfs:label>
    </owl:Class>
    


    <!-- http://www.dronetology.net/dronetology#GroundStationCommunicationSystem -->

    <owl:Class rdf:about="http://www.dronetology.net/dronetology#GroundStationCommunicationSystem">
        <rdfs:subClassOf rdf:resource="http://www.dronetology.net/dronetology#GroundStationComponent"/>
        <owl:disjointWith rdf:resource="http://www.dronetology.net/dronetology#MissionCommanderStation"/>
        <owl:disjointWith rdf:resource="http://www.dronetology.net/dronetology#PayloadOperatorStation"/>
        <owl:disjointWith rdf:resource="http://www.dronetology.net/dronetology#RemotePilotConsole"/>
        <rdfs:comment xml:lang="en">GroundStationCommunicationSystem. Communication systems used to communicate with the drone.</rdfs:comment>
        <rdfs:label xml:lang="en">GroundStationCommunicationSystem</rdfs:label>
    </owl:Class>
    


    <!-- http://www.dronetology.net/dronetology#GroundStationComponent -->

    <owl:Class rdf:about="http://www.dronetology.net/dronetology#GroundStationComponent">
        <rdfs:subClassOf rdf:resource="http://www.dronetology.net/dronetology#HardwareComponent"/>
        <owl:disjointWith rdf:resource="http://www.dronetology.net/dronetology#LaunchSystem"/>
        <rdfs:comment xml:lang="en">GroundStationComponent. Any component of the ground station.</rdfs:comment>
        <rdfs:label xml:lang="en">GroundStationComponent</rdfs:label>
    </owl:Class>
    


    <!-- http://www.dronetology.net/dronetology#Group1 -->

    <owl:Class rdf:about="http://www.dronetology.net/dronetology#Group1">
        <rdfs:subClassOf rdf:resource="http://www.dronetology.net/dronetology#Drone"/>
        <rdfs:comment xml:lang="en">Group1. A drone-category for small drone defined by the U.S. Department of Defense (DoD).</rdfs:comment>
        <rdfs:label xml:lang="en">Group1</rdfs:label>
    </owl:Class>
    


    <!-- http://www.dronetology.net/dronetology#Group2 -->

    <owl:Class rdf:about="http://www.dronetology.net/dronetology#Group2">
        <rdfs:subClassOf rdf:resource="http://www.dronetology.net/dronetology#Drone"/>
        <rdfs:comment xml:lang="en">Group2. A drone-category for medium drone defined by the U.S. Department of Defense (DoD).</rdfs:comment>
        <rdfs:label xml:lang="en">Group2</rdfs:label>
    </owl:Class>
    


    <!-- http://www.dronetology.net/dronetology#Group3 -->

    <owl:Class rdf:about="http://www.dronetology.net/dronetology#Group3">
        <rdfs:subClassOf rdf:resource="http://www.dronetology.net/dronetology#Drone"/>
        <rdfs:comment xml:lang="en">Group3. A drone-category for large drone defined by the U.S. Department of Defense (DoD).</rdfs:comment>
        <rdfs:label xml:lang="en">Group3</rdfs:label>
    </owl:Class>
    


    <!-- http://www.dronetology.net/dronetology#Group4 -->

    <owl:Class rdf:about="http://www.dronetology.net/dronetology#Group4">
        <rdfs:subClassOf rdf:resource="http://www.dronetology.net/dronetology#Drone"/>
        <rdfs:comment xml:lang="en">Group4. A drone-category for larger drone defined by the U.S. Department of Defense (DoD).</rdfs:comment>
        <rdfs:label xml:lang="en">Group4</rdfs:label>
    </owl:Class>
    


    <!-- http://www.dronetology.net/dronetology#Group5 -->

    <owl:Class rdf:about="http://www.dronetology.net/dronetology#Group5">
        <rdfs:subClassOf rdf:resource="http://www.dronetology.net/dronetology#Drone"/>
        <rdfs:comment xml:lang="en">Group5. A drone-category for the largest drone defined by the U.S. Department of Defense (DoD).</rdfs:comment>
        <rdfs:label xml:lang="en">Group5</rdfs:label>
    </owl:Class>
    


    <!-- http://www.dronetology.net/dronetology#Gyroscope -->

    <owl:Class rdf:about="http://www.dronetology.net/dronetology#Gyroscope">
        <rdfs:subClassOf rdf:resource="http://www.dronetology.net/dronetology#InertialNavigationUnit"/>
        <rdfs:comment xml:lang="en">Gyroscope. A gyroscope is a sensor that measures rotational movement and provides feedback to maintain stability in an aircraft.</rdfs:comment>
        <rdfs:label xml:lang="en">Gyroscope</rdfs:label>
    </owl:Class>
    


    <!-- http://www.dronetology.net/dronetology#HALE -->

    <owl:Class rdf:about="http://www.dronetology.net/dronetology#HALE">
        <rdfs:subClassOf rdf:resource="http://www.dronetology.net/dronetology#Drone"/>
        <rdfs:comment xml:lang="en">HALE. High-Altitude Long Endurance drone.</rdfs:comment>
        <rdfs:label xml:lang="en">HALE</rdfs:label>
    </owl:Class>
    


    <!-- http://www.dronetology.net/dronetology#HardwareComponent -->

    <owl:Class rdf:about="http://www.dronetology.net/dronetology#HardwareComponent">
        <rdfs:subClassOf rdf:resource="http://www.dronetology.net/dronetology#Component"/>
        <rdfs:subClassOf rdf:resource="http://www.ontologydesignpatterns.org/ont/dul/DUL.owl#PhysicalObject"/>
        <owl:disjointWith rdf:resource="http://www.dronetology.net/dronetology#SoftwareComponent"/>
        <rdfs:comment xml:lang="en">HardwareComponent. Hardware component.</rdfs:comment>
        <rdfs:label xml:lang="en">HardwareComponent</rdfs:label>
    </owl:Class>
    


    <!-- http://www.dronetology.net/dronetology#Height -->

    <owl:Class rdf:about="http://www.dronetology.net/dronetology#Height">
        <rdfs:subClassOf rdf:resource="http://qudt.org/schema/qudt/Quantity"/>
        <rdfs:comment xml:lang="en">Height. The vertical distance of a drone above whatever surface.</rdfs:comment>
        <rdfs:label xml:lang="en">Height</rdfs:label>
    </owl:Class>
    


    <!-- http://www.dronetology.net/dronetology#HighImpact -->

    <owl:Class rdf:about="http://www.dronetology.net/dronetology#HighImpact">
        <rdfs:subClassOf rdf:resource="http://www.dronetology.net/dronetology#RiskImpact"/>
        <rdfs:comment xml:lang="en">HighImpact. High-impact risks are those that have a significant probability of occurring and a large negative effect on a UAS flight.</rdfs:comment>
        <rdfs:label xml:lang="en">HighImpact</rdfs:label>
    </owl:Class>
    


    <!-- http://www.dronetology.net/dronetology#HighLikelihood -->

    <owl:Class rdf:about="http://www.dronetology.net/dronetology#HighLikelihood">
        <rdfs:subClassOf rdf:resource="http://www.dronetology.net/dronetology#RiskLikelihood"/>
        <rdfs:comment xml:lang="en">HighLikelihood. A high level of probability the risk will occur or be realized.</rdfs:comment>
        <rdfs:label xml:lang="en">HighLikelihood</rdfs:label>
    </owl:Class>
    


    <!-- http://www.dronetology.net/dronetology#HighPriorityMission -->

    <owl:Class rdf:about="http://www.dronetology.net/dronetology#HighPriorityMission">
        <rdfs:subClassOf rdf:resource="http://www.dronetology.net/dronetology#MissionPriority"/>
        <rdfs:comment xml:lang="en">HighPriorityMission. Immediate mission that takes precedence over others.</rdfs:comment>
        <rdfs:label xml:lang="en">HighPriorityMission</rdfs:label>
    </owl:Class>
    


    <!-- http://www.dronetology.net/dronetology#HomeLocation -->

    <owl:Class rdf:about="http://www.dronetology.net/dronetology#HomeLocation">
        <rdfs:subClassOf rdf:resource="http://www.dronetology.net/dronetology#Waypoint"/>
    </owl:Class>
    


    <!-- http://www.dronetology.net/dronetology#IRNSS -->

    <owl:Class rdf:about="http://www.dronetology.net/dronetology#IRNSS">
        <rdfs:subClassOf rdf:resource="http://www.dronetology.net/dronetology#GlobalNavigationSatelliteSystem"/>
        <rdfs:comment xml:lang="en">IRNSS. IRNSS is a regional GNSS owned and operated by the Government of India. IRNSS is an autonomous system designed to cover the Indian region and 1500 km around the Indian mainland.</rdfs:comment>
        <rdfs:label xml:lang="en">IRNSS</rdfs:label>
    </owl:Class>
    


    <!-- http://www.dronetology.net/dronetology#InertialNavigationUnit -->

    <owl:Class rdf:about="http://www.dronetology.net/dronetology#InertialNavigationUnit">
        <rdfs:subClassOf rdf:resource="http://www.dronetology.net/dronetology#AircraftComponent"/>
        <owl:disjointWith rdf:resource="http://www.dronetology.net/dronetology#LandingComponent"/>
        <owl:disjointWith rdf:resource="http://www.dronetology.net/dronetology#LiftGeneratorComponent"/>
        <owl:disjointWith rdf:resource="http://www.dronetology.net/dronetology#Payload"/>
        <rdfs:comment xml:lang="en">InertialNavigationUnit. The INS provides the drone with data on linear acceleration across three axes, as well as measurements of pitch, roll, and yaw.</rdfs:comment>
        <rdfs:label xml:lang="en">InertialNavigationUnit</rdfs:label>
    </owl:Class>
    


    <!-- http://www.dronetology.net/dronetology#InjuryRisk -->

    <owl:Class rdf:about="http://www.dronetology.net/dronetology#InjuryRisk">
        <rdfs:subClassOf rdf:resource="http://www.dronetology.net/dronetology#Risk"/>
        <rdfs:comment xml:lang="en">InjuryRisk. Risk of injury means a risk of death or personal injury provoked by a UAS.</rdfs:comment>
        <rdfs:label xml:lang="en">InjuryRisk</rdfs:label>
    </owl:Class>
    


    <!-- http://www.dronetology.net/dronetology#InterComponentMessage -->

    <owl:Class rdf:about="http://www.dronetology.net/dronetology#InterComponentMessage">
        <rdfs:subClassOf rdf:resource="http://www.dronetology.net/dronetology#CommunicationMessage"/>
        <rdfs:comment xml:lang="en">InterComponentMessage. A message used internally between drone components.</rdfs:comment>
        <rdfs:label xml:lang="en">InterComponentMessage</rdfs:label>
    </owl:Class>
    


    <!-- http://www.dronetology.net/dronetology#InventorySoftware -->

    <owl:Class rdf:about="http://www.dronetology.net/dronetology#InventorySoftware">
        <rdfs:subClassOf rdf:resource="http://www.dronetology.net/dronetology#SoftwareComponent"/>
        <rdfs:comment xml:lang="en">InventorySoftware. A business applications that are designed to track and manage drone product, material purchases, delivery of goods, etc.</rdfs:comment>
        <rdfs:label xml:lang="en">InventorySoftware</rdfs:label>
    </owl:Class>
    


    <!-- http://www.dronetology.net/dronetology#Iteration -->

    <owl:Class rdf:about="http://www.dronetology.net/dronetology#Iteration">
        <rdfs:subClassOf rdf:resource="http://www.dronetology.net/dronetology#MissionTemporalElement"/>
        <rdfs:comment xml:lang="en">Iteration. An auto-incremental number that increases in each repetition of a computational procedure that involves Dronetology during a mission.</rdfs:comment>
        <rdfs:label xml:lang="en">Iteration</rdfs:label>
    </owl:Class>
    


    <!-- http://www.dronetology.net/dronetology#LALE -->

    <owl:Class rdf:about="http://www.dronetology.net/dronetology#LALE">
        <rdfs:subClassOf rdf:resource="http://www.dronetology.net/dronetology#Drone"/>
        <rdfs:comment xml:lang="en">LALE. Low Altitude Large Endurance drone.</rdfs:comment>
        <rdfs:label xml:lang="en">LALE</rdfs:label>
    </owl:Class>
    


    <!-- http://www.dronetology.net/dronetology#LASE -->

    <owl:Class rdf:about="http://www.dronetology.net/dronetology#LASE">
        <rdfs:subClassOf rdf:resource="http://www.dronetology.net/dronetology#Drone"/>
        <rdfs:comment xml:lang="en">LASE. Low Altitude Short Endurance drone.</rdfs:comment>
        <rdfs:label xml:lang="en">LASE</rdfs:label>
    </owl:Class>
    


    <!-- http://www.dronetology.net/dronetology#LandingComponent -->

    <owl:Class rdf:about="http://www.dronetology.net/dronetology#LandingComponent">
        <rdfs:subClassOf rdf:resource="http://www.dronetology.net/dronetology#AircraftComponent"/>
        <owl:disjointWith rdf:resource="http://www.dronetology.net/dronetology#LiftGeneratorComponent"/>
        <owl:disjointWith rdf:resource="http://www.dronetology.net/dronetology#Payload"/>
        <rdfs:comment xml:lang="en">LandingComponent. This is one of the most important parts to ensure the integrity of the drone when it comes into contact with the ground.</rdfs:comment>
        <rdfs:label xml:lang="en">LandingComponent</rdfs:label>
    </owl:Class>
    


    <!-- http://www.dronetology.net/dronetology#LandingGear -->

    <owl:Class rdf:about="http://www.dronetology.net/dronetology#LandingGear">
        <rdfs:subClassOf rdf:resource="http://www.dronetology.net/dronetology#LandingComponent"/>
        <rdfs:comment xml:lang="en">LandingGear. A structure that goes on the bottom of the drone, which allows you to maintain an adequate distance between the body of the drone and the ground. Synonym of landing leg.</rdfs:comment>
        <rdfs:label xml:lang="en">LandingGear</rdfs:label>
    </owl:Class>
    


    <!-- http://www.dronetology.net/dronetology#LandingPlan -->

    <owl:Class rdf:about="http://www.dronetology.net/dronetology#LandingPlan">
        <rdfs:subClassOf rdf:resource="http://www.dronetology.net/dronetology#FlightPlan"/>
        <owl:disjointWith rdf:resource="http://www.dronetology.net/dronetology#TakeoffPlan"/>
        <rdfs:comment xml:lang="en">LandingPlan. A part of the flightplan that starts when the aircraft is climbing until it levels off.</rdfs:comment>
        <rdfs:label xml:lang="en">LandingPlan</rdfs:label>
    </owl:Class>
    


    <!-- http://www.dronetology.net/dronetology#LandingSpeed -->

    <owl:Class rdf:about="http://www.dronetology.net/dronetology#LandingSpeed">
        <rdfs:subClassOf rdf:resource="http://www.dronetology.net/dronetology#Speed"/>
        <rdfs:comment xml:lang="en">LandingSpeed. The speed at which a drone lands.</rdfs:comment>
        <rdfs:label xml:lang="en">LandingSpeed</rdfs:label>
    </owl:Class>
    


    <!-- http://www.dronetology.net/dronetology#LandingWheel -->

    <owl:Class rdf:about="http://www.dronetology.net/dronetology#LandingWheel">
        <rdfs:subClassOf rdf:resource="http://www.dronetology.net/dronetology#LandingComponent"/>
        <rdfs:comment xml:lang="en">LandingWheel. Wheel used to takeoff or land in a runway. The fixed tricycle arrangement with one nose wheel (NLG) and two main wheels (MLG) at the rear is very common.</rdfs:comment>
        <rdfs:label xml:lang="en">LandingWheel</rdfs:label>
    </owl:Class>
    


    <!-- http://www.dronetology.net/dronetology#LargeUA -->

    <owl:Class rdf:about="http://www.dronetology.net/dronetology#LargeUA">
        <rdfs:subClassOf rdf:resource="http://www.dronetology.net/dronetology#Drone"/>
        <owl:disjointWith rdf:resource="http://www.dronetology.net/dronetology#MediumUA"/>
        <owl:disjointWith rdf:resource="http://www.dronetology.net/dronetology#SmallUA"/>
        <owl:disjointWith rdf:resource="http://www.dronetology.net/dronetology#VerySmallUA"/>
        <rdfs:comment xml:lang="en">LargeUA. Unmmaned aircraft with a wingspan greater than 10 m.</rdfs:comment>
        <rdfs:label xml:lang="en">LargeUA</rdfs:label>
    </owl:Class>
    


    <!-- http://www.dronetology.net/dronetology#LaunchSystem -->

    <owl:Class rdf:about="http://www.dronetology.net/dronetology#LaunchSystem">
        <rdfs:subClassOf rdf:resource="http://www.dronetology.net/dronetology#AuxiliaryComponent"/>
        <rdfs:comment xml:lang="en">LaunchSystem. A system that allows the drone takeoff.</rdfs:comment>
        <rdfs:label xml:lang="en">LaunchSystem</rdfs:label>
    </owl:Class>
    


    <!-- http://www.dronetology.net/dronetology#LiftGeneratorComponent -->

    <owl:Class rdf:about="http://www.dronetology.net/dronetology#LiftGeneratorComponent">
        <rdfs:subClassOf rdf:resource="http://www.dronetology.net/dronetology#AircraftComponent"/>
        <owl:disjointWith rdf:resource="http://www.dronetology.net/dronetology#Payload"/>
        <rdfs:comment xml:lang="en">LiftGeneratorComponent. A component that generates lift that holds the airplane in the air.</rdfs:comment>
        <rdfs:label xml:lang="en">LiftGeneratorComponent</rdfs:label>
    </owl:Class>
    


    <!-- http://www.dronetology.net/dronetology#LossCommunicationsRisk -->

    <owl:Class rdf:about="http://www.dronetology.net/dronetology#LossCommunicationsRisk">
        <rdfs:subClassOf rdf:resource="http://www.dronetology.net/dronetology#Risk"/>
        <rdfs:comment xml:lang="en">LossCommunicationRisk. Loss of communication implies risk like loss of aircraft control, missing clearence info, etc.</rdfs:comment>
        <rdfs:label xml:lang="en">LossCommunicationRisk</rdfs:label>
    </owl:Class>
    


    <!-- http://www.dronetology.net/dronetology#LossRisk -->

    <owl:Class rdf:about="http://www.dronetology.net/dronetology#LossRisk">
        <rdfs:subClassOf rdf:resource="http://www.dronetology.net/dronetology#Risk"/>
        <rdfs:comment xml:lang="en">LossRisk. Risk of loss is the allocation of responsibility for covering the risk of damage to or loss of goods.</rdfs:comment>
        <rdfs:label xml:lang="en">LossRisk</rdfs:label>
    </owl:Class>
    


    <!-- http://www.dronetology.net/dronetology#LowAltitudeCollisionRisk -->

    <owl:Class rdf:about="http://www.dronetology.net/dronetology#LowAltitudeCollisionRisk">
        <rdfs:subClassOf rdf:resource="http://www.dronetology.net/dronetology#CollisionRisk"/>
        <rdfs:comment xml:lang="en">LowAltitudeCollisionRisk. Collision risk in low altitude flights.</rdfs:comment>
        <rdfs:label xml:lang="en">LowAltitudeCollisionRisk</rdfs:label>
    </owl:Class>
    


    <!-- http://www.dronetology.net/dronetology#LowImpact -->

    <owl:Class rdf:about="http://www.dronetology.net/dronetology#LowImpact">
        <rdfs:subClassOf rdf:resource="http://www.dronetology.net/dronetology#RiskImpact"/>
        <rdfs:comment xml:lang="en">LowImpact. Low-impact risks are those that have a low probability of occurring and a limited negative effect on a UAS flight.</rdfs:comment>
        <rdfs:label xml:lang="en">LowImpact</rdfs:label>
    </owl:Class>
    


    <!-- http://www.dronetology.net/dronetology#LowLikelihood -->

    <owl:Class rdf:about="http://www.dronetology.net/dronetology#LowLikelihood">
        <rdfs:subClassOf rdf:resource="http://www.dronetology.net/dronetology#RiskLikelihood"/>
        <rdfs:label xml:lang="en">LowLikelihood</rdfs:label>
        <rdfs:label xml:lang="en">LowLikelihood. A low level of probability the risk will occur or be realized.</rdfs:label>
    </owl:Class>
    


    <!-- http://www.dronetology.net/dronetology#LowPriorityMission -->

    <owl:Class rdf:about="http://www.dronetology.net/dronetology#LowPriorityMission">
        <rdfs:subClassOf rdf:resource="http://www.dronetology.net/dronetology#MissionPriority"/>
        <rdfs:comment xml:lang="en">LowPriorityMission. Mission without any precedence.</rdfs:comment>
        <rdfs:label xml:lang="en">LowPriorityMission</rdfs:label>
    </owl:Class>
    


    <!-- http://www.dronetology.net/dronetology#MALE -->

    <owl:Class rdf:about="http://www.dronetology.net/dronetology#MALE">
        <rdfs:subClassOf rdf:resource="http://www.dronetology.net/dronetology#Drone"/>
        <rdfs:comment xml:lang="en">MALE. Medium Altitude Long Endurance drone.</rdfs:comment>
        <rdfs:label xml:lang="en">MALE</rdfs:label>
    </owl:Class>
    


    <!-- http://www.dronetology.net/dronetology#MAV -->

    <owl:Class rdf:about="http://www.dronetology.net/dronetology#MAV">
        <rdfs:subClassOf rdf:resource="http://www.dronetology.net/dronetology#Drone"/>
        <rdfs:comment xml:lang="en">MAV. Micro Air Vehicle. Unmanned aircraft bellow 2 kg of weight.</rdfs:comment>
        <rdfs:label xml:lang="en">MAV</rdfs:label>
    </owl:Class>
    


    <!-- http://www.dronetology.net/dronetology#MTOM -->

    <owl:Class rdf:about="http://www.dronetology.net/dronetology#MTOM">
        <rdfs:subClassOf rdf:resource="http://www.dronetology.net/dronetology#Mass"/>
        <rdfs:comment xml:lang="en">MTOM. It is the maximum mass at which the drone is certified for take off due to structural or other limits.</rdfs:comment>
        <rdfs:label xml:lang="en">MTOM</rdfs:label>
    </owl:Class>
    


    <!-- http://www.dronetology.net/dronetology#MTOW -->

    <owl:Class rdf:about="http://www.dronetology.net/dronetology#MTOW">
        <rdfs:subClassOf rdf:resource="http://www.dronetology.net/dronetology#Mass"/>
        <rdfs:comment xml:lang="en">MTOW. The maximum takeoff weight (MTOW) is the maximum takeoff mass.</rdfs:comment>
        <rdfs:label xml:lang="en">MTOW</rdfs:label>
    </owl:Class>
    


    <!-- http://www.dronetology.net/dronetology#MannedAircraft -->

    <owl:Class rdf:about="http://www.dronetology.net/dronetology#MannedAircraft">
        <rdfs:subClassOf rdf:resource="http://www.ontologydesignpatterns.org/ont/dul/DUL.owl#PhysicalObject"/>
        <rdfs:comment xml:lang="en">MannedAircraft. Manned aricraft.</rdfs:comment>
        <rdfs:label xml:lang="en">MannedAircraft</rdfs:label>
    </owl:Class>
    


    <!-- http://www.dronetology.net/dronetology#Manufacturer -->

    <owl:Class rdf:about="http://www.dronetology.net/dronetology#Manufacturer">
        <rdfs:comment xml:lang="en">Manufacturer. A drone manufacturer is a company or individual involved in the various aspects of designing, building, testing, selling, and maintaining aircraft or aircraft parts.</rdfs:comment>
        <rdfs:label xml:lang="en">Manufacturer</rdfs:label>
    </owl:Class>
    


    <!-- http://www.dronetology.net/dronetology#Mass -->

    <owl:Class rdf:about="http://www.dronetology.net/dronetology#Mass">
        <rdfs:subClassOf rdf:resource="http://qudt.org/schema/qudt/Quantity"/>
        <rdfs:comment xml:lang="en">Mass. The drone weight.</rdfs:comment>
        <rdfs:label xml:lang="en">Mass</rdfs:label>
    </owl:Class>
    


    <!-- http://www.dronetology.net/dronetology#MaxDimension -->

    <owl:Class rdf:about="http://www.dronetology.net/dronetology#MaxDimension">
        <rdfs:subClassOf rdf:resource="http://www.dronetology.net/dronetology#Dimension"/>
        <rdfs:comment xml:lang="en">MaxDimension. Maximun dimension permitted or regulated</rdfs:comment>
        <rdfs:label xml:lang="en">MaxDimension</rdfs:label>
    </owl:Class>
    


    <!-- http://www.dronetology.net/dronetology#MaxFlightRange -->

    <owl:Class rdf:about="http://www.dronetology.net/dronetology#MaxFlightRange">
        <rdfs:subClassOf rdf:resource="http://qudt.org/schema/qudt/Quantity"/>
        <rdfs:comment xml:lang="en">MaxFlightRange. The maximum distance that the aircraft can fly is equal to the ground speed times the maximum time.</rdfs:comment>
        <rdfs:label xml:lang="en">MaxFlightRange</rdfs:label>
    </owl:Class>
    


    <!-- http://www.dronetology.net/dronetology#MaxHeight -->

    <owl:Class rdf:about="http://www.dronetology.net/dronetology#MaxHeight">
        <rdfs:subClassOf rdf:resource="http://www.dronetology.net/dronetology#Height"/>
        <rdfs:comment xml:lang="en">MaxHeight. Maximun height a drone can fly.</rdfs:comment>
        <rdfs:label xml:lang="en">MaxHeight</rdfs:label>
    </owl:Class>
    


    <!-- http://www.dronetology.net/dronetology#MaxLandingSpeed -->

    <owl:Class rdf:about="http://www.dronetology.net/dronetology#MaxLandingSpeed">
        <rdfs:subClassOf rdf:resource="http://www.dronetology.net/dronetology#LandingSpeed"/>
        <rdfs:comment xml:lang="en">MaxLandingSpeed. Maximum safe landing speed.</rdfs:comment>
        <rdfs:label xml:lang="en">MaxLandingSpeed</rdfs:label>
    </owl:Class>
    


    <!-- http://www.dronetology.net/dronetology#MaxPayloadMass -->

    <owl:Class rdf:about="http://www.dronetology.net/dronetology#MaxPayloadMass">
        <rdfs:subClassOf rdf:resource="http://www.dronetology.net/dronetology#PayloadMass"/>
        <rdfs:comment xml:lang="en">MaxPayloadMass. Maximun payload weight.</rdfs:comment>
        <rdfs:label xml:lang="en">MaxPayloadMass</rdfs:label>
    </owl:Class>
    


    <!-- http://www.dronetology.net/dronetology#MaxVerticalTakeoffSpeed -->

    <owl:Class rdf:about="http://www.dronetology.net/dronetology#MaxVerticalTakeoffSpeed">
        <rdfs:subClassOf rdf:resource="http://www.dronetology.net/dronetology#VerticalTakeoffSpeed"/>
        <rdfs:comment xml:lang="en">MaxVerticalTakeoffSpeed. Maximun safe vertical takeoff speed.</rdfs:comment>
        <rdfs:label xml:lang="en">MaxVerticalTakeoffSpeed</rdfs:label>
    </owl:Class>
    


    <!-- http://www.dronetology.net/dronetology#MediumImpact -->

    <owl:Class rdf:about="http://www.dronetology.net/dronetology#MediumImpact">
        <rdfs:subClassOf rdf:resource="http://www.dronetology.net/dronetology#RiskImpact"/>
        <rdfs:comment xml:lang="en">MediumImpact.  Medium-impact risks are those that have a medium probability of occurring and a limited negative effect on a UAS flight.</rdfs:comment>
        <rdfs:label xml:lang="en">MediumImpact</rdfs:label>
    </owl:Class>
    


    <!-- http://www.dronetology.net/dronetology#MediumLikelihood -->

    <owl:Class rdf:about="http://www.dronetology.net/dronetology#MediumLikelihood">
        <rdfs:subClassOf rdf:resource="http://www.dronetology.net/dronetology#RiskLikelihood"/>
        <rdfs:comment xml:lang="en">MediumLikelihood. A medium level of probability the risk will occur or be realized.</rdfs:comment>
        <rdfs:label xml:lang="en">MediumLikelihood</rdfs:label>
    </owl:Class>
    


    <!-- http://www.dronetology.net/dronetology#MediumUA -->

    <owl:Class rdf:about="http://www.dronetology.net/dronetology#MediumUA">
        <rdfs:subClassOf rdf:resource="http://www.dronetology.net/dronetology#Drone"/>
        <owl:disjointWith rdf:resource="http://www.dronetology.net/dronetology#SmallUA"/>
        <owl:disjointWith rdf:resource="http://www.dronetology.net/dronetology#VerySmallUA"/>
        <rdfs:comment xml:lang="en">MediumUA. Unmanned aircraft with a wingspan of about 5-10 m that can carry payloads of 100 to 200 kg.</rdfs:comment>
        <rdfs:label xml:lang="en">MediumUA</rdfs:label>
    </owl:Class>
    


    <!-- http://www.dronetology.net/dronetology#MessageReceived -->

    <owl:Class rdf:about="http://www.dronetology.net/dronetology#MessageReceived">
        <rdfs:subClassOf rdf:resource="http://www.dronetology.net/dronetology#CommunicationMessage"/>
        <rdfs:comment xml:lang="en">MessageReceived. A communication message received in any radio receiver.</rdfs:comment>
        <rdfs:label xml:lang="en">MessageReceived</rdfs:label>
    </owl:Class>
    


    <!-- http://www.dronetology.net/dronetology#MessageSent -->

    <owl:Class rdf:about="http://www.dronetology.net/dronetology#MessageSent">
        <rdfs:subClassOf rdf:resource="http://www.dronetology.net/dronetology#CommunicationMessage"/>
        <rdfs:comment xml:lang="en">MessageSent. Any message sent using a radio transmitter.</rdfs:comment>
        <rdfs:label xml:lang="en">MessageSent</rdfs:label>
    </owl:Class>
    


    <!-- http://www.dronetology.net/dronetology#MilitaryManufacturer -->

    <owl:Class rdf:about="http://www.dronetology.net/dronetology#MilitaryManufacturer">
        <rdfs:subClassOf rdf:resource="http://www.dronetology.net/dronetology#Manufacturer"/>
        <rdfs:comment>Manufacturers that focus exclusively towards military drones.</rdfs:comment>
        <rdfs:label xml:lang="en">MilitaryManufacturer</rdfs:label>
    </owl:Class>
    


    <!-- http://www.dronetology.net/dronetology#Mission -->

    <owl:Class rdf:about="http://www.dronetology.net/dronetology#Mission">
        <rdfs:subClassOf>
            <owl:Class>
                <owl:intersectionOf rdf:parseType="Collection">
                    <owl:Restriction>
                        <owl:onProperty rdf:resource="http://www.dronetology.net/dronetology#hasObjective"/>
                        <owl:minQualifiedCardinality rdf:datatype="http://www.w3.org/2001/XMLSchema#nonNegativeInteger">1</owl:minQualifiedCardinality>
                        <owl:onClass rdf:resource="http://www.dronetology.net/dronetology#MissionObjective"/>
                    </owl:Restriction>
                    <owl:Restriction>
                        <owl:onProperty rdf:resource="http://www.dronetology.net/dronetology#hasElement"/>
                        <owl:qualifiedCardinality rdf:datatype="http://www.w3.org/2001/XMLSchema#nonNegativeInteger">1</owl:qualifiedCardinality>
                        <owl:onClass rdf:resource="http://www.dronetology.net/dronetology#MissionPilot"/>
                    </owl:Restriction>
                </owl:intersectionOf>
            </owl:Class>
        </rdfs:subClassOf>
        <rdfs:comment xml:lang="en">Mission. A drone mission is a flight planned or unplanned, with one or multiple objetives and a pilot.</rdfs:comment>
        <rdfs:label xml:lang="en">Mission</rdfs:label>
    </owl:Class>
    


    <!-- http://www.dronetology.net/dronetology#MissionAdvisory -->

    <owl:Class rdf:about="http://www.dronetology.net/dronetology#MissionAdvisory">
        <rdfs:subClassOf rdf:resource="http://www.dronetology.net/dronetology#MissionTemporalElement"/>
        <rdfs:comment xml:lang="en">MissionAdvisory. Mission recommendations.</rdfs:comment>
        <rdfs:label xml:lang="en">MissionAdvisory</rdfs:label>
    </owl:Class>
    


    <!-- http://www.dronetology.net/dronetology#MissionAirSpace -->

    <owl:Class rdf:about="http://www.dronetology.net/dronetology#MissionAirSpace">
        <rdfs:subClassOf>
            <owl:Class>
                <owl:intersectionOf rdf:parseType="Collection">
                    <rdf:Description rdf:about="http://www.dronetology.net/dronetology#FlyZone"/>
                    <rdf:Description rdf:about="http://www.dronetology.net/dronetology#MissionGeometryElement"/>
                    <rdf:Description rdf:about="http://www.dronetology.net/dronetology#MissionTemporalElement"/>
                </owl:intersectionOf>
            </owl:Class>
        </rdfs:subClassOf>
        <rdfs:comment xml:lang="en">MissionAirSpace. The portion of the atmosphere directly above the land or water, used by aircraft during a mission.</rdfs:comment>
        <rdfs:label xml:lang="en">MissionAirSpace</rdfs:label>
    </owl:Class>
    


    <!-- http://www.dronetology.net/dronetology#MissionAlarm -->

    <owl:Class rdf:about="http://www.dronetology.net/dronetology#MissionAlarm">
        <rdfs:subClassOf rdf:resource="http://www.dronetology.net/dronetology#MissionEventElement"/>
        <rdfs:comment xml:lang="en">MissionAlarm. Alarm during a drone mission.</rdfs:comment>
        <rdfs:label xml:lang="en">MissionAlarm</rdfs:label>
    </owl:Class>
    


    <!-- http://www.dronetology.net/dronetology#MissionCommand -->

    <owl:Class rdf:about="http://www.dronetology.net/dronetology#MissionCommand">
        <rdfs:subClassOf>
            <owl:Class>
                <owl:intersectionOf rdf:parseType="Collection">
                    <rdf:Description rdf:about="http://www.dronetology.net/dronetology#MissionGeometryPointElement"/>
                    <rdf:Description rdf:about="http://www.dronetology.net/dronetology#MissionTemporalElement"/>
                </owl:intersectionOf>
            </owl:Class>
        </rdfs:subClassOf>
        <rdfs:comment xml:lang="en">MissionCommand. A flight command assigned to a mission.</rdfs:comment>
        <rdfs:label xml:lang="en">MissionCommand</rdfs:label>
    </owl:Class>
    


    <!-- http://www.dronetology.net/dronetology#MissionCommanderStation -->

    <owl:Class rdf:about="http://www.dronetology.net/dronetology#MissionCommanderStation">
        <rdfs:subClassOf rdf:resource="http://www.dronetology.net/dronetology#GroundStationComponent"/>
        <owl:disjointWith rdf:resource="http://www.dronetology.net/dronetology#PayloadOperatorStation"/>
        <owl:disjointWith rdf:resource="http://www.dronetology.net/dronetology#RemotePilotConsole"/>
        <rdfs:comment xml:lang="en">MissionCommanderStation. Workstation used to control the drone.</rdfs:comment>
        <rdfs:label xml:lang="en">MissionCommanderStation</rdfs:label>
    </owl:Class>
    


    <!-- http://www.dronetology.net/dronetology#MissionCommunicationMessage -->

    <owl:Class rdf:about="http://www.dronetology.net/dronetology#MissionCommunicationMessage">
        <rdfs:subClassOf>
            <owl:Class>
                <owl:intersectionOf rdf:parseType="Collection">
                    <rdf:Description rdf:about="http://www.dronetology.net/dronetology#MissionGeometryPointElement"/>
                    <rdf:Description rdf:about="http://www.dronetology.net/dronetology#MissionTemporalElement"/>
                </owl:intersectionOf>
            </owl:Class>
        </rdfs:subClassOf>
        <rdfs:comment xml:lang="en">MissionCommunicationMessage. A communication message received or transmitted during a mission.</rdfs:comment>
        <rdfs:label xml:lang="en">MissionCommunicationMessage</rdfs:label>
    </owl:Class>
    


    <!-- http://www.dronetology.net/dronetology#MissionComplaince -->

    <owl:Class rdf:about="http://www.dronetology.net/dronetology#MissionComplaince">
        <rdfs:subClassOf rdf:resource="http://www.dronetology.net/dronetology#MissionElement"/>
        <rdfs:comment xml:lang="en">MissionCompliance. Any compliance regulation that may affect the UAS mission.</rdfs:comment>
        <rdfs:label xml:lang="en">MissionCompliance</rdfs:label>
    </owl:Class>
    


    <!-- http://www.dronetology.net/dronetology#MissionConflict -->

    <owl:Class rdf:about="http://www.dronetology.net/dronetology#MissionConflict">
        <rdfs:subClassOf>
            <owl:Class>
                <owl:intersectionOf rdf:parseType="Collection">
                    <rdf:Description rdf:about="http://www.dronetology.net/dronetology#Conflict"/>
                    <rdf:Description rdf:about="http://www.dronetology.net/dronetology#MissionGeometryElement"/>
                    <rdf:Description rdf:about="http://www.dronetology.net/dronetology#MissionTemporalElement"/>
                </owl:intersectionOf>
            </owl:Class>
        </rdfs:subClassOf>
        <rdfs:comment xml:lang="en">MissionConflict. A conflict identified in a specific UAS mission with the position and the time when ocurred.</rdfs:comment>
        <rdfs:label xml:lang="en">MissionConflict</rdfs:label>
    </owl:Class>
    


    <!-- http://www.dronetology.net/dronetology#MissionElement -->

    <owl:Class rdf:about="http://www.dronetology.net/dronetology#MissionElement">
        <rdfs:comment xml:lang="en">MissionElement. Any related UAS mission element, like an time interval, a point, etc.</rdfs:comment>
        <rdfs:label xml:lang="en">MissionElement</rdfs:label>
    </owl:Class>
    


    <!-- http://www.dronetology.net/dronetology#MissionEventElement -->

    <owl:Class rdf:about="http://www.dronetology.net/dronetology#MissionEventElement">
        <rdfs:subClassOf>
            <owl:Class>
                <owl:intersectionOf rdf:parseType="Collection">
                    <rdf:Description rdf:about="http://www.dronetology.net/dronetology#MissionElement"/>
                    <rdf:Description rdf:about="http://www.dronetology.net/dronetology#MissionTemporalElement"/>
                    <rdf:Description rdf:about="http://www.ontologydesignpatterns.org/ont/dul/DUL.owl#Event"/>
                </owl:intersectionOf>
            </owl:Class>
        </rdfs:subClassOf>
        <rdfs:comment xml:lang="en">MissionEventElement. A mission related things that are happening in a particular situation.</rdfs:comment>
        <rdfs:label xml:lang="en">MissionEventElement</rdfs:label>
    </owl:Class>
    


    <!-- http://www.dronetology.net/dronetology#MissionEventualRelationship -->

    <owl:Class rdf:about="http://www.dronetology.net/dronetology#MissionEventualRelationship">
        <rdfs:subClassOf>
            <owl:Class>
                <owl:intersectionOf rdf:parseType="Collection">
                    <rdf:Description rdf:about="http://www.dronetology.net/dronetology#MissionRelationship"/>
                    <rdf:Description rdf:about="http://www.ontologydesignpatterns.org/ont/dul/DUL.owl#Event"/>
                </owl:intersectionOf>
            </owl:Class>
        </rdfs:subClassOf>
        <rdfs:comment xml:lang="en">MissionEventualRelationship. A relationship between two UAS defined after an event.</rdfs:comment>
        <rdfs:label xml:lang="en">MissionEventualRelationship</rdfs:label>
    </owl:Class>
    


    <!-- http://www.dronetology.net/dronetology#MissionFlightPlan -->

    <owl:Class rdf:about="http://www.dronetology.net/dronetology#MissionFlightPlan">
        <rdfs:subClassOf rdf:resource="http://www.dronetology.net/dronetology#MissionTemporalElement"/>
        <rdfs:comment xml:lang="en">MissionFlightPlan. A fligh plan assigned to a drone mission.</rdfs:comment>
        <rdfs:label xml:lang="en">MissionFlightPlan</rdfs:label>
    </owl:Class>
    


    <!-- http://www.dronetology.net/dronetology#MissionFlightTrack -->

    <owl:Class rdf:about="http://www.dronetology.net/dronetology#MissionFlightTrack">
        <rdfs:subClassOf>
            <owl:Class>
                <owl:intersectionOf rdf:parseType="Collection">
                    <rdf:Description rdf:about="http://www.dronetology.net/dronetology#MissionGeometryPointElement"/>
                    <rdf:Description rdf:about="http://www.dronetology.net/dronetology#MissionTemporalElement"/>
                </owl:intersectionOf>
            </owl:Class>
        </rdfs:subClassOf>
        <rdfs:comment xml:lang="en">MissionFlightTrack. A sequence of locations of the aircraft during a mission.</rdfs:comment>
        <rdfs:label xml:lang="en">MissionFlightTrack</rdfs:label>
    </owl:Class>
    


    <!-- http://www.dronetology.net/dronetology#MissionGeometryElement -->

    <owl:Class rdf:about="http://www.dronetology.net/dronetology#MissionGeometryElement">
        <rdfs:subClassOf rdf:resource="http://www.dronetology.net/dronetology#MissionElement"/>
        <rdfs:comment xml:lang="en">MissionGeometryElement. Any mission element that have a geometry.</rdfs:comment>
        <rdfs:label xml:lang="en">MissionGeometryElement</rdfs:label>
    </owl:Class>
    


    <!-- http://www.dronetology.net/dronetology#MissionGeometryPointElement -->

    <owl:Class rdf:about="http://www.dronetology.net/dronetology#MissionGeometryPointElement">
        <rdfs:subClassOf rdf:resource="http://www.dronetology.net/dronetology#MissionElement"/>
        <rdfs:comment xml:lang="en">MissionGeometryPointElement. A mission element located at a single location in a defined coordinate space.</rdfs:comment>
        <rdfs:label xml:lang="en">MissionGeometryPointElement</rdfs:label>
    </owl:Class>
    


    <!-- http://www.dronetology.net/dronetology#MissionManagementSoftware -->

    <owl:Class rdf:about="http://www.dronetology.net/dronetology#MissionManagementSoftware">
        <rdfs:subClassOf rdf:resource="http://www.dronetology.net/dronetology#SoftwareComponent"/>
        <rdfs:comment xml:lang="en">MissionManagementSoftware. A software capable to prepare a drone mission with usually interfaces with mission planning and flight management systems.</rdfs:comment>
        <rdfs:label xml:lang="en">MissionManagementSoftware</rdfs:label>
    </owl:Class>
    


    <!-- http://www.dronetology.net/dronetology#MissionMode -->

    <owl:Class rdf:about="http://www.dronetology.net/dronetology#MissionMode">
        <rdfs:subClassOf rdf:resource="http://www.dronetology.net/dronetology#MissionElement"/>
        <rdfs:comment xml:lang="en">MissionMode. Defines the way the vehicle execute a mission.</rdfs:comment>
        <rdfs:label xml:lang="en">MissionMode</rdfs:label>
    </owl:Class>
    


    <!-- http://www.dronetology.net/dronetology#MissionObjective -->

    <owl:Class rdf:about="http://www.dronetology.net/dronetology#MissionObjective">
        <rdfs:subClassOf>
            <owl:Class>
                <owl:intersectionOf rdf:parseType="Collection">
                    <rdf:Description rdf:about="http://www.dronetology.net/dronetology#MissionTemporalElement"/>
                    <rdf:Description rdf:about="http://www.ontologydesignpatterns.org/ont/dul/DUL.owl#Goal"/>
                </owl:intersectionOf>
            </owl:Class>
        </rdfs:subClassOf>
        <rdfs:comment xml:lang="en">MissionObjective. A mission goal is a measurable indicator that must be achieved during the aircraft flight</rdfs:comment>
        <rdfs:label xml:lang="en">MissionObjective</rdfs:label>
    </owl:Class>
    


    <!-- http://www.dronetology.net/dronetology#MissionObstacle -->

    <owl:Class rdf:about="http://www.dronetology.net/dronetology#MissionObstacle">
        <rdfs:subClassOf>
            <owl:Class>
                <owl:intersectionOf rdf:parseType="Collection">
                    <rdf:Description rdf:about="http://www.dronetology.net/dronetology#MissionGeometryElement"/>
                    <rdf:Description rdf:about="http://www.dronetology.net/dronetology#MissionTemporalElement"/>
                    <rdf:Description rdf:about="http://www.dronetology.net/dronetology#Obstacle"/>
                </owl:intersectionOf>
            </owl:Class>
        </rdfs:subClassOf>
        <rdfs:comment xml:lang="en">MissionObstacle. An obstacle in a mission.</rdfs:comment>
        <rdfs:label xml:lang="en">MissionObstacle</rdfs:label>
    </owl:Class>
    


    <!-- http://www.dronetology.net/dronetology#MissionPilot -->

    <owl:Class rdf:about="http://www.dronetology.net/dronetology#MissionPilot">
        <rdfs:subClassOf>
            <owl:Class>
                <owl:intersectionOf rdf:parseType="Collection">
                    <rdf:Description rdf:about="http://www.dronetology.net/dronetology#MissionGeometryPointElement"/>
                    <rdf:Description rdf:about="http://www.dronetology.net/dronetology#MissionTemporalElement"/>
                    <rdf:Description rdf:about="http://www.dronetology.net/dronetology#Pilot"/>
                </owl:intersectionOf>
            </owl:Class>
        </rdfs:subClassOf>
        <rdfs:comment xml:lang="en">MissionPilot. A pilot assigned to a specific mission.</rdfs:comment>
        <rdfs:label xml:lang="en">MissionPilot</rdfs:label>
    </owl:Class>
    


    <!-- http://www.dronetology.net/dronetology#MissionPriority -->

    <owl:Class rdf:about="http://www.dronetology.net/dronetology#MissionPriority">
        <rdfs:subClassOf rdf:resource="http://www.dronetology.net/dronetology#MissionElement"/>
        <rdfs:comment xml:lang="en">MissionPriority. Stablish the fact or condition of a mission being regarded or treated as more important than others.</rdfs:comment>
        <rdfs:label xml:lang="en">MissionPriority</rdfs:label>
    </owl:Class>
    


    <!-- http://www.dronetology.net/dronetology#MissionRelationship -->

    <owl:Class rdf:about="http://www.dronetology.net/dronetology#MissionRelationship">
        <rdfs:subClassOf>
            <owl:Class>
                <owl:intersectionOf rdf:parseType="Collection">
                    <rdf:Description rdf:about="http://www.dronetology.net/dronetology#MissionElement"/>
                    <rdf:Description rdf:about="http://www.dronetology.net/dronetology#MissionEventElement"/>
                    <rdf:Description rdf:about="http://www.dronetology.net/dronetology#Relationship"/>
                </owl:intersectionOf>
            </owl:Class>
        </rdfs:subClassOf>
        <rdfs:comment xml:lang="en">MissionRelationship. The way in which two or more UAS are connected, or the state of being connected.</rdfs:comment>
        <rdfs:label xml:lang="en">MissionRelationship</rdfs:label>
    </owl:Class>
    


    <!-- http://www.dronetology.net/dronetology#MissionRisk -->

    <owl:Class rdf:about="http://www.dronetology.net/dronetology#MissionRisk">
        <rdfs:subClassOf>
            <owl:Class>
                <owl:intersectionOf rdf:parseType="Collection">
                    <rdf:Description rdf:about="http://www.dronetology.net/dronetology#MissionElement"/>
                    <rdf:Description rdf:about="http://www.dronetology.net/dronetology#Risk"/>
                </owl:intersectionOf>
            </owl:Class>
        </rdfs:subClassOf>
        <rdfs:comment xml:lang="en">MissionRisk. A situation involving exposure to danger during a UAS mission.</rdfs:comment>
        <rdfs:label xml:lang="en">MissionRisk</rdfs:label>
    </owl:Class>
    


    <!-- http://www.dronetology.net/dronetology#MissionSensorData -->

    <owl:Class rdf:about="http://www.dronetology.net/dronetology#MissionSensorData">
        <rdfs:subClassOf rdf:resource="http://www.dronetology.net/dronetology#MissionEventElement"/>
        <rdfs:comment xml:lang="en">MissionSensorData. Observation made by a sensor harvested during a UAS mission.</rdfs:comment>
        <rdfs:label xml:lang="en">MissionSensorData</rdfs:label>
    </owl:Class>
    


    <!-- http://www.dronetology.net/dronetology#MissionStatus -->

    <owl:Class rdf:about="http://www.dronetology.net/dronetology#MissionStatus">
        <rdfs:subClassOf rdf:resource="http://www.dronetology.net/dronetology#MissionElement"/>
        <rdfs:comment xml:lang="en">MissionStatus. The situation of a UAS mission at a particular time during a process.</rdfs:comment>
        <rdfs:label xml:lang="en">MissionStatus</rdfs:label>
    </owl:Class>
    


    <!-- http://www.dronetology.net/dronetology#MissionTemporalElement -->

    <owl:Class rdf:about="http://www.dronetology.net/dronetology#MissionTemporalElement">
        <rdfs:subClassOf rdf:resource="http://www.dronetology.net/dronetology#MissionElement"/>
        <rdfs:comment xml:lang="en">MissionTemporalElement. Any mission element that has a time interval relation.</rdfs:comment>
        <rdfs:label xml:lang="en">MissionTemporalElement</rdfs:label>
    </owl:Class>
    


    <!-- http://www.dronetology.net/dronetology#MissionWeatherReport -->

    <owl:Class rdf:about="http://www.dronetology.net/dronetology#MissionWeatherReport">
        <rdfs:subClassOf>
            <owl:Class>
                <owl:intersectionOf rdf:parseType="Collection">
                    <rdf:Description rdf:about="http://www.dronetology.net/dronetology#MissionGeometryElement"/>
                    <rdf:Description rdf:about="http://www.dronetology.net/dronetology#MissionTemporalElement"/>
                </owl:intersectionOf>
            </owl:Class>
        </rdfs:subClassOf>
        <rdfs:comment xml:lang="en">MissionWeatherReport. A weather report related to a UAS mission</rdfs:comment>
        <rdfs:label xml:lang="en">MissionWeatherReport</rdfs:label>
    </owl:Class>
    


    <!-- http://www.dronetology.net/dronetology#NEDVelocityCommand -->

    <owl:Class rdf:about="http://www.dronetology.net/dronetology#NEDVelocityCommand">
        <rdfs:subClassOf rdf:resource="http://www.dronetology.net/dronetology#Command"/>
        <owl:disjointWith>
            <owl:Class>
                <owl:unionOf rdf:parseType="Collection">
                    <rdf:Description rdf:about="http://www.dronetology.net/dronetology#AuxiliaryCommand"/>
                    <rdf:Description rdf:about="http://www.dronetology.net/dronetology#GoToCommand"/>
                </owl:unionOf>
            </owl:Class>
        </owl:disjointWith>
        <rdfs:comment xml:lang="en">NEDVelocityCommand. A command that changes the velocity using the North-East-Down Coordinates.</rdfs:comment>
        <rdfs:label xml:lang="en">NEDVelocityCommand</rdfs:label>
    </owl:Class>
    


    <!-- http://www.dronetology.net/dronetology#NoFlyZone -->

    <owl:Class rdf:about="http://www.dronetology.net/dronetology#NoFlyZone">
        <rdfs:subClassOf rdf:resource="http://www.dronetology.net/dronetology#AirSpaceVolume"/>
        <rdfs:comment xml:lang="en">NoFlyZone. A restricted area of airspace over a landmark, event or geographic region in which aircraft are forbidden to fly, unless they have special authorization.</rdfs:comment>
        <rdfs:label xml:lang="en">NoFlyZone</rdfs:label>
    </owl:Class>
    


    <!-- http://www.dronetology.net/dronetology#NoFlyZoneAlarm -->

    <owl:Class rdf:about="http://www.dronetology.net/dronetology#NoFlyZoneAlarm">
        <rdfs:subClassOf rdf:resource="http://www.dronetology.net/dronetology#Alarm"/>
        <rdfs:comment xml:lang="en">NoFlyZoneAlarm. A warning provoked when the UAS overflown a restricted area or no-fly zone.</rdfs:comment>
        <rdfs:label xml:lang="en">NoFlyZoneAlarm</rdfs:label>
    </owl:Class>
    


    <!-- http://www.dronetology.net/dronetology#NonComplianceRisk -->

    <owl:Class rdf:about="http://www.dronetology.net/dronetology#NonComplianceRisk">
        <rdfs:subClassOf rdf:resource="http://www.dronetology.net/dronetology#Risk"/>
        <rdfs:isDefinedBy xml:lang="en">NonComplianceRisk. Occurs when a UAS mission fails to comply with the policies, standards, regulations or laws relevant to its operations.</rdfs:isDefinedBy>
        <rdfs:label xml:lang="en">NonComplianceRisk</rdfs:label>
    </owl:Class>
    


    <!-- http://www.dronetology.net/dronetology#Nose -->

    <owl:Class rdf:about="http://www.dronetology.net/dronetology#Nose">
        <rdfs:subClassOf rdf:resource="http://www.dronetology.net/dronetology#Fuselage"/>
        <owl:disjointWith rdf:resource="http://www.dronetology.net/dronetology#Tail"/>
        <rdfs:comment xml:lang="en">Nose. The nose structure is the forward part of the fuselage and includes critical parts, such as the windshield, canopy, side sheet, and radome.</rdfs:comment>
        <rdfs:label xml:lang="en">Nose</rdfs:label>
    </owl:Class>
    


    <!-- http://www.dronetology.net/dronetology#Obstacle -->

    <owl:Class rdf:about="http://www.dronetology.net/dronetology#Obstacle">
        <rdfs:subClassOf rdf:resource="http://www.opengis.net/ont/geosparql#Feature"/>
        <rdfs:comment xml:lang="en">Obstacle. All fixed (whether temporary or permanent) and mobile objects, or parts thereof, that are located on an area intended for the surface movement of aircraft.</rdfs:comment>
        <rdfs:label xml:lang="en">Obstacle</rdfs:label>
    </owl:Class>
    


    <!-- http://www.dronetology.net/dronetology#OnboardComputer -->

    <owl:Class rdf:about="http://www.dronetology.net/dronetology#OnboardComputer">
        <rdfs:subClassOf rdf:resource="http://www.dronetology.net/dronetology#Payload"/>
        <rdfs:comment xml:lang="en">OnboardComputer. Any unit flying on board a drone which provides processing capability.</rdfs:comment>
        <rdfs:label xml:lang="en">OnboardComputer</rdfs:label>
    </owl:Class>
    


    <!-- http://www.dronetology.net/dronetology#OnboardSensor -->

    <owl:Class rdf:about="http://www.dronetology.net/dronetology#OnboardSensor">
        <rdfs:subClassOf rdf:resource="http://www.dronetology.net/dronetology#AircraftComponent"/>
        <rdfs:subClassOf rdf:resource="http://www.w3.org/ns/ssn/SensingDevice"/>
        <rdfs:comment xml:lang="en">OnboardSensor. Sensors integrated in the aircraft or carried as part of the drone payload.</rdfs:comment>
        <rdfs:label xml:lang="en">OnboardSensor</rdfs:label>
    </owl:Class>
    


    <!-- http://www.dronetology.net/dronetology#Parameter -->

    <owl:Class rdf:about="http://www.dronetology.net/dronetology#Parameter">
        <rdfs:comment xml:lang="en">Parameter. A numerical or other measurable factor forming one of a set that defines a system or sets the conditions of its operation.</rdfs:comment>
        <rdfs:label xml:lang="en">Parameter</rdfs:label>
    </owl:Class>
    


    <!-- http://www.dronetology.net/dronetology#PartialAutonomousMission -->

    <owl:Class rdf:about="http://www.dronetology.net/dronetology#PartialAutonomousMission">
        <rdfs:subClassOf rdf:resource="http://www.dronetology.net/dronetology#Mission"/>
        <rdfs:comment xml:lang="en">PartialAutonomousMission. A mission with parts that do not require a pilot.</rdfs:comment>
        <rdfs:label xml:lang="en">PartialAutonomousMission</rdfs:label>
    </owl:Class>
    


    <!-- http://www.dronetology.net/dronetology#Payload -->

    <owl:Class rdf:about="http://www.dronetology.net/dronetology#Payload">
        <rdfs:subClassOf rdf:resource="http://www.dronetology.net/dronetology#AircraftComponent"/>
        <owl:disjointWith rdf:resource="http://www.dronetology.net/dronetology#PowerDistributionBoard"/>
        <rdfs:comment xml:lang="en">Payload. The part of a vehicle&apos;s load, especially an aircraft&apos;s.</rdfs:comment>
        <rdfs:label xml:lang="en">Payload</rdfs:label>
    </owl:Class>
    


    <!-- http://www.dronetology.net/dronetology#PayloadLink -->

    <owl:Class rdf:about="http://www.dronetology.net/dronetology#PayloadLink">
        <rdfs:subClassOf rdf:resource="http://www.dronetology.net/dronetology#DataLink"/>
    </owl:Class>
    


    <!-- http://www.dronetology.net/dronetology#PayloadLossRisk -->

    <owl:Class rdf:about="http://www.dronetology.net/dronetology#PayloadLossRisk">
        <rdfs:subClassOf rdf:resource="http://www.dronetology.net/dronetology#LossRisk"/>
        <rdfs:comment xml:lang="en">PayloadLossRisk. Risk of loss of the payload.</rdfs:comment>
        <rdfs:label xml:lang="en">PayloadLossRisk</rdfs:label>
    </owl:Class>
    


    <!-- http://www.dronetology.net/dronetology#PayloadMass -->

    <owl:Class rdf:about="http://www.dronetology.net/dronetology#PayloadMass">
        <rdfs:subClassOf rdf:resource="http://qudt.org/schema/qudt/Quantity"/>
        <rdfs:comment xml:lang="en">PayloadMass. Weight of the drone payload</rdfs:comment>
        <rdfs:label xml:lang="en">PayloadMass</rdfs:label>
    </owl:Class>
    


    <!-- http://www.dronetology.net/dronetology#PayloadOperatorStation -->

    <owl:Class rdf:about="http://www.dronetology.net/dronetology#PayloadOperatorStation">
        <rdfs:subClassOf rdf:resource="http://www.dronetology.net/dronetology#GroundStationComponent"/>
        <owl:disjointWith rdf:resource="http://www.dronetology.net/dronetology#RemotePilotConsole"/>
        <rdfs:comment xml:lang="en">PayloadOperatorStation. Workstation to control the payload.</rdfs:comment>
        <rdfs:label xml:lang="en">PayloadOperatorStation</rdfs:label>
    </owl:Class>
    


    <!-- http://www.dronetology.net/dronetology#Photograph -->

    <owl:Class rdf:about="http://www.dronetology.net/dronetology#Photograph">
        <rdfs:subClassOf rdf:resource="http://www.dronetology.net/dronetology#MissionTemporalElement"/>
        <rdfs:subClassOf>
            <owl:Restriction>
                <owl:onProperty rdf:resource="http://www.dronetology.net/dronetology#isStoredIn"/>
                <owl:someValuesFrom rdf:resource="http://www.dronetology.net/dronetology#DataStorageDevice"/>
            </owl:Restriction>
        </rdfs:subClassOf>
        <owl:disjointWith rdf:resource="http://www.dronetology.net/dronetology#Video"/>
        <rdfs:comment xml:lang="en">Photograph. A picture made using a camera installed as payload of the UAS during a mission.</rdfs:comment>
        <rdfs:label xml:lang="en">Photograph</rdfs:label>
    </owl:Class>
    


    <!-- http://www.dronetology.net/dronetology#Pilot -->

    <owl:Class rdf:about="http://www.dronetology.net/dronetology#Pilot">
        <rdfs:subClassOf rdf:resource="http://www.ontologydesignpatterns.org/ont/dul/DUL.owl#NaturalPerson"/>
        <rdfs:comment xml:lang="en">Pilot. A person who operates the flying controls of an aircraft, onboard or remotely.</rdfs:comment>
        <rdfs:label xml:lang="en">Pilot</rdfs:label>
    </owl:Class>
    


    <!-- http://www.dronetology.net/dronetology#PilotIncapacitationRisk -->

    <owl:Class rdf:about="http://www.dronetology.net/dronetology#PilotIncapacitationRisk">
        <rdfs:subClassOf rdf:resource="http://www.dronetology.net/dronetology#Risk"/>
        <rdfs:comment xml:lang="en">PilotIncapacitationRisk. Risk provoked by a pilot disease during the flight.</rdfs:comment>
        <rdfs:label xml:lang="en">PilotIncapacitationRisk</rdfs:label>
    </owl:Class>
    


    <!-- http://www.dronetology.net/dronetology#PilotLicence -->

    <owl:Class rdf:about="http://www.dronetology.net/dronetology#PilotLicence">
        <rdfs:subClassOf rdf:resource="http://www.dronetology.net/dronetology#RegulationRequirement"/>
        <rdfs:comment xml:lang="en">PilotLicence. A competency certificate required for some drone mission.</rdfs:comment>
        <rdfs:label xml:lang="en">PilotLicence</rdfs:label>
    </owl:Class>
    


    <!-- http://www.dronetology.net/dronetology#Pitch -->

    <owl:Class rdf:about="http://www.dronetology.net/dronetology#Pitch">
        <rdfs:subClassOf rdf:resource="http://qudt.org/schema/qudt/Quantity"/>
        <rdfs:comment xml:lang="en">Pitch. The forward and backward tilt of the drone.</rdfs:comment>
        <rdfs:label xml:lang="en">Pitch</rdfs:label>
    </owl:Class>
    


    <!-- http://www.dronetology.net/dronetology#PlannedMission -->

    <owl:Class rdf:about="http://www.dronetology.net/dronetology#PlannedMission">
        <rdfs:subClassOf rdf:resource="http://www.dronetology.net/dronetology#Mission"/>
        <rdfs:comment xml:lang="en">PlannedMission. A mission with a planned fligh.</rdfs:comment>
        <rdfs:label xml:lang="en">PlannedMission</rdfs:label>
    </owl:Class>
    


    <!-- http://www.dronetology.net/dronetology#PowerDistributionBoard -->

    <owl:Class rdf:about="http://www.dronetology.net/dronetology#PowerDistributionBoard">
        <rdfs:subClassOf rdf:resource="http://www.dronetology.net/dronetology#AircraftComponent"/>
        <rdfs:comment xml:lang="en">PowerDistributionBoard. It distributes power to different areas of the drone.</rdfs:comment>
        <rdfs:label xml:lang="en">PowerDistributionBoard</rdfs:label>
    </owl:Class>
    


    <!-- http://www.dronetology.net/dronetology#Product -->

    <owl:Class rdf:about="http://www.dronetology.net/dronetology#Product">
        <rdfs:subClassOf>
            <owl:Restriction>
                <owl:onProperty rdf:resource="http://www.dronetology.net/dronetology#isProductOf"/>
                <owl:someValuesFrom rdf:resource="http://www.dronetology.net/dronetology#Drone"/>
            </owl:Restriction>
        </rdfs:subClassOf>
        <rdfs:comment xml:lang="en">Product. The drone model.</rdfs:comment>
        <rdfs:label xml:lang="en">Product</rdfs:label>
    </owl:Class>
    


    <!-- http://www.dronetology.net/dronetology#Propeller -->

    <owl:Class rdf:about="http://www.dronetology.net/dronetology#Propeller">
        <rdfs:subClassOf rdf:resource="http://www.dronetology.net/dronetology#RotorComponent"/>
        <owl:disjointWith rdf:resource="http://www.dronetology.net/dronetology#Rotor"/>
        <rdfs:comment xml:lang="en">Propeller. Are in charge of rotating to provide lift to the drone,</rdfs:comment>
        <rdfs:label xml:lang="en">Propeller</rdfs:label>
    </owl:Class>
    


    <!-- http://www.dronetology.net/dronetology#QZSS -->

    <owl:Class rdf:about="http://www.dronetology.net/dronetology#QZSS">
        <rdfs:subClassOf rdf:resource="http://www.dronetology.net/dronetology#GlobalNavigationSatelliteSystem"/>
        <rdfs:comment xml:lang="en">QZSS. QZSS is a regional GNSS owned by the Government of Japan and operated by QZS System Service Inc. (QSS). QZSS complements GPS to improve coverage in East Asia and Oceania.</rdfs:comment>
        <rdfs:label xml:lang="en">QZSS</rdfs:label>
    </owl:Class>
    


    <!-- http://www.dronetology.net/dronetology#RPA -->

    <owl:Class rdf:about="http://www.dronetology.net/dronetology#RPA">
        <rdfs:subClassOf rdf:resource="http://www.dronetology.net/dronetology#Drone"/>
        <rdfs:comment xml:lang="en">RPA. Remotely piloted aircraft.</rdfs:comment>
        <rdfs:label xml:lang="en">RPA</rdfs:label>
    </owl:Class>
    


    <!-- http://www.dronetology.net/dronetology#RPAS -->

    <owl:Class rdf:about="http://www.dronetology.net/dronetology#RPAS">
        <rdfs:subClassOf rdf:resource="http://www.dronetology.net/dronetology#RPA"/>
        <rdfs:comment xml:lang="en">RPAS. Remotely piloted aircraft system.</rdfs:comment>
        <rdfs:label xml:lang="en">RPAS</rdfs:label>
    </owl:Class>
    


    <!-- http://www.dronetology.net/dronetology#RainFall -->

    <owl:Class rdf:about="http://www.dronetology.net/dronetology#RainFall">
        <rdfs:subClassOf rdf:resource="http://qudt.org/schema/qudt/Quantity"/>
        <rdfs:comment xml:lang="en">RainFall. The amount of water falling in rain, snow, etc., within a given time and area,</rdfs:comment>
        <rdfs:label xml:lang="en">RainFall</rdfs:label>
    </owl:Class>
    


    <!-- http://www.dronetology.net/dronetology#RecoveryNet -->

    <owl:Class rdf:about="http://www.dronetology.net/dronetology#RecoveryNet">
        <rdfs:subClassOf rdf:resource="http://www.dronetology.net/dronetology#AuxiliaryComponent"/>
        <rdfs:comment xml:lang="en">RecoveryNet. Safety net in which a drone can land.</rdfs:comment>
        <rdfs:label xml:lang="en">RecoveryNet</rdfs:label>
    </owl:Class>
    


    <!-- http://www.dronetology.net/dronetology#RefuelingSystem -->

    <owl:Class rdf:about="http://www.dronetology.net/dronetology#RefuelingSystem">
        <rdfs:subClassOf rdf:resource="http://www.dronetology.net/dronetology#AuxiliaryComponent"/>
        <rdfs:comment xml:lang="en">RefuelingSystem. A facility that provides fuel and engine lubricants for motor vehicles.</rdfs:comment>
        <rdfs:label xml:lang="en">RefuelingSystem</rdfs:label>
    </owl:Class>
    


    <!-- http://www.dronetology.net/dronetology#Regulation -->

    <owl:Class rdf:about="http://www.dronetology.net/dronetology#Regulation">
        <rdfs:comment xml:lang="en">Regulation. Regulation of unmanned aerial vehicles (UAVs) involves setting safety requirements, outlining regulations for the safe flying of drones, and enforcing action against errant users.</rdfs:comment>
        <rdfs:label xml:lang="en">Regulation</rdfs:label>
    </owl:Class>
    


    <!-- http://www.dronetology.net/dronetology#RegulationRequirement -->

    <owl:Class rdf:about="http://www.dronetology.net/dronetology#RegulationRequirement">
        <rdfs:comment xml:lang="en">RegulationRequirement. Groups drone rules that a drone operator must comply with in a specific geographic area</rdfs:comment>
        <rdfs:label xml:lang="en">RegulationRequirement</rdfs:label>
    </owl:Class>
    


    <!-- http://www.dronetology.net/dronetology#Relationship -->

    <owl:Class rdf:about="http://www.dronetology.net/dronetology#Relationship">
        <rdfs:comment xml:lang="en">Relationship. The way two or more UAS are connected, or the way they behave toward each other.</rdfs:comment>
        <rdfs:label xml:lang="en">Relationship</rdfs:label>
    </owl:Class>
    


    <!-- http://www.dronetology.net/dronetology#RemoteGuided -->

    <owl:Class rdf:about="http://www.dronetology.net/dronetology#RemoteGuided">
        <rdfs:subClassOf rdf:resource="http://www.dronetology.net/dronetology#Mission"/>
        <rdfs:subClassOf>
            <owl:Restriction>
                <owl:onProperty rdf:resource="http://www.dronetology.net/dronetology#hasElement"/>
                <owl:someValuesFrom rdf:resource="http://www.dronetology.net/dronetology#FlightPlan"/>
            </owl:Restriction>
        </rdfs:subClassOf>
        <rdfs:subClassOf>
            <owl:Restriction>
                <owl:onProperty rdf:resource="http://www.dronetology.net/dronetology#hasElement"/>
                <owl:minQualifiedCardinality rdf:datatype="http://www.w3.org/2001/XMLSchema#nonNegativeInteger">1</owl:minQualifiedCardinality>
                <owl:onClass rdf:resource="http://www.dronetology.net/dronetology#Pilot"/>
            </owl:Restriction>
        </rdfs:subClassOf>
        <rdfs:comment xml:lang="en">RemoteGuided. A mission guided remotely by a pilot.</rdfs:comment>
        <rdfs:label xml:lang="en">RemotedGuided</rdfs:label>
    </owl:Class>
    


    <!-- http://www.dronetology.net/dronetology#RemoteID -->

    <owl:Class rdf:about="http://www.dronetology.net/dronetology#RemoteID">
        <rdfs:subClassOf rdf:resource="http://www.dronetology.net/dronetology#CommunicationSystem"/>
        <rdfs:comment xml:lang="en">RemoteID. A system that allows drones to transmit identification and location information.</rdfs:comment>
        <rdfs:label xml:lang="en">RemoteID</rdfs:label>
    </owl:Class>
    


    <!-- http://www.dronetology.net/dronetology#RemoteId -->

    <owl:Class rdf:about="http://www.dronetology.net/dronetology#RemoteId">
        <rdfs:subClassOf rdf:resource="http://www.dronetology.net/dronetology#MessageReceived"/>
        <rdfs:comment xml:lang="en">RemoteId. A message sent by a wireless technology that broadcast drone identificator.</rdfs:comment>
        <rdfs:label xml:lang="en">RemoteId</rdfs:label>
    </owl:Class>
    


    <!-- http://www.dronetology.net/dronetology#RemoteIdentification -->

    <owl:Class rdf:about="http://www.dronetology.net/dronetology#RemoteIdentification">
        <rdfs:subClassOf rdf:resource="http://www.dronetology.net/dronetology#RegulationRequirement"/>
        <rdfs:comment xml:lang="en">RemoteIdentification. A rquired system that allows to identify remotely the drone.</rdfs:comment>
        <rdfs:label xml:lang="en">RemoteIdentification</rdfs:label>
    </owl:Class>
    


    <!-- http://www.dronetology.net/dronetology#RemotePilotConsole -->

    <owl:Class rdf:about="http://www.dronetology.net/dronetology#RemotePilotConsole">
        <rdfs:subClassOf rdf:resource="http://www.dronetology.net/dronetology#GroundStationComponent"/>
        <rdfs:comment xml:lang="en">RemotePilotConsole. Worksapce for a remote pilot.</rdfs:comment>
        <rdfs:label xml:lang="en">RemotePilotConsole</rdfs:label>
    </owl:Class>
    


    <!-- http://www.dronetology.net/dronetology#Requirement -->

    <owl:Class rdf:about="http://www.dronetology.net/dronetology#Requirement">
        <rdfs:comment xml:lang="en">Requirement. A requirement specify the properties (functional, structural, physical, etc.) of the artifact being designed.</rdfs:comment>
        <rdfs:label xml:lang="en">Requirement</rdfs:label>
    </owl:Class>
    


    <!-- http://www.dronetology.net/dronetology#Risk -->

    <owl:Class rdf:about="http://www.dronetology.net/dronetology#Risk">
        <rdfs:comment xml:lang="en">A situation involving exposure to danger.</rdfs:comment>
    </owl:Class>
    


    <!-- http://www.dronetology.net/dronetology#RiskImpact -->

    <owl:Class rdf:about="http://www.dronetology.net/dronetology#RiskImpact">
        <rdfs:comment xml:lang="en">RiskImpact. The level of severity the risk will have if the risk is realized.</rdfs:comment>
        <rdfs:label xml:lang="en">RiskImpact</rdfs:label>
    </owl:Class>
    


    <!-- http://www.dronetology.net/dronetology#RiskLikelihood -->

    <owl:Class rdf:about="http://www.dronetology.net/dronetology#RiskLikelihood">
        <rdfs:comment xml:lang="en">RiskLikelihood. Risk likelihood means the possibility of a potential risk occurring, interpreted using qualitative values.</rdfs:comment>
        <rdfs:label xml:lang="en">RiskLikelihood</rdfs:label>
    </owl:Class>
    


    <!-- http://www.dronetology.net/dronetology#Roll -->

    <owl:Class rdf:about="http://www.dronetology.net/dronetology#Roll">
        <rdfs:subClassOf rdf:resource="http://qudt.org/schema/qudt/Quantity"/>
        <rdfs:comment xml:lang="en">Roll. The rotation of the drone along the x-axis, i.e. the side to side motion of the drone.</rdfs:comment>
        <rdfs:label xml:lang="en">Roll</rdfs:label>
    </owl:Class>
    


    <!-- http://www.dronetology.net/dronetology#Rotor -->

    <owl:Class rdf:about="http://www.dronetology.net/dronetology#Rotor">
        <rdfs:subClassOf rdf:resource="http://www.dronetology.net/dronetology#LiftGeneratorComponent"/>
        <rdfs:subClassOf>
            <owl:Restriction>
                <owl:onProperty rdf:resource="http://www.dronetology.net/dronetology#hasPart"/>
                <owl:allValuesFrom rdf:resource="http://www.dronetology.net/dronetology#RotorComponent"/>
            </owl:Restriction>
        </rdfs:subClassOf>
        <owl:disjointWith rdf:resource="http://www.dronetology.net/dronetology#Wing"/>
        <rdfs:comment xml:lang="en">Rotor. A rotor is the rotating cylindrical part of a machine, placed inside the stator with a narrow air gap.</rdfs:comment>
        <rdfs:label xml:lang="en">Rotor</rdfs:label>
    </owl:Class>
    


    <!-- http://www.dronetology.net/dronetology#RotorComponent -->

    <owl:Class rdf:about="http://www.dronetology.net/dronetology#RotorComponent">
        <rdfs:subClassOf rdf:resource="http://www.dronetology.net/dronetology#LiftGeneratorComponent"/>
        <rdfs:comment xml:lang="en">RotorComponent. Parts of the rotor.</rdfs:comment>
        <rdfs:label xml:lang="en">RotorComponent</rdfs:label>
    </owl:Class>
    


    <!-- http://www.dronetology.net/dronetology#Runway -->

    <owl:Class rdf:about="http://www.dronetology.net/dronetology#Runway">
        <rdfs:subClassOf rdf:resource="http://www.opengis.net/ont/geosparql#Feature"/>
        <rdfs:comment xml:lang="en">Runway. A runway is a defined rectangular area on a land aerodrome prepared for the landing and takeoff of aircraft.</rdfs:comment>
        <rdfs:label xml:lang="en">Runway</rdfs:label>
    </owl:Class>
    


    <!-- http://www.dronetology.net/dronetology#STOLCraft -->

    <owl:Class rdf:about="http://www.dronetology.net/dronetology#STOLCraft">
        <rdfs:subClassOf rdf:resource="http://www.dronetology.net/dronetology#Drone"/>
        <owl:disjointWith rdf:resource="http://www.dronetology.net/dronetology#VTOLCraft"/>
        <rdfs:comment xml:lang="en">STOLCraft. A short takeoff and landing (STOL) aircraft is a conventional fixed-wing aircraft that has short runway requirements for takeoff and landing.</rdfs:comment>
        <rdfs:label xml:lang="en">STOLCraft</rdfs:label>
    </owl:Class>
    


    <!-- http://www.dronetology.net/dronetology#ScheduledFlightPlan -->

    <owl:Class rdf:about="http://www.dronetology.net/dronetology#ScheduledFlightPlan">
        <rdfs:subClassOf rdf:resource="http://www.dronetology.net/dronetology#FlightPlan"/>
        <rdfs:comment xml:lang="en">ScheduledFlightPlan. A flightplan that includes time references in different aircraft locations.</rdfs:comment>
        <rdfs:label xml:lang="en">ScheduledFlightPlan</rdfs:label>
    </owl:Class>
    


    <!-- http://www.dronetology.net/dronetology#SensorHarvestingMission -->

    <owl:Class rdf:about="http://www.dronetology.net/dronetology#SensorHarvestingMission">
        <rdfs:subClassOf rdf:resource="http://www.dronetology.net/dronetology#Mission"/>
        <rdfs:comment xml:lang="en">SensorHarvestingMission. Mission that harvest data from sensors using the dorne as a sink data.</rdfs:comment>
        <rdfs:label xml:lang="en">SensorHarvestingMission</rdfs:label>
    </owl:Class>
    


    <!-- http://www.dronetology.net/dronetology#SimulatedTelemetry -->

    <owl:Class rdf:about="http://www.dronetology.net/dronetology#SimulatedTelemetry">
        <rdfs:subClassOf rdf:resource="http://www.dronetology.net/dronetology#Telemetry"/>
        <rdfs:comment xml:lang="en">SimulatedTelemetry. Telemetry generated by a drone simulator.</rdfs:comment>
        <rdfs:label xml:lang="en">SimulatedTelemetry</rdfs:label>
    </owl:Class>
    


    <!-- http://www.dronetology.net/dronetology#SituationalAwareness -->

    <owl:Class rdf:about="http://www.dronetology.net/dronetology#SituationalAwareness">
        <rdfs:comment xml:lang="en">SituationalAwareness. Situational awareness is the ability to perceive, understand, and effectively respond to one&apos;s situation.</rdfs:comment>
        <rdfs:label xml:lang="en">SituationalAwareness</rdfs:label>
    </owl:Class>
    


    <!-- http://www.dronetology.net/dronetology#SmallUA -->

    <owl:Class rdf:about="http://www.dronetology.net/dronetology#SmallUA">
        <rdfs:subClassOf rdf:resource="http://www.dronetology.net/dronetology#Drone"/>
        <owl:disjointWith rdf:resource="http://www.dronetology.net/dronetology#VerySmallUA"/>
        <rdfs:comment xml:lang="en">SmallUA. Unmanned aircraft that have at least one dimension greater than 50 cm and no larger than 2 meters.</rdfs:comment>
        <rdfs:label xml:lang="en">SmallUA</rdfs:label>
    </owl:Class>
    


    <!-- http://www.dronetology.net/dronetology#SoftwareComponent -->

    <owl:Class rdf:about="http://www.dronetology.net/dronetology#SoftwareComponent">
        <rdfs:subClassOf rdf:resource="http://www.dronetology.net/dronetology#Component"/>
        <rdfs:comment xml:lang="en">SoftwareComponent. A software package or a module that encapsulates a set of related functions for the operation or management of a drone.</rdfs:comment>
        <rdfs:label xml:lang="en">SoftwareComponent</rdfs:label>
    </owl:Class>
    


    <!-- http://www.dronetology.net/dronetology#Speed -->

    <owl:Class rdf:about="http://www.dronetology.net/dronetology#Speed">
        <rdfs:subClassOf rdf:resource="http://qudt.org/schema/qudt/Quantity"/>
        <rdfs:comment xml:lang="en">Speed. The rate at which a drone moves or operates or is able to move or operate.</rdfs:comment>
        <rdfs:label xml:lang="en">Speed</rdfs:label>
    </owl:Class>
    


    <!-- http://www.dronetology.net/dronetology#StallSpeed -->

    <owl:Class rdf:about="http://www.dronetology.net/dronetology#StallSpeed">
        <rdfs:subClassOf rdf:resource="http://www.dronetology.net/dronetology#Speed"/>
        <rdfs:comment xml:lang="en">StallSpeed. Stall speed refers to the minimum speed at which an airplane must fly to produce lift.</rdfs:comment>
        <rdfs:label xml:lang="en">StallSpeed</rdfs:label>
    </owl:Class>
    


    <!-- http://www.dronetology.net/dronetology#Strator -->

    <owl:Class rdf:about="http://www.dronetology.net/dronetology#Strator">
        <rdfs:subClassOf rdf:resource="http://www.dronetology.net/dronetology#RotorComponent"/>
        <rdfs:comment xml:lang="en">Strator.  The stationary part of an electrical motor.</rdfs:comment>
        <rdfs:label xml:lang="en">Strator</rdfs:label>
    </owl:Class>
    


    <!-- http://www.dronetology.net/dronetology#Swarm -->

    <owl:Class rdf:about="http://www.dronetology.net/dronetology#Swarm">
        <rdfs:subClassOf rdf:resource="http://www.opengis.net/ont/geosparql#Feature"/>
        <rdfs:comment xml:lang="en">Swarm. A swarm or fleet of Unmanned Aerial Vehicles (UAVs) is a set of aerial robots i.e., drones that work together to achieve a specific goal.</rdfs:comment>
        <rdfs:label xml:lang="en">Swarm</rdfs:label>
    </owl:Class>
    


    <!-- http://www.dronetology.net/dronetology#Tail -->

    <owl:Class rdf:about="http://www.dronetology.net/dronetology#Tail">
        <rdfs:subClassOf rdf:resource="http://www.dronetology.net/dronetology#Fuselage"/>
        <rdfs:comment xml:lang="en">Tail. Part of the fuselage located at the rear of an aircraft that provides stability during flight.</rdfs:comment>
        <rdfs:label xml:lang="en">Tail</rdfs:label>
    </owl:Class>
    


    <!-- http://www.dronetology.net/dronetology#TakeoffPlan -->

    <owl:Class rdf:about="http://www.dronetology.net/dronetology#TakeoffPlan">
        <rdfs:subClassOf rdf:resource="http://www.dronetology.net/dronetology#FlightPlan"/>
        <rdfs:comment xml:lang="en">TakeoffPlan. A part of the flighplan that starts when the aircraft begins to descend for landing.</rdfs:comment>
        <rdfs:label xml:lang="en">TakeoffPlan</rdfs:label>
    </owl:Class>
    


    <!-- http://www.dronetology.net/dronetology#Telemetry -->

    <owl:Class rdf:about="http://www.dronetology.net/dronetology#Telemetry">
        <rdfs:subClassOf>
            <owl:Class>
                <owl:intersectionOf rdf:parseType="Collection">
                    <rdf:Description rdf:about="http://www.dronetology.net/dronetology#MissionGeometryPointElement"/>
                    <rdf:Description rdf:about="http://www.dronetology.net/dronetology#MissionTemporalElement"/>
                </owl:intersectionOf>
            </owl:Class>
        </rdfs:subClassOf>
        <rdfs:comment xml:lang="en">Telemetry. Data gathered about the aircraft and its surroundings that is sent back to the operator or ground control station during a mission.</rdfs:comment>
        <rdfs:label xml:lang="en">Telemetry</rdfs:label>
    </owl:Class>
    


    <!-- http://www.dronetology.net/dronetology#TiltRotorCraft -->

    <owl:Class rdf:about="http://www.dronetology.net/dronetology#TiltRotorCraft">
        <rdfs:subClassOf rdf:resource="http://www.dronetology.net/dronetology#FixedWingVTOLCraft"/>
        <rdfs:comment xml:lang="en">TiltRotorCraft. Aircraft that convert from vertical to horizontal flight by rotating propellers or ducted fans from horizontal positions like conventional aircraft propellers to vertical like a helicopter&apos;s rotors.</rdfs:comment>
        <rdfs:label xml:lang="en">TiltRotorCraft</rdfs:label>
    </owl:Class>
    


    <!-- http://www.dronetology.net/dronetology#TiltWingCraft -->

    <owl:Class rdf:about="http://www.dronetology.net/dronetology#TiltWingCraft">
        <rdfs:subClassOf rdf:resource="http://www.dronetology.net/dronetology#FixedWingVTOLCraft"/>
        <rdfs:comment xml:lang="en">TiltWingCraft. A tiltwing aircraft features a wing that is horizontal for conventional forward flight and rotates up for vertical takeoff and landing.</rdfs:comment>
        <rdfs:label xml:lang="en">TiltWingCraft</rdfs:label>
    </owl:Class>
    


    <!-- http://www.dronetology.net/dronetology#TrailingEdge -->

    <owl:Class rdf:about="http://www.dronetology.net/dronetology#TrailingEdge">
        <rdfs:subClassOf rdf:resource="http://www.dronetology.net/dronetology#WingComponent"/>
        <rdfs:comment xml:lang="en">TrailingEdge. The rear part of the wing that extends from the wing root to the wingtip. The trailing edge plays a crucial role in the overall aerodynamic performance of the aircraft.</rdfs:comment>
        <rdfs:label xml:lang="en">TrailingEdge</rdfs:label>
    </owl:Class>
    


    <!-- http://www.dronetology.net/dronetology#UA -->

    <owl:Class rdf:about="http://www.dronetology.net/dronetology#UA">
        <rdfs:subClassOf rdf:resource="http://www.dronetology.net/dronetology#Drone"/>
        <rdfs:comment xml:lang="en">UA. Unmanned aircraft.</rdfs:comment>
        <rdfs:label xml:lang="en">UA</rdfs:label>
    </owl:Class>
    


    <!-- http://www.dronetology.net/dronetology#UAS -->

    <owl:Class rdf:about="http://www.dronetology.net/dronetology#UAS">
        <rdfs:subClassOf rdf:resource="http://www.dronetology.net/dronetology#Drone"/>
        <rdfs:subClassOf>
            <owl:Restriction>
                <owl:onProperty rdf:resource="http://www.dronetology.net/dronetology#hasComponent"/>
                <owl:minQualifiedCardinality rdf:datatype="http://www.w3.org/2001/XMLSchema#nonNegativeInteger">1</owl:minQualifiedCardinality>
                <owl:onClass rdf:resource="http://www.dronetology.net/dronetology#DataLink"/>
            </owl:Restriction>
        </rdfs:subClassOf>
        <rdfs:subClassOf>
            <owl:Restriction>
                <owl:onProperty rdf:resource="http://www.dronetology.net/dronetology#hasComponent"/>
                <owl:qualifiedCardinality rdf:datatype="http://www.w3.org/2001/XMLSchema#nonNegativeInteger">1</owl:qualifiedCardinality>
                <owl:onClass rdf:resource="http://www.dronetology.net/dronetology#GroundStation"/>
            </owl:Restriction>
        </rdfs:subClassOf>
        <rdfs:comment xml:lang="en">UAS. Unmanned aircraft system (UAS) means an unmanned aircraft and the equipment to control it remotely.</rdfs:comment>
        <rdfs:label xml:lang="en">UAS</rdfs:label>
    </owl:Class>
    


    <!-- http://www.dronetology.net/dronetology#UAV -->

    <owl:Class rdf:about="http://www.dronetology.net/dronetology#UAV">
        <rdfs:subClassOf rdf:resource="http://www.dronetology.net/dronetology#Drone"/>
        <rdfs:comment xml:lang="en">UAV. An unmanned aerial vehicle (UAV) is a powered, aerial vehicle that does not carry a human pilot.</rdfs:comment>
        <rdfs:label xml:lang="en">UAV</rdfs:label>
    </owl:Class>
    


    <!-- http://www.dronetology.net/dronetology#UnidentifiedAircraft -->

    <owl:Class rdf:about="http://www.dronetology.net/dronetology#UnidentifiedAircraft">
        <rdfs:subClassOf rdf:resource="http://www.ontologydesignpatterns.org/ont/dul/DUL.owl#PhysicalObject"/>
        <rdfs:comment xml:lang="en">UnidentifiedAircraft. An aircraft which has been observed or reported to be operating in a given area but whose identity has not been established.</rdfs:comment>
        <rdfs:label xml:lang="en">UnidentifiedAircraft</rdfs:label>
    </owl:Class>
    


    <!-- http://www.dronetology.net/dronetology#VLOSMission -->

    <owl:Class rdf:about="http://www.dronetology.net/dronetology#VLOSMission">
        <rdfs:subClassOf rdf:resource="http://www.dronetology.net/dronetology#Mission"/>
        <rdfs:comment xml:lang="en">VLOSMission. Mission in the visual line of sight of the pilot.</rdfs:comment>
        <rdfs:label xml:lang="en">VLOSMission</rdfs:label>
    </owl:Class>
    


    <!-- http://www.dronetology.net/dronetology#VTOLCraft -->

    <owl:Class rdf:about="http://www.dronetology.net/dronetology#VTOLCraft">
        <rdfs:subClassOf rdf:resource="http://www.dronetology.net/dronetology#Drone"/>
        <rdfs:comment xml:lang="en">VTOLCraft. Any aircraft that can take off and land vertically without relying on a runway.</rdfs:comment>
        <rdfs:label xml:lang="en">VTOLCraft</rdfs:label>
    </owl:Class>
    


    <!-- http://www.dronetology.net/dronetology#VerticalTakeOffLandingMission -->

    <owl:Class rdf:about="http://www.dronetology.net/dronetology#VerticalTakeOffLandingMission">
        <rdfs:subClassOf rdf:resource="http://www.dronetology.net/dronetology#Mission"/>
        <rdfs:comment xml:lang="en">VerticalTakeOffLandingMission. Mission defined using vertical takeoff and anding.</rdfs:comment>
        <rdfs:label xml:lang="en">VerticalTakeOffLandingMission</rdfs:label>
    </owl:Class>
    


    <!-- http://www.dronetology.net/dronetology#VerticalTakeoffSpeed -->

    <owl:Class rdf:about="http://www.dronetology.net/dronetology#VerticalTakeoffSpeed">
        <rdfs:subClassOf rdf:resource="http://www.dronetology.net/dronetology#Speed"/>
        <rdfs:comment xml:lang="en">VerticalTakeoffSpeed. The minimum speed at which climb shall be achieved with the critical engine inoperative, the remaining engines operating within approved operating limits.</rdfs:comment>
        <rdfs:label xml:lang="en">VerticalTakeoffSpeed</rdfs:label>
    </owl:Class>
    


    <!-- http://www.dronetology.net/dronetology#Vertiport -->

    <owl:Class rdf:about="http://www.dronetology.net/dronetology#Vertiport">
        <rdfs:subClassOf rdf:resource="http://www.opengis.net/ont/geosparql#Feature"/>
        <rdfs:comment xml:lang="en">Vertiport. A vertiport is a defined area that can support the landing and take-off of eVTOL aircrafts during flight operations.</rdfs:comment>
        <rdfs:label xml:lang="en">Vertiport</rdfs:label>
    </owl:Class>
    


    <!-- http://www.dronetology.net/dronetology#VerySmallUA -->

    <owl:Class rdf:about="http://www.dronetology.net/dronetology#VerySmallUA">
        <rdfs:subClassOf rdf:resource="http://www.dronetology.net/dronetology#Drone"/>
        <rdfs:comment xml:lang="en">VerySmallUA. Unmanned aircraft with size of a large insect to 30-50 cm long.</rdfs:comment>
        <rdfs:label xml:lang="en">VerySmallUA</rdfs:label>
    </owl:Class>
    


    <!-- http://www.dronetology.net/dronetology#Video -->

    <owl:Class rdf:about="http://www.dronetology.net/dronetology#Video">
        <rdfs:subClassOf>
            <owl:Class>
                <owl:intersectionOf rdf:parseType="Collection">
                    <rdf:Description rdf:about="http://www.dronetology.net/dronetology#MissionGeometryElement"/>
                    <rdf:Description rdf:about="http://www.dronetology.net/dronetology#MissionTemporalElement"/>
                </owl:intersectionOf>
            </owl:Class>
        </rdfs:subClassOf>
        <rdfs:subClassOf>
            <owl:Restriction>
                <owl:onProperty rdf:resource="http://www.dronetology.net/dronetology#isStoredIn"/>
                <owl:someValuesFrom rdf:resource="http://www.dronetology.net/dronetology#DataStorageDevice"/>
            </owl:Restriction>
        </rdfs:subClassOf>
        <rdfs:comment xml:lang="en">Video. A recording of moving visual images made digitally using an onboard camera during a mission.</rdfs:comment>
        <rdfs:label xml:lang="en">Video</rdfs:label>
    </owl:Class>
    


    <!-- http://www.dronetology.net/dronetology#Visibility -->

    <owl:Class rdf:about="http://www.dronetology.net/dronetology#Visibility">
        <rdfs:subClassOf rdf:resource="http://qudt.org/schema/qudt/Quantity"/>
        <rdfs:comment xml:lang="en">Visibility. The distance a drone pilot can see as determined by light and weather conditions.</rdfs:comment>
        <rdfs:label xml:lang="en">Visibility</rdfs:label>
    </owl:Class>
    


    <!-- http://www.dronetology.net/dronetology#Waiver -->

    <owl:Class rdf:about="http://www.dronetology.net/dronetology#Waiver">
        <rdfs:subClassOf rdf:resource="http://www.dronetology.net/dronetology#RegulationRequirement"/>
        <rdfs:comment xml:lang="en">Waiver. Allow drone pilots to deviate from certain rules by demonstrating they can still fly safely using alternative methods, applied only in USA.</rdfs:comment>
        <rdfs:label xml:lang="en">Waiver</rdfs:label>
    </owl:Class>
    


    <!-- http://www.dronetology.net/dronetology#Waypoint -->

    <owl:Class rdf:about="http://www.dronetology.net/dronetology#Waypoint">
        <rdfs:subClassOf rdf:resource="http://www.dronetology.net/dronetology#MissionGeometryPointElement"/>
        <rdfs:comment xml:lang="en">Waypoint. Points predefined on the map by the pilot or a planning software that define the UAS flight during a mission.</rdfs:comment>
        <rdfs:label xml:lang="en">Waypoint</rdfs:label>
    </owl:Class>
    


    <!-- http://www.dronetology.net/dronetology#WaypointMission -->

    <owl:Class rdf:about="http://www.dronetology.net/dronetology#WaypointMission">
        <rdfs:subClassOf rdf:resource="http://www.dronetology.net/dronetology#Mission"/>
        <rdfs:comment xml:lang="en">WaypointMission. A mission defined using waypoints.</rdfs:comment>
        <rdfs:label xml:lang="en">WaypointMission</rdfs:label>
    </owl:Class>
    


    <!-- http://www.dronetology.net/dronetology#Weapon -->

    <owl:Class rdf:about="http://www.dronetology.net/dronetology#Weapon">
        <rdfs:subClassOf rdf:resource="http://www.dronetology.net/dronetology#Payload"/>
        <rdfs:comment xml:lang="en">Weapon. A thing designed or used for inflicting bodily harm or physical damage, carried by the drone.</rdfs:comment>
        <rdfs:label xml:lang="en">Weapon</rdfs:label>
    </owl:Class>
    


    <!-- http://www.dronetology.net/dronetology#WeatherReport -->

    <owl:Class rdf:about="http://www.dronetology.net/dronetology#WeatherReport">
        <rdfs:comment xml:lang="en">WeatherReport. A systematic statement of the existing and usually the predicted meteorological conditions over a particular area.</rdfs:comment>
        <rdfs:label xml:lang="en">WeatherReport</rdfs:label>
    </owl:Class>
    


    <!-- http://www.dronetology.net/dronetology#WeatherTemperature -->

    <owl:Class rdf:about="http://www.dronetology.net/dronetology#WeatherTemperature">
        <rdfs:subClassOf rdf:resource="http://qudt.org/schema/qudt/Quantity"/>
        <rdfs:comment xml:lang="en">WeatherTemperature. The temperature that is manifested in the several layers of the atmosphere.</rdfs:comment>
        <rdfs:label xml:lang="en">WeatherTemperature</rdfs:label>
    </owl:Class>
    


    <!-- http://www.dronetology.net/dronetology#WindSpeed -->

    <owl:Class rdf:about="http://www.dronetology.net/dronetology#WindSpeed">
        <rdfs:subClassOf rdf:resource="http://www.dronetology.net/dronetology#Speed"/>
        <rdfs:comment xml:lang="en">WindSpeed. The speed of the weather related air movement from one place to the next.</rdfs:comment>
        <rdfs:label xml:lang="en">WindSpeed</rdfs:label>
    </owl:Class>
    


    <!-- http://www.dronetology.net/dronetology#Wing -->

    <owl:Class rdf:about="http://www.dronetology.net/dronetology#Wing">
        <rdfs:subClassOf rdf:resource="http://www.dronetology.net/dronetology#LiftGeneratorComponent"/>
        <rdfs:subClassOf>
            <owl:Restriction>
                <owl:onProperty rdf:resource="http://www.dronetology.net/dronetology#hasPart"/>
                <owl:allValuesFrom rdf:resource="http://www.dronetology.net/dronetology#WingComponent"/>
            </owl:Restriction>
        </rdfs:subClassOf>
        <rdfs:comment xml:lang="en">Wing. A rigid horizontal structure that projects from both sides of an aircraft and supports it in the air.</rdfs:comment>
        <rdfs:label xml:lang="en">Wing</rdfs:label>
    </owl:Class>
    


    <!-- http://www.dronetology.net/dronetology#WingComponent -->

    <owl:Class rdf:about="http://www.dronetology.net/dronetology#WingComponent">
        <rdfs:subClassOf rdf:resource="http://www.dronetology.net/dronetology#LiftGeneratorComponent"/>
        <rdfs:comment xml:lang="en">WingComponent. Parts of a wing.</rdfs:comment>
        <rdfs:label xml:lang="en">WingComponent</rdfs:label>
    </owl:Class>
    


    <!-- http://www.dronetology.net/dronetology#WingRoot -->

    <owl:Class rdf:about="http://www.dronetology.net/dronetology#WingRoot">
        <rdfs:subClassOf rdf:resource="http://www.dronetology.net/dronetology#WingComponent"/>
        <rdfs:comment xml:lang="en">WingRoot.  The thickest part of the wing.</rdfs:comment>
        <rdfs:label xml:lang="en">WingRoot</rdfs:label>
    </owl:Class>
    


    <!-- http://www.dronetology.net/dronetology#WingTip -->

    <owl:Class rdf:about="http://www.dronetology.net/dronetology#WingTip">
        <rdfs:subClassOf rdf:resource="http://www.dronetology.net/dronetology#WingComponent"/>
        <rdfs:comment xml:lang="en">WingTip. The wing tip refers to the outward ends of each wing. It is the part of the wing that is farthest away from the fuselage of the aircraft. The wing tip is designed to improve the aerodynamic performance of the aircraft and reduce drag.</rdfs:comment>
        <rdfs:label xml:lang="en">WingTip</rdfs:label>
    </owl:Class>
    


    <!-- http://www.dronetology.net/dronetology#Yaw -->

    <owl:Class rdf:about="http://www.dronetology.net/dronetology#Yaw">
        <rdfs:subClassOf rdf:resource="http://qudt.org/schema/qudt/Quantity"/>
        <rdfs:comment xml:lang="en">Yaw. A spin on the Z axis to face a direction. The ability to point the drone in a direction before making it go that way.</rdfs:comment>
        <rdfs:label xml:lang="en">Yaw</rdfs:label>
    </owl:Class>
    


    <!-- http://www.dronetology.net/dronetology#eVTOL -->

    <owl:Class rdf:about="http://www.dronetology.net/dronetology#eVTOL">
        <rdfs:subClassOf>
            <owl:Class>
                <owl:intersectionOf rdf:parseType="Collection">
                    <rdf:Description rdf:about="http://www.dronetology.net/dronetology#VTOLCraft"/>
                    <owl:Restriction>
                        <owl:onProperty rdf:resource="http://www.dronetology.net/dronetology#hasPart"/>
                        <owl:someValuesFrom rdf:resource="http://www.dronetology.net/dronetology#ElectricalEngine"/>
                    </owl:Restriction>
                </owl:intersectionOf>
            </owl:Class>
        </rdfs:subClassOf>
        <rdfs:comment xml:lang="en">eVTOL. An electric Vertical Take-Off and Landing aircraft.</rdfs:comment>
        <rdfs:label xml:lang="en">eVTOL</rdfs:label>
    </owl:Class>
    


    <!-- http://www.ontologydesignpatterns.org/ont/dul/DUL.owl#Event -->

    <owl:Class rdf:about="http://www.ontologydesignpatterns.org/ont/dul/DUL.owl#Event"/>
    


    <!-- http://www.ontologydesignpatterns.org/ont/dul/DUL.owl#Goal -->

    <owl:Class rdf:about="http://www.ontologydesignpatterns.org/ont/dul/DUL.owl#Goal"/>
    


    <!-- http://www.ontologydesignpatterns.org/ont/dul/DUL.owl#NaturalPerson -->

    <owl:Class rdf:about="http://www.ontologydesignpatterns.org/ont/dul/DUL.owl#NaturalPerson"/>
    


    <!-- http://www.ontologydesignpatterns.org/ont/dul/DUL.owl#PhysicalObject -->

    <owl:Class rdf:about="http://www.ontologydesignpatterns.org/ont/dul/DUL.owl#PhysicalObject"/>
    


    <!-- http://www.opengis.net/ont/geosparql#Feature -->

    <owl:Class rdf:about="http://www.opengis.net/ont/geosparql#Feature"/>
    


    <!-- http://www.opengis.net/ont/geosparql#Geometry -->

    <owl:Class rdf:about="http://www.opengis.net/ont/geosparql#Geometry"/>
    


    <!-- http://www.opengis.net/ont/geosparql#SpatialObject -->

    <owl:Class rdf:about="http://www.opengis.net/ont/geosparql#SpatialObject"/>
    


    <!-- http://www.opengis.net/ont/sf#Point -->

    <owl:Class rdf:about="http://www.opengis.net/ont/sf#Point"/>
    


    <!-- http://www.w3.org/2003/01/geo/SpatialThing -->

    <owl:Class rdf:about="http://www.w3.org/2003/01/geo/SpatialThing"/>
    


    <!-- http://www.w3.org/2006/time#Instant -->

    <owl:Class rdf:about="http://www.w3.org/2006/time#Instant"/>
    


    <!-- http://www.w3.org/2006/time#Interval -->

    <owl:Class rdf:about="http://www.w3.org/2006/time#Interval"/>
    


    <!-- http://www.w3.org/2006/time#TemporalEntity -->

    <owl:Class rdf:about="http://www.w3.org/2006/time#TemporalEntity"/>
    


    <!-- http://www.w3.org/ns/sosa#Sensor -->

    <owl:Class rdf:about="http://www.w3.org/ns/sosa#Sensor"/>
    


    <!-- http://www.w3.org/ns/ssn/SensingDevice -->

    <owl:Class rdf:about="http://www.w3.org/ns/ssn/SensingDevice"/>
    


    <!-- https://qudt.org/vocab/unit/KiloM -->

    <owl:Class rdf:about="https://qudt.org/vocab/unit/KiloM"/>
    


    <!-- 
    ///////////////////////////////////////////////////////////////////////////////////////
    //
    // Individuals
    //
    ///////////////////////////////////////////////////////////////////////////////////////
     -->

    


    <!-- http://www.dronetology.net/dronetology#DronetologyLicenseTerms -->

    <owl:NamedIndividual rdf:about="http://www.dronetology.net/dronetology#DronetologyLicenseTerms">
        <rdf:type rdf:resource="http://purl.org/dc/terms/LicenseDocument"/>
        <dc:description>Release Terms, Information, and Acknowledgments
Dronetology: the UAS domain ontology

Dronetology was developed as a key component of a semantic data integration system built to support integration, query, and search over multiple sources of heterogeneous UAS data.

Dronetology serves as the backbone upon which to overlay data from multiple sources. 

Dronetology incorporates data (provided under any applicable distribution terms and conditions) from the following sources, and we gratefully acknowledges their contribution: Fuvex, NASA, Enaire.

THE DATA IS PROVIDED &quot;AS IS&quot; WITHOUT ANY WARRANTY OF ANY KIND, EITHER EXPRESS, IMPLIED, OR STATUTORY, INCLUDING BUT NOT LIMITED TO, ANY WARRANTY THAT THE DATA WILL CONFORM TO SPECIFICATIONS, ANY IMPLIED WARRANTIES OF MERCHANTABILITY, FITNESS FOR A PARTICULAR PURPOSE, FREEDOM FROM INFRINGEMENT, OR ANY WARRANTY THAT THE DATA WILL BE ERROR FREE OR ANY WARRANTY THAT RELATED DOCUMENTATION/RELEASE NOTES WILL CONFORM TO THE DATA PROVIDED. 
IN NO EVENT SHALL THE AUTHORS BE LIABLE FOR ANY DAMAGES, INCLUDING BUT NOT LIMITED TO, DIRECT, INDIRECT, SPECIAL OR CONSEQUENTIAL DAMAGES, ARISING OUT OF OR RESULTING FROM OR IN ANY WAY CONNECTED WITH THIS DATA.  
</dc:description>
    </owl:NamedIndividual>
    <rdf:Description>
        <owl:minCardinality rdf:datatype="http://www.w3.org/2001/XMLSchema#nonNegativeInteger">100</owl:minCardinality>
    </rdf:Description>
    <rdf:Description>
        <owl:maxCardinality rdf:datatype="http://www.w3.org/2001/XMLSchema#nonNegativeInteger">500</owl:maxCardinality>
    </rdf:Description>
    


    <!-- 
    ///////////////////////////////////////////////////////////////////////////////////////
    //
    // General axioms
    //
    ///////////////////////////////////////////////////////////////////////////////////////
     -->

    <rdf:Description>
        <rdf:type rdf:resource="http://www.w3.org/2002/07/owl#AllDisjointClasses"/>
        <owl:members rdf:parseType="Collection">
            <rdf:Description rdf:about="http://www.dronetology.net/dronetology#Beidou"/>
            <rdf:Description rdf:about="http://www.dronetology.net/dronetology#GLONASS"/>
            <rdf:Description rdf:about="http://www.dronetology.net/dronetology#GPS"/>
            <rdf:Description rdf:about="http://www.dronetology.net/dronetology#Galileo"/>
            <rdf:Description rdf:about="http://www.dronetology.net/dronetology#IRNSS"/>
            <rdf:Description rdf:about="http://www.dronetology.net/dronetology#QZSS"/>
        </owl:members>
    </rdf:Description>
    <rdf:Description>
        <rdf:type rdf:resource="http://www.w3.org/2002/07/owl#AllDisjointClasses"/>
        <owl:members rdf:parseType="Collection">
            <rdf:Description rdf:about="http://www.dronetology.net/dronetology#Group1"/>
            <rdf:Description rdf:about="http://www.dronetology.net/dronetology#Group2"/>
            <rdf:Description rdf:about="http://www.dronetology.net/dronetology#Group3"/>
            <rdf:Description rdf:about="http://www.dronetology.net/dronetology#Group4"/>
            <rdf:Description rdf:about="http://www.dronetology.net/dronetology#Group5"/>
        </owl:members>
    </rdf:Description>
    <rdf:Description>
        <rdf:type rdf:resource="http://www.w3.org/2002/07/owl#AllDisjointClasses"/>
        <owl:members rdf:parseType="Collection">
            <rdf:Description rdf:about="http://www.dronetology.net/dronetology#HALE"/>
            <rdf:Description rdf:about="http://www.dronetology.net/dronetology#LALE"/>
            <rdf:Description rdf:about="http://www.dronetology.net/dronetology#LASE"/>
            <rdf:Description rdf:about="http://www.dronetology.net/dronetology#MALE"/>
            <rdf:Description rdf:about="http://www.dronetology.net/dronetology#MAV"/>
        </owl:members>
    </rdf:Description>
</rdf:RDF>



<!-- Generated by the OWL API (version 4.2.8.20170104-2310) https://github.com/owlcs/owlapi -->

